<?xml version="1.0"?>
<rdf:RDF xmlns="https://w3id.org/rains#"
     xml:base="https://w3id.org/rains"
     xmlns:ns="http://creativecommons.org/ns#"
     xmlns:owl="http://www.w3.org/2002/07/owl#"
     xmlns:rdf="http://www.w3.org/1999/02/22-rdf-syntax-ns#"
     xmlns:xml="http://www.w3.org/XML/1998/namespace"
     xmlns:xsd="http://www.w3.org/2001/XMLSchema#"
     xmlns:rdfs="http://www.w3.org/2000/01/rdf-schema#"
     xmlns:vann="http://purl.org/vocab/vann/"
     xmlns:terms="http://purl.org/dc/terms/">
    <owl:Ontology rdf:about="https://w3id.org/rains">
        <ns:license rdf:resource="https://creativecommons.org/licenses/by-nc-sa/4.0/"/>
        <terms:creator rdf:resource="https://www.abdn.ac.uk/ncs/profiles/iman.naja"/>
        <terms:creator rdf:resource="https://www.abdn.ac.uk/ncs/profiles/p.edwards"/>
        <terms:creator rdf:resource="https://www.abdn.ac.uk/ncs/profiles/milan.markovic/"/>
        <terms:description xml:lang="en">An ontology to model accountability of AI systems which use machine learning.</terms:description>
        <terms:issued rdf:datatype="http://www.w3.org/2001/XMLSchema#date">2020-12-18</terms:issued>
        <terms:modified xml:lang="en">2022-06-29</terms:modified>
        <terms:rights>Copyright 2020 University of Aberdeen</terms:rights>
        <terms:title xml:lang="en">The RAInS Ontology</terms:title>
        <vann:preferredNamespacePrefix>rains</vann:preferredNamespacePrefix>
        <vann:preferredNamespaceUri>https://w3id.org/rains#</vann:preferredNamespaceUri>
        <rdfs:comment xml:lang="en">-Version 3.0: added classes and relationships to model the Deployment and Operation stages of an AI system 
-Version 2.2: Some more minor edits to Guideline, Guideance, and Log classes and their subclasses. Plus minor edits to rdf:comments describing some Entities and Properties so that the description is clearer to the reader.
-Version 2.1: minor edits and additions of relationships: corrected the range of version and added the dropped properties hasInputFormat and hasOutputFormat. Plus minor edits and additions to the ontology metadata to reflect LOV requirements. 
-Version 2.0: added classes and relationships to model the Implementation stage of an AI system 
-Version 1.1: creation, models the Design stage of an AI system</rdfs:comment>
        <rdfs:comment xml:lang="en">To contact the RAInS team, please send an email to therainsproject [at] gmail [dot] com</rdfs:comment>
        <rdfs:label xml:lang="en">The RAInS Ontology</rdfs:label>
        <owl:versionInfo xml:lang="en">3.0</owl:versionInfo>
    </owl:Ontology>
    


    <!-- 
    ///////////////////////////////////////////////////////////////////////////////////////
    //
    // Annotation properties
    //
    ///////////////////////////////////////////////////////////////////////////////////////
     -->


    


    <!-- http://creativecommons.org/ns#license -->


    <owl:AnnotationProperty rdf:about="http://creativecommons.org/ns#license"/>
    


    <!-- http://purl.org/dc/terms/creator -->


    <owl:AnnotationProperty rdf:about="http://purl.org/dc/terms/creator"/>
    


    <!-- http://purl.org/dc/terms/description -->


    <owl:AnnotationProperty rdf:about="http://purl.org/dc/terms/description"/>
    


    <!-- http://purl.org/dc/terms/issued -->


    <owl:AnnotationProperty rdf:about="http://purl.org/dc/terms/issued"/>
    


    <!-- http://purl.org/dc/terms/modified -->


    <owl:AnnotationProperty rdf:about="http://purl.org/dc/terms/modified"/>
    


    <!-- http://purl.org/dc/terms/rights -->


    <owl:AnnotationProperty rdf:about="http://purl.org/dc/terms/rights"/>
    


    <!-- http://purl.org/dc/terms/title -->


    <owl:AnnotationProperty rdf:about="http://purl.org/dc/terms/title"/>
    


    <!-- http://purl.org/vocab/vann/preferredNamespacePrefix -->


    <owl:AnnotationProperty rdf:about="http://purl.org/vocab/vann/preferredNamespacePrefix"/>
    


    <!-- http://purl.org/vocab/vann/preferredNamespaceUri -->


    <owl:AnnotationProperty rdf:about="http://purl.org/vocab/vann/preferredNamespaceUri"/>
    


    <!-- 
    ///////////////////////////////////////////////////////////////////////////////////////
    //
    // Datatypes
    //
    ///////////////////////////////////////////////////////////////////////////////////////
     -->


    


    <!-- http://www.w3.org/2001/XMLSchema#date -->


    <rdfs:Datatype rdf:about="http://www.w3.org/2001/XMLSchema#date"/>
    


    <!-- 
    ///////////////////////////////////////////////////////////////////////////////////////
    //
    // Object Properties
    //
    ///////////////////////////////////////////////////////////////////////////////////////
     -->


    


    <!-- https://w3id.org/ep-plan#hasInputVariable -->


    <owl:ObjectProperty rdf:about="https://w3id.org/ep-plan#hasInputVariable"/>
    


    <!-- https://w3id.org/ep-plan#hasOutputVariable -->


    <owl:ObjectProperty rdf:about="https://w3id.org/ep-plan#hasOutputVariable"/>
    


    <!-- https://w3id.org/ep-plan#includesPlanElement -->


    <owl:ObjectProperty rdf:about="https://w3id.org/ep-plan#includesPlanElement"/>
    


    <!-- https://w3id.org/ep-plan#includesStep -->


    <owl:ObjectProperty rdf:about="https://w3id.org/ep-plan#includesStep">
        <owl:inverseOf rdf:resource="https://w3id.org/ep-plan#isStepOfPlan"/>
    </owl:ObjectProperty>
    


    <!-- https://w3id.org/ep-plan#includesVariable -->


    <owl:ObjectProperty rdf:about="https://w3id.org/ep-plan#includesVariable"/>
    


    <!-- https://w3id.org/ep-plan#isElementOfPlan -->


    <owl:ObjectProperty rdf:about="https://w3id.org/ep-plan#isElementOfPlan"/>
    


    <!-- https://w3id.org/ep-plan#isInputVariableOf -->


    <owl:ObjectProperty rdf:about="https://w3id.org/ep-plan#isInputVariableOf"/>
    


    <!-- https://w3id.org/ep-plan#isOutputVariableOf -->


    <owl:ObjectProperty rdf:about="https://w3id.org/ep-plan#isOutputVariableOf">
        <rdfs:subPropertyOf rdf:resource="http://www.w3.org/2002/07/owl#topObjectProperty"/>
    </owl:ObjectProperty>
    


    <!-- https://w3id.org/ep-plan#isStepOfPlan -->


    <owl:ObjectProperty rdf:about="https://w3id.org/ep-plan#isStepOfPlan"/>
    


    <!-- https://w3id.org/ep-plan#isVariableOfPlan -->


    <owl:ObjectProperty rdf:about="https://w3id.org/ep-plan#isVariableOfPlan"/>
    


    <!-- https://w3id.org/rains#hasEvaluationResult -->


    <owl:ObjectProperty rdf:about="https://w3id.org/rains#hasEvaluationResult">
        <owl:inverseOf rdf:resource="https://w3id.org/rains#isEvaluationResultOf"/>
        <rdfs:domain rdf:resource="https://w3id.org/rains#EvaluationMeassure"/>
        <rdfs:range rdf:resource="https://w3id.org/rains#EvaluationResult"/>
        <rdfs:comment>A relation that links some evaluation measure to one or more results produced for this measure.</rdfs:comment>
        <rdfs:label>hasEvaluationResult</rdfs:label>
    </owl:ObjectProperty>
    


    <!-- https://w3id.org/rains#hasExplanation -->


    <owl:ObjectProperty rdf:about="https://w3id.org/rains#hasExplanation">
        <owl:inverseOf rdf:resource="https://w3id.org/rains#isExplanationOf"/>
        <rdfs:domain rdf:resource="https://w3id.org/rains#SystemOutput"/>
        <rdfs:range rdf:resource="https://w3id.org/rains#Explanation"/>
        <rdfs:comment>A relation that links some system output to an explanation.</rdfs:comment>
        <rdfs:label>hasExplanation</rdfs:label>
    </owl:ObjectProperty>
    


    <!-- https://w3id.org/rains#hasJustification -->


    <owl:ObjectProperty rdf:about="https://w3id.org/rains#hasJustification">
        <owl:inverseOf rdf:resource="https://w3id.org/rains#isJustificationOf"/>
        <rdfs:domain rdf:resource="https://w3id.org/rains#OverrideResult"/>
        <rdfs:range rdf:resource="https://w3id.org/rains#ChangeLog"/>
        <rdfs:comment>A relation that links some override result to a justification.</rdfs:comment>
        <rdfs:label>hasJustification</rdfs:label>
    </owl:ObjectProperty>
    


    <!-- https://w3id.org/rains#hasRealizableObjectCharacteristic -->


    <owl:ObjectProperty rdf:about="https://w3id.org/rains#hasRealizableObjectCharacteristic">
        <owl:inverseOf rdf:resource="https://w3id.org/rains#isCharacteristicOfRealizableObject"/>
        <rdfs:domain rdf:resource="https://w3id.org/rains#RealizableObject"/>
        <rdfs:range rdf:resource="https://w3id.org/rains#RealizableObjectCharacteristic"/>
        <rdfs:comment>A relation that links a realizable object (e.g., model) to the information element describing its characteristic.</rdfs:comment>
        <rdfs:label>hasRealizableObjectCharacteristic</rdfs:label>
    </owl:ObjectProperty>
    


    <!-- https://w3id.org/rains#isCharacteristicOfRealizableObject -->


    <owl:ObjectProperty rdf:about="https://w3id.org/rains#isCharacteristicOfRealizableObject">
        <rdfs:domain rdf:resource="https://w3id.org/rains#RealizableObjectCharacteristic"/>
        <rdfs:range rdf:resource="https://w3id.org/rains#RealizableObject"/>
        <rdfs:comment>Inverse of hasRealizableObjectCharacteristic.</rdfs:comment>
        <rdfs:label>isCharacteristicOfRealizableObject</rdfs:label>
    </owl:ObjectProperty>
    


    <!-- https://w3id.org/rains#isEvaluationResultOf -->


    <owl:ObjectProperty rdf:about="https://w3id.org/rains#isEvaluationResultOf">
        <rdfs:domain rdf:resource="https://w3id.org/rains#EvaluationResult"/>
        <rdfs:range rdf:resource="https://w3id.org/rains#EvaluationMeassure"/>
        <rdfs:comment>A relation that links a result to some evaluation measure for which the result was produced. This property is the inverse of hasEvaluationResult.</rdfs:comment>
        <rdfs:label>isEvaluationResultOf</rdfs:label>
    </owl:ObjectProperty>
    


    <!-- https://w3id.org/rains#isExplanationOf -->


    <owl:ObjectProperty rdf:about="https://w3id.org/rains#isExplanationOf">
        <rdfs:comment>A relation that links an explanation to some system output. This property is the inverse of hasExplanation.</rdfs:comment>
    </owl:ObjectProperty>
    


    <!-- https://w3id.org/rains#isJustificationOf -->


    <owl:ObjectProperty rdf:about="https://w3id.org/rains#isJustificationOf">
        <rdfs:comment>A relation that links a justification to an override result. This property is the inverse of hasJustification.</rdfs:comment>
        <rdfs:label>isJustification</rdfs:label>
    </owl:ObjectProperty>
    


    <!-- 
    ///////////////////////////////////////////////////////////////////////////////////////
    //
    // Data properties
    //
    ///////////////////////////////////////////////////////////////////////////////////////
     -->


    


    <!-- https://w3id.org/rains#computedOnDecisionThreshold -->


    <owl:DatatypeProperty rdf:about="https://w3id.org/rains#computedOnDecisionThreshold">
        <rdf:type rdf:resource="http://www.w3.org/2002/07/owl#FunctionalProperty"/>
        <rdfs:domain rdf:resource="https://w3id.org/rains#EvaluationResult"/>
        <rdfs:comment>The decision threshold the metric that produced evaluation result was computed on. Inspired by the Model Card Toolkit schema https://github.com/tensorflow/model-card-toolkit/blob/master/model_card_toolkit/schema/v0.0.1/model_card.schema.json</rdfs:comment>
        <rdfs:label>computedOnDecisionThreshold</rdfs:label>
    </owl:DatatypeProperty>
    


    <!-- https://w3id.org/rains#computedOnSlice -->


    <owl:DatatypeProperty rdf:about="https://w3id.org/rains#computedOnSlice">
        <rdf:type rdf:resource="http://www.w3.org/2002/07/owl#FunctionalProperty"/>
        <rdfs:domain rdf:resource="https://w3id.org/rains#EvaluationResult"/>
        <rdfs:comment>The description of slice that the metric which  produced evaluation result was computed on. Inspired by the Model Card Toolkit schema https://github.com/tensorflow/model-card-toolkit/blob/master/model_card_toolkit/schema/v0.0.1/model_card.schema.json</rdfs:comment>
        <rdfs:label>computedOnSlice</rdfs:label>
    </owl:DatatypeProperty>
    


    <!-- https://w3id.org/rains#hasBase64Image -->


    <owl:DatatypeProperty rdf:about="https://w3id.org/rains#hasBase64Image">
        <rdfs:domain rdf:resource="https://w3id.org/sao#InformationElement"/>
        <rdfs:range rdf:resource="http://www.w3.org/2001/XMLSchema#string"/>
        <rdfs:comment>A value indicating what an :InformationElement&apos;s base 64 image is in String format. Inspired by the Model Card Toolkit schema https://github.com/tensorflow/model-card-toolkit/blob/master/model_card_toolkit/schema/v0.0.1/model_card.schema.json</rdfs:comment>
        <rdfs:label>hasBase64Image</rdfs:label>
    </owl:DatatypeProperty>
    


    <!-- https://w3id.org/rains#hasConfidenceLevel -->


    <owl:DatatypeProperty rdf:about="https://w3id.org/rains#hasConfidenceLevel">
        <rdfs:domain rdf:resource="https://w3id.org/rains#SystemOutput"/>
        <rdfs:range rdf:resource="http://www.w3.org/2001/XMLSchema#decimal"/>
        <rdfs:comment>A value indicating the level of confidence in an output.</rdfs:comment>
        <rdfs:label>hasConfidenceLevel</rdfs:label>
    </owl:DatatypeProperty>
    


    <!-- https://w3id.org/rains#hasInputFormat -->


    <owl:DatatypeProperty rdf:about="https://w3id.org/rains#hasInputFormat">
        <rdfs:range rdf:resource="http://www.w3.org/2001/XMLSchema#string"/>
        <rdfs:comment>A value describing the format of an input. Inspired by the Model Card Toolkit schema https://github.com/tensorflow/model-card-toolkit/blob/master/model_card_toolkit/schema/v0.0.1/model_card.schema.json</rdfs:comment>
        <rdfs:label>hasInputFormat</rdfs:label>
    </owl:DatatypeProperty>
    


    <!-- https://w3id.org/rains#hasMitigationStrategy -->


    <owl:DatatypeProperty rdf:about="https://w3id.org/rains#hasMitigationStrategy">
        <rdfs:domain rdf:resource="https://w3id.org/rains#Risk"/>
        <rdfs:range rdf:resource="http://www.w3.org/2001/XMLSchema#string"/>
        <rdfs:comment>A value indicating what a :Risk&apos;s mitigation strategy is, expressed in String format. Inspired by the Model Card Toolkit schema https://github.com/tensorflow/model-card-toolkit/blob/master/model_card_toolkit/schema/v0.0.1/model_card.schema.json</rdfs:comment>
        <rdfs:label>hasMitigationStrategy</rdfs:label>
    </owl:DatatypeProperty>
    


    <!-- https://w3id.org/rains#hasOutputFormat -->


    <owl:DatatypeProperty rdf:about="https://w3id.org/rains#hasOutputFormat">
        <rdfs:range rdf:resource="http://www.w3.org/2001/XMLSchema#string"/>
        <rdfs:comment>A value describing the format of an output. Inspired by the Model Card Toolkit schema https://github.com/tensorflow/model-card-toolkit/blob/master/model_card_toolkit/schema/v0.0.1/model_card.schema.json</rdfs:comment>
        <rdfs:label>hasOutputFormat</rdfs:label>
    </owl:DatatypeProperty>
    


    <!-- https://w3id.org/rains#hasResultLowerBound -->


    <owl:DatatypeProperty rdf:about="https://w3id.org/rains#hasResultLowerBound">
        <rdf:type rdf:resource="http://www.w3.org/2002/07/owl#FunctionalProperty"/>
        <rdfs:domain rdf:resource="https://w3id.org/rains#EvaluationResult"/>
        <rdfs:comment>The lower bound of the confidence interval. Inspired by the Model Card Toolkit schema https://github.com/tensorflow/model-card-toolkit/blob/master/model_card_toolkit/schema/v0.0.1/model_card.schema.json</rdfs:comment>
        <rdfs:label>hasResultLowerBound</rdfs:label>
    </owl:DatatypeProperty>
    


    <!-- https://w3id.org/rains#hasResultUpperBound -->


    <owl:DatatypeProperty rdf:about="https://w3id.org/rains#hasResultUpperBound">
        <rdf:type rdf:resource="http://www.w3.org/2002/07/owl#FunctionalProperty"/>
        <rdfs:domain rdf:resource="https://w3id.org/rains#EvaluationResult"/>
        <rdfs:comment>The upper bound of the confidence interval.

Inspired by the Model Card Toolkit schema https://github.com/tensorflow/model-card-toolkit/blob/master/model_card_toolkit/schema/v0.0.1/model_card.schema.json</rdfs:comment>
        <rdfs:label>hasResultUpperBound</rdfs:label>
    </owl:DatatypeProperty>
    


    <!-- https://w3id.org/rains#hasResultValue -->


    <owl:DatatypeProperty rdf:about="https://w3id.org/rains#hasResultValue">
        <rdf:type rdf:resource="http://www.w3.org/2002/07/owl#FunctionalProperty"/>
        <rdfs:domain rdf:resource="https://w3id.org/rains#EvaluationResult"/>
        <rdfs:comment>The description of the result value.</rdfs:comment>
        <rdfs:label>hasResultValue</rdfs:label>
    </owl:DatatypeProperty>
    


    <!-- https://w3id.org/rains#isFinalSystemOutput -->


    <owl:DatatypeProperty rdf:about="https://w3id.org/rains#isFinalSystemOutput">
        <rdfs:domain rdf:resource="https://w3id.org/rains#SystemOutput"/>
        <rdfs:range rdf:resource="http://www.w3.org/2001/XMLSchema#boolean"/>
        <rdfs:comment>A valuae indicating whether or not an output is the final output produced by the system.</rdfs:comment>
        <rdfs:label>isFinalSystemOutput</rdfs:label>
    </owl:DatatypeProperty>
    


    <!-- https://w3id.org/rains#isReusedObject -->


    <owl:DatatypeProperty rdf:about="https://w3id.org/rains#isReusedObject">
        <rdf:type rdf:resource="http://www.w3.org/2002/07/owl#FunctionalProperty"/>
        <rdfs:domain>
            <owl:Class>
                <owl:unionOf rdf:parseType="Collection">
                    <rdf:Description rdf:about="http://ontosoft.org/software#Software"/>
                    <rdf:Description rdf:about="https://w3id.org/rains#ExcludedObject"/>
                    <rdf:Description rdf:about="https://w3id.org/rains#RealizableObject"/>
                    <rdf:Description rdf:about="https://w3id.org/rains#RealizededObject"/>
                </owl:unionOf>
            </owl:Class>
        </rdfs:domain>
        <rdfs:range rdf:resource="http://www.w3.org/2001/XMLSchema#boolean"/>
        <rdfs:comment>A value indicating whether the :RealizableObject is a third party resource.</rdfs:comment>
        <rdfs:label>isReusedObject</rdfs:label>
    </owl:DatatypeProperty>
    


    <!-- https://w3id.org/rains#version -->


    <owl:DatatypeProperty rdf:about="https://w3id.org/rains#version">
        <rdf:type rdf:resource="http://www.w3.org/2002/07/owl#FunctionalProperty"/>
        <rdfs:domain>
            <owl:Class>
                <owl:unionOf rdf:parseType="Collection">
                    <rdf:Description rdf:about="http://ontosoft.org/software#Software"/>
                    <rdf:Description rdf:about="https://w3id.org/rains#ExcludedObject"/>
                    <rdf:Description rdf:about="https://w3id.org/rains#RealizableObject"/>
                    <rdf:Description rdf:about="https://w3id.org/rains#RealizededObject"/>
                </owl:unionOf>
            </owl:Class>
        </rdfs:domain>
        <rdfs:range rdf:resource="http://www.w3.org/2001/XMLSchema#string"/>
        <rdfs:comment>A value indicating what a :RealizableObject&apos;s version is. Inspired by the Model Card Toolkit schema https://github.com/tensorflow/model-card-toolkit/blob/master/model_card_toolkit/schema/v0.0.1/model_card.schema.json</rdfs:comment>
        <rdfs:label>version</rdfs:label>
    </owl:DatatypeProperty>
    


    <!-- https://w3id.org/rains#versionDate -->


    <owl:DatatypeProperty rdf:about="https://w3id.org/rains#versionDate">
        <rdf:type rdf:resource="http://www.w3.org/2002/07/owl#FunctionalProperty"/>
        <rdfs:domain>
            <owl:Class>
                <owl:unionOf rdf:parseType="Collection">
                    <rdf:Description rdf:about="http://ontosoft.org/software#Software"/>
                    <rdf:Description rdf:about="https://w3id.org/rains#ExcludedObject"/>
                    <rdf:Description rdf:about="https://w3id.org/rains#RealizableObject"/>
                    <rdf:Description rdf:about="https://w3id.org/rains#RealizededObject"/>
                </owl:unionOf>
            </owl:Class>
        </rdfs:domain>
        <rdfs:range rdf:resource="http://www.w3.org/2001/XMLSchema#dateTime"/>
        <rdfs:comment>A value indicating what the version date of a :RealizableObject&apos;s is. Inspired by the Model Card Toolkit schema https://github.com/tensorflow/model-card-toolkit/blob/master/model_card_toolkit/schema/v0.0.1/model_card.schema.json</rdfs:comment>
        <rdfs:label>versionDate</rdfs:label>
    </owl:DatatypeProperty>
    


    <!-- https://w3id.org/rains#versionNote -->


    <owl:DatatypeProperty rdf:about="https://w3id.org/rains#versionNote">
        <rdfs:domain>
            <owl:Class>
                <owl:unionOf rdf:parseType="Collection">
                    <rdf:Description rdf:about="http://ontosoft.org/software#Software"/>
                    <rdf:Description rdf:about="https://w3id.org/rains#ExcludedObject"/>
                    <rdf:Description rdf:about="https://w3id.org/rains#RealizableObject"/>
                    <rdf:Description rdf:about="https://w3id.org/rains#RealizededObject"/>
                </owl:unionOf>
            </owl:Class>
        </rdfs:domain>
        <rdfs:range rdf:resource="http://www.w3.org/2001/XMLSchema#string"/>
        <rdfs:comment>A value describing a note about the version date of a :RealizableObject. Inspired by the Model Card Toolkit schema https://github.com/tensorflow/model-card-toolkit/blob/master/model_card_toolkit/schema/v0.0.1/model_card.schema.json</rdfs:comment>
        <rdfs:label>versionNote</rdfs:label>
    </owl:DatatypeProperty>
    


    <!-- 
    ///////////////////////////////////////////////////////////////////////////////////////
    //
    // Classes
    //
    ///////////////////////////////////////////////////////////////////////////////////////
     -->


    


    <!-- http://ontosoft.org/software#Software -->


    <owl:Class rdf:about="http://ontosoft.org/software#Software">
        <rdfs:subClassOf rdf:resource="http://www.w3.org/ns/prov#SoftwareAgent"/>
        <rdfs:subClassOf rdf:resource="https://w3id.org/ep-plan#Agent"/>
        <rdfs:subClassOf rdf:resource="https://w3id.org/sao#InformationElement"/>
        <rdfs:comment>Imported definition: A Software is any piece of code that is described in Ontosoft. This could some visualisation software, software package, library, componentised scripts, etc. This can be subclassed if software categories with extra properties are required, otherwise one should use SoftwareTag to categorise software.</rdfs:comment>
    </owl:Class>
    


    <!-- http://purl.org/dc/terms/LicenseDocument -->


    <owl:Class rdf:about="http://purl.org/dc/terms/LicenseDocument">
        <rdfs:subClassOf rdf:resource="https://w3id.org/sao#InformationElement"/>
        <rdfs:comment>Imported definition: A legal document giving official permission to do something with a resource.</rdfs:comment>
    </owl:Class>
    


    <!-- http://www.w3.org/ns/mls#Algorithm -->


    <owl:Class rdf:about="http://www.w3.org/ns/mls#Algorithm">
        <rdfs:subClassOf rdf:resource="https://w3id.org/rains#RealizableObjectCharacteristic"/>
        <rdfs:comment>Imported Definition: The algorithm regardless software implementation.</rdfs:comment>
    </owl:Class>
    


    <!-- http://www.w3.org/ns/mls#Dataset -->


    <owl:Class rdf:about="http://www.w3.org/ns/mls#Dataset">
        <rdfs:subClassOf rdf:resource="https://w3id.org/rains#RealizableObject"/>
        <rdfs:subClassOf>
            <owl:Class>
                <owl:unionOf rdf:parseType="Collection">
                    <rdf:Description rdf:about="https://w3id.org/rains#ExcludedObject"/>
                    <rdf:Description rdf:about="https://w3id.org/rains#RealizededObject"/>
                </owl:unionOf>
            </owl:Class>
        </rdfs:subClassOf>
        <rdfs:comment>A set composed of data item(s).</rdfs:comment>
        <rdfs:label>Dataset</rdfs:label>
    </owl:Class>
    


    <!-- http://www.w3.org/ns/mls#DatasetCharacteristic -->


    <owl:Class rdf:about="http://www.w3.org/ns/mls#DatasetCharacteristic">
        <rdfs:subClassOf rdf:resource="https://w3id.org/rains#RealizableObjectCharacteristic"/>
        <rdfs:comment>This concept is imported from ML-Schema to describe the characteristics of the dataset. 

In RAInS, this includes how many instances make up the dataset, what do the instances represent, what are the types of instances, whether the instances have associated labels or targets, whether the relationships between instances are explicit, as well as the errors, noises, redundancies in the dataset and whether is there any information missing from instances.

When used to describe a Training Dataset, Validation Dataset, or Evaluation Dataset produced by splitting the Dataset Component, it is advisable to describe how the dataset was split, including the ratios of train-validate-test and the class representation percentage in each.</rdfs:comment>
    </owl:Class>
    


    <!-- http://www.w3.org/ns/mls#EvaluationMeasure -->


    <owl:Class rdf:about="http://www.w3.org/ns/mls#EvaluationMeasure">
        <rdfs:subClassOf rdf:resource="https://w3id.org/rains#EvaluationMeassure"/>
        <rdfs:comment>A  specific rains:EvaluationMeasure which records a specific piece of  information detailing some measure used as part of an evaluation process of the Model Component.
Imported defintion from ML-Schema: EvaluationMeasure is a measure to assess the performance of the model generated by the process that realizes the task. Examples are predictive accuracy or f-measure.</rdfs:comment>
        <rdfs:label>Evaluation Measure</rdfs:label>
    </owl:Class>
    


    <!-- http://www.w3.org/ns/mls#EvaluationProcedure -->


    <owl:Class rdf:about="http://www.w3.org/ns/mls#EvaluationProcedure">
        <rdfs:subClassOf rdf:resource="https://w3id.org/rains#EvaluationProcedure"/>
        <rdfs:comment>A specific type of rains:EvaluationProcedure which records a specific piece of  information detailing the procedure by which a Model Component was evaluated.
Imported Definition from ML-Schema: EvaluationProcedure is a technique to evaluate machine learning models. Examples are cross-validation and leave-one-out.</rdfs:comment>
        <rdfs:label>Evaluation Procedure</rdfs:label>
    </owl:Class>
    


    <!-- http://www.w3.org/ns/mls#HyperParameter -->


    <owl:Class rdf:about="http://www.w3.org/ns/mls#HyperParameter">
        <rdfs:subClassOf rdf:resource="https://w3id.org/rains#Parameter"/>
        <rdfs:comment>Imported Definition: Hyperparameter is a prior parameter of an implementation, i.e., a parameter which is set before its execution (e.g. C, the complexity parameter, in weka.SMO).</rdfs:comment>
        <rdfs:label>Hyperparameter</rdfs:label>
    </owl:Class>
    


    <!-- http://www.w3.org/ns/mls#Model -->


    <owl:Class rdf:about="http://www.w3.org/ns/mls#Model">
        <rdfs:subClassOf rdf:resource="https://w3id.org/rains#RealizableObject"/>
        <rdfs:subClassOf>
            <owl:Class>
                <owl:unionOf rdf:parseType="Collection">
                    <rdf:Description rdf:about="https://w3id.org/rains#ExcludedObject"/>
                    <rdf:Description rdf:about="https://w3id.org/rains#RealizededObject"/>
                </owl:unionOf>
            </owl:Class>
        </rdfs:subClassOf>
        <rdfs:comment>Imported Definition: Model is a generalization of a set of training data able to predict values for unseen instances. It is an output from an execution of a data mining algorithm implementation. Models have a dual nature. They can be treated as data structures and as such represented, stored and manipulated. On the other hand, they act as functions and are executed, taking as input data examples and giving as output the result of applying the function to a data example. Models can also be divided into global or local ones. A global model has global coverage of a data set, i.e., it generalizes the whole data set. A local model, such as a pattern set, is a set of local hypotheses, i.e. each applies to a limited region of the data set.</rdfs:comment>
        <rdfs:label>Model</rdfs:label>
    </owl:Class>
    


    <!-- http://www.w3.org/ns/mls#ModelCharacteristic -->


    <owl:Class rdf:about="http://www.w3.org/ns/mls#ModelCharacteristic">
        <rdfs:subClassOf rdf:resource="https://w3id.org/rains#RealizableObjectCharacteristic"/>
        <rdfs:comment>Imported Definition: ModelCharacteristic is a distinguishing quality or property that distinguish one model from another. An example model characteristic may be interpretabilty or a complexity of the model.

In RAInS, this includes the type of model, programming method, excluded features, emphasized features, decision thresholds, basis of prioritisation, semantics and similarity functions, editorial criteria, and type of uncertainty. Plus, how those were chosen.

There are separate concepts that represent the algorithm and parameters.</rdfs:comment>
    </owl:Class>
    


    <!-- http://www.w3.org/ns/mls#ModelEvaluation -->


    <owl:Class rdf:about="http://www.w3.org/ns/mls#ModelEvaluation">
        <rdfs:subClassOf rdf:resource="https://w3id.org/rains#EvaluationResult"/>
        <rdfs:comment>A  specific rains:EvaluationResult which records a specific piece of  information detailing the result of an evaluation process of a Model Component.
Imported Definition from ML-Schema: ModelEvaluation is a setting of a value of the performance measure  specified by the evaluation specification. It connects a measure specification with its value.</rdfs:comment>
        <rdfs:label>Model Evaluation</rdfs:label>
    </owl:Class>
    


    <!-- http://www.w3.org/ns/prov#Agent -->


    <owl:Class rdf:about="http://www.w3.org/ns/prov#Agent"/>
    


    <!-- http://www.w3.org/ns/prov#SoftwareAgent -->


    <owl:Class rdf:about="http://www.w3.org/ns/prov#SoftwareAgent">
        <rdfs:subClassOf rdf:resource="http://www.w3.org/ns/prov#Agent"/>
    </owl:Class>
    


    <!-- https://w3id.org/ep-plan#Agent -->


    <owl:Class rdf:about="https://w3id.org/ep-plan#Agent">
        <rdfs:subClassOf rdf:resource="http://www.w3.org/ns/prov#Agent"/>
    </owl:Class>
    


    <!-- https://w3id.org/ep-plan#Constraint -->


    <owl:Class rdf:about="https://w3id.org/ep-plan#Constraint"/>
    


    <!-- https://w3id.org/rains#AI_System -->


    <owl:Class rdf:about="https://w3id.org/rains#AI_System">
        <rdfs:subClassOf rdf:resource="https://w3id.org/sao#System"/>
        <rdfs:comment>The AI System for which the accountability plan is specified.</rdfs:comment>
        <rdfs:label>AI System</rdfs:label>
    </owl:Class>
    


    <!-- https://w3id.org/rains#ActuateOutput -->


    <owl:Class rdf:about="https://w3id.org/rains#ActuateOutput">
        <rdfs:subClassOf rdf:resource="https://w3id.org/rains#ReturnOutput"/>
        <rdfs:subClassOf>
            <owl:Restriction>
                <owl:onProperty rdf:resource="https://w3id.org/ep-plan#hasOutputVariable"/>
                <owl:allValuesFrom rdf:resource="https://w3id.org/rains#SystemOutput"/>
            </owl:Restriction>
        </rdfs:subClassOf>
        <rdfs:subClassOf>
            <owl:Restriction>
                <owl:onProperty rdf:resource="https://w3id.org/ep-plan#isElementOfPlan"/>
                <owl:allValuesFrom>
                    <owl:Class>
                        <owl:unionOf rdf:parseType="Collection">
                            <rdf:Description rdf:about="https://w3id.org/rains#OperationStageAccountabilityPlan"/>
                            <rdf:Description rdf:about="https://w3id.org/rains#RuntimeAccountabilityPlan"/>
                        </owl:unionOf>
                    </owl:Class>
                </owl:allValuesFrom>
            </owl:Restriction>
        </rdfs:subClassOf>
        <rdfs:subClassOf>
            <owl:Restriction>
                <owl:onProperty rdf:resource="https://w3id.org/ep-plan#isStepOfPlan"/>
                <owl:allValuesFrom>
                    <owl:Class>
                        <owl:unionOf rdf:parseType="Collection">
                            <rdf:Description rdf:about="https://w3id.org/rains#OperationStageAccountabilityPlan"/>
                            <rdf:Description rdf:about="https://w3id.org/rains#RuntimeAccountabilityPlan"/>
                        </owl:unionOf>
                    </owl:Class>
                </owl:allValuesFrom>
            </owl:Restriction>
        </rdfs:subClassOf>
        <rdfs:comment>A planned step that describes actuating an output by the AI System. This step is typically part of the Operation stage (specifically  Runtime stage) and has a member of the class System Output as its expected output.</rdfs:comment>
        <rdfs:label>Actuate Output</rdfs:label>
    </owl:Class>
    


    <!-- https://w3id.org/rains#AffectedAgent -->


    <owl:Class rdf:about="https://w3id.org/rains#AffectedAgent">
        <rdfs:subClassOf rdf:resource="https://w3id.org/sao#InformationElement"/>
        <rdfs:comment>An agent, typically a human, who has undergone User Training an/or who has been affected directly or indirectly by an AI Systems&apos; output(s) or any of its components&apos; output(s). Within the same AI System a human may take on the role of both or either Affected Agent or Accountable Agent. For example, a user may be accountable for installing and configuring a facial recognition AI system, but may later be affected by the AI System&apos;s output of recognision or not recognision their face. Then may then also be accountable for overriding the system&apos;s output by using a manual passcode.</rdfs:comment>
        <rdfs:label>Affected Agent</rdfs:label>
    </owl:Class>
    


    <!-- https://w3id.org/rains#Aggregate -->


    <owl:Class rdf:about="https://w3id.org/rains#Aggregate">
        <rdfs:subClassOf rdf:resource="https://w3id.org/rains#GenerateOutput"/>
        <rdfs:subClassOf>
            <owl:Restriction>
                <owl:onProperty rdf:resource="https://w3id.org/ep-plan#hasOutputVariable"/>
                <owl:allValuesFrom>
                    <owl:Class>
                        <owl:unionOf rdf:parseType="Collection">
                            <rdf:Description rdf:about="https://w3id.org/rains#AggregationResult"/>
                            <rdf:Description rdf:about="https://w3id.org/rains#Explanation"/>
                        </owl:unionOf>
                    </owl:Class>
                </owl:allValuesFrom>
            </owl:Restriction>
        </rdfs:subClassOf>
        <rdfs:subClassOf>
            <owl:Restriction>
                <owl:onProperty rdf:resource="https://w3id.org/ep-plan#isElementOfPlan"/>
                <owl:allValuesFrom>
                    <owl:Class>
                        <owl:unionOf rdf:parseType="Collection">
                            <rdf:Description rdf:about="https://w3id.org/rains#ConfigurationAccountabilityPlan"/>
                            <rdf:Description rdf:about="https://w3id.org/rains#DeploymentStageAccountabilityPlan"/>
                            <rdf:Description rdf:about="https://w3id.org/rains#InstallationAccountabilityPlan"/>
                            <rdf:Description rdf:about="https://w3id.org/rains#OperationStageAccountabilityPlan"/>
                            <rdf:Description rdf:about="https://w3id.org/rains#RuntimeAccountabilityPlan"/>
                        </owl:unionOf>
                    </owl:Class>
                </owl:allValuesFrom>
            </owl:Restriction>
        </rdfs:subClassOf>
        <rdfs:subClassOf>
            <owl:Restriction>
                <owl:onProperty rdf:resource="https://w3id.org/ep-plan#isStepOfPlan"/>
                <owl:allValuesFrom>
                    <owl:Class>
                        <owl:unionOf rdf:parseType="Collection">
                            <rdf:Description rdf:about="https://w3id.org/rains#ConfigurationAccountabilityPlan"/>
                            <rdf:Description rdf:about="https://w3id.org/rains#DeploymentStageAccountabilityPlan"/>
                            <rdf:Description rdf:about="https://w3id.org/rains#InstallationAccountabilityPlan"/>
                            <rdf:Description rdf:about="https://w3id.org/rains#OperationStageAccountabilityPlan"/>
                            <rdf:Description rdf:about="https://w3id.org/rains#RuntimeAccountabilityPlan"/>
                        </owl:unionOf>
                    </owl:Class>
                </owl:allValuesFrom>
            </owl:Restriction>
        </rdfs:subClassOf>
        <owl:disjointWith rdf:resource="https://w3id.org/rains#GenerateModelOutput"/>
        <owl:disjointWith rdf:resource="https://w3id.org/rains#Override"/>
        <rdfs:comment>A planned step that has some impact on the output of AI System where a user or a system component aggregates some outputs to generate a new (aggregated) output. This step is typically part of the Deplpoyment or Operation Stages (specifically Intallation or Configuration or Runtime Stages) and has a member of the class Aggregation Result as its expected output. It may also generate a member of the class Explanation as its output if it produces an explanation along with the output.</rdfs:comment>
        <rdfs:label>Aggregate</rdfs:label>
    </owl:Class>
    


    <!-- https://w3id.org/rains#AggregationResult -->


    <owl:Class rdf:about="https://w3id.org/rains#AggregationResult">
        <rdfs:subClassOf rdf:resource="https://w3id.org/rains#SystemOutput"/>
        <rdfs:subClassOf>
            <owl:Restriction>
                <owl:onProperty rdf:resource="https://w3id.org/ep-plan#isElementOfPlan"/>
                <owl:allValuesFrom>
                    <owl:Class>
                        <owl:unionOf rdf:parseType="Collection">
                            <rdf:Description rdf:about="https://w3id.org/rains#ConfigurationAccountabilityPlan"/>
                            <rdf:Description rdf:about="https://w3id.org/rains#DeploymentStageAccountabilityPlan"/>
                            <rdf:Description rdf:about="https://w3id.org/rains#InstallationAccountabilityPlan"/>
                            <rdf:Description rdf:about="https://w3id.org/rains#OperationStageAccountabilityPlan"/>
                            <rdf:Description rdf:about="https://w3id.org/rains#RuntimeAccountabilityPlan"/>
                        </owl:unionOf>
                    </owl:Class>
                </owl:allValuesFrom>
            </owl:Restriction>
        </rdfs:subClassOf>
        <rdfs:subClassOf>
            <owl:Restriction>
                <owl:onProperty rdf:resource="https://w3id.org/ep-plan#isOutputVariableOf"/>
                <owl:allValuesFrom rdf:resource="https://w3id.org/rains#Aggregate"/>
            </owl:Restriction>
        </rdfs:subClassOf>
        <rdfs:subClassOf>
            <owl:Restriction>
                <owl:onProperty rdf:resource="https://w3id.org/ep-plan#isVariableOfPlan"/>
                <owl:allValuesFrom>
                    <owl:Class>
                        <owl:unionOf rdf:parseType="Collection">
                            <rdf:Description rdf:about="https://w3id.org/rains#ConfigurationAccountabilityPlan"/>
                            <rdf:Description rdf:about="https://w3id.org/rains#DeploymentStageAccountabilityPlan"/>
                            <rdf:Description rdf:about="https://w3id.org/rains#InstallationAccountabilityPlan"/>
                            <rdf:Description rdf:about="https://w3id.org/rains#OperationStageAccountabilityPlan"/>
                            <rdf:Description rdf:about="https://w3id.org/rains#RuntimeAccountabilityPlan"/>
                        </owl:unionOf>
                    </owl:Class>
                </owl:allValuesFrom>
            </owl:Restriction>
        </rdfs:subClassOf>
        <owl:disjointWith rdf:resource="https://w3id.org/rains#ModelOutput"/>
        <owl:disjointWith rdf:resource="https://w3id.org/rains#OverrideResult"/>
        <rdfs:comment>A specific type of planned System Output which describes the results of aggregating outputs produced by Model component(s) and/or Supporting Infrastrcuture Component(s).

If the AI System is involved in making decisions/recommendations/actions affecting human users, then it is advisable that the information realization corresponding to the Aggregation Result variable contains the following information elements: Affected Agent.</rdfs:comment>
        <rdfs:label>Aggregation Result</rdfs:label>
    </owl:Class>
    


    <!-- https://w3id.org/rains#ApprovalDecision -->


    <owl:Class rdf:about="https://w3id.org/rains#ApprovalDecision">
        <rdfs:subClassOf rdf:resource="https://w3id.org/rains#HumanDecision"/>
        <rdfs:subClassOf>
            <owl:Restriction>
                <owl:onProperty rdf:resource="https://w3id.org/ep-plan#isElementOfPlan"/>
                <owl:allValuesFrom>
                    <owl:Class>
                        <owl:unionOf rdf:parseType="Collection">
                            <rdf:Description rdf:about="https://w3id.org/rains#DeploymentStageAccountabilityPlan"/>
                            <rdf:Description rdf:about="https://w3id.org/rains#DesignStageAccountabilityPlan"/>
                            <rdf:Description rdf:about="https://w3id.org/rains#ImplementationStageAccountabilityPlan"/>
                            <rdf:Description rdf:about="https://w3id.org/rains#InstallationAccountabilityPlan"/>
                            <rdf:Description rdf:about="https://w3id.org/rains#MaintenanceAccountabilityPlan"/>
                            <rdf:Description rdf:about="https://w3id.org/rains#ManualProductionAccountabilityPlan"/>
                            <rdf:Description rdf:about="https://w3id.org/rains#OperationStageAccountabilityPlan"/>
                            <rdf:Description rdf:about="https://w3id.org/rains#UserTrainingAccountabilityPlan"/>
                        </owl:unionOf>
                    </owl:Class>
                </owl:allValuesFrom>
            </owl:Restriction>
        </rdfs:subClassOf>
        <rdfs:subClassOf>
            <owl:Restriction>
                <owl:onProperty rdf:resource="https://w3id.org/ep-plan#isOutputVariableOf"/>
                <owl:allValuesFrom rdf:resource="https://w3id.org/rains#Decide"/>
            </owl:Restriction>
        </rdfs:subClassOf>
        <rdfs:subClassOf>
            <owl:Restriction>
                <owl:onProperty rdf:resource="https://w3id.org/ep-plan#isVariableOfPlan"/>
                <owl:allValuesFrom>
                    <owl:Class>
                        <owl:unionOf rdf:parseType="Collection">
                            <rdf:Description rdf:about="https://w3id.org/rains#DeploymentStageAccountabilityPlan"/>
                            <rdf:Description rdf:about="https://w3id.org/rains#DesignStageAccountabilityPlan"/>
                            <rdf:Description rdf:about="https://w3id.org/rains#ImplementationStageAccountabilityPlan"/>
                            <rdf:Description rdf:about="https://w3id.org/rains#InstallationAccountabilityPlan"/>
                            <rdf:Description rdf:about="https://w3id.org/rains#MaintenanceAccountabilityPlan"/>
                            <rdf:Description rdf:about="https://w3id.org/rains#ManualProductionAccountabilityPlan"/>
                            <rdf:Description rdf:about="https://w3id.org/rains#OperationStageAccountabilityPlan"/>
                            <rdf:Description rdf:about="https://w3id.org/rains#UserTrainingAccountabilityPlan"/>
                        </owl:unionOf>
                    </owl:Class>
                </owl:allValuesFrom>
            </owl:Restriction>
        </rdfs:subClassOf>
        <rdfs:comment>A specific type of a planned human decision representing approvals and sign offs.</rdfs:comment>
        <rdfs:label>Approval Decision</rdfs:label>
    </owl:Class>
    


    <!-- https://w3id.org/rains#ApproveOutput -->


    <owl:Class rdf:about="https://w3id.org/rains#ApproveOutput">
        <rdfs:subClassOf rdf:resource="https://w3id.org/rains#SystemAction"/>
        <rdfs:subClassOf>
            <owl:Restriction>
                <owl:onProperty rdf:resource="https://w3id.org/ep-plan#hasOutputVariable"/>
                <owl:allValuesFrom rdf:resource="https://w3id.org/rains#SystemOutput"/>
            </owl:Restriction>
        </rdfs:subClassOf>
        <rdfs:subClassOf>
            <owl:Restriction>
                <owl:onProperty rdf:resource="https://w3id.org/ep-plan#isElementOfPlan"/>
                <owl:allValuesFrom>
                    <owl:Class>
                        <owl:unionOf rdf:parseType="Collection">
                            <rdf:Description rdf:about="https://w3id.org/rains#OperationStageAccountabilityPlan"/>
                            <rdf:Description rdf:about="https://w3id.org/rains#RuntimeAccountabilityPlan"/>
                        </owl:unionOf>
                    </owl:Class>
                </owl:allValuesFrom>
            </owl:Restriction>
        </rdfs:subClassOf>
        <rdfs:subClassOf>
            <owl:Restriction>
                <owl:onProperty rdf:resource="https://w3id.org/ep-plan#isStepOfPlan"/>
                <owl:allValuesFrom>
                    <owl:Class>
                        <owl:unionOf rdf:parseType="Collection">
                            <rdf:Description rdf:about="https://w3id.org/rains#OperationStageAccountabilityPlan"/>
                            <rdf:Description rdf:about="https://w3id.org/rains#RuntimeAccountabilityPlan"/>
                        </owl:unionOf>
                    </owl:Class>
                </owl:allValuesFrom>
            </owl:Restriction>
        </rdfs:subClassOf>
        <owl:disjointWith rdf:resource="https://w3id.org/rains#CollectUserFeedback"/>
        <owl:disjointWith rdf:resource="https://w3id.org/rains#Configure"/>
        <owl:disjointWith rdf:resource="https://w3id.org/rains#Consent"/>
        <owl:disjointWith rdf:resource="https://w3id.org/rains#Explain"/>
        <owl:disjointWith rdf:resource="https://w3id.org/rains#GenerateOutput"/>
        <owl:disjointWith rdf:resource="https://w3id.org/rains#Justify"/>
        <owl:disjointWith rdf:resource="https://w3id.org/rains#NotifyUser"/>
        <owl:disjointWith rdf:resource="https://w3id.org/rains#PreprocessInputData"/>
        <owl:disjointWith rdf:resource="https://w3id.org/rains#ProvideSystemInputData"/>
        <owl:disjointWith rdf:resource="https://w3id.org/rains#ReturnOutput"/>
        <owl:disjointWith rdf:resource="https://w3id.org/rains#Validate"/>
        <rdfs:comment>A planned step that has some impact on the output of AI System where a user or a system component approves some output. This step is typically part of the Operation stage (specifically Runtime Stage) and has a member of the class System Output as its expected output. Note that this step is not related to the Decide step (which may have a member of the class Approval Decision as its expected output).</rdfs:comment>
        <rdfs:label>Approve Output</rdfs:label>
    </owl:Class>
    


    <!-- https://w3id.org/rains#AutoConstraint -->


    <owl:Class rdf:about="https://w3id.org/rains#AutoConstraint">
        <rdfs:subClassOf rdf:resource="https://w3id.org/ep-plan#Constraint"/>
        <owl:disjointWith rdf:resource="https://w3id.org/rains#HumanConstraint"/>
        <rdfs:comment>A specific type of planned Constraint that describes a constraint which can be evaluated automatically against corresponding accountability trace. Such constraint would normally link to its implementation (e.g., a SHACL rule) using the  https://w3id.org/ep-plan#hasConstraintImplementation property.</rdfs:comment>
        <rdfs:label>Auto Constraint</rdfs:label>
    </owl:Class>
    


    <!-- https://w3id.org/rains#Bias -->


    <owl:Class rdf:about="https://w3id.org/rains#Bias">
        <rdfs:subClassOf rdf:resource="https://w3id.org/rains#Risk"/>
        <rdfs:comment>A type of :Risk  which records a specific piece of  information detailing a potential inclination or prejudice related to some aspects of :AI_Sytem (e.g., a training dataset containing more data about males when both genders will be considered by the ML model)

If a mitigation strategy is used to abate the bias, then these can be indicated using the property :hasMitigationStrategy. It is advisable that information about the bias before and after mitigation is included.</rdfs:comment>
        <rdfs:label>Bias</rdfs:label>
    </owl:Class>
    


    <!-- https://w3id.org/rains#Certificate -->


    <owl:Class rdf:about="https://w3id.org/rains#Certificate">
        <rdfs:subClassOf rdf:resource="https://w3id.org/sao#InformationElement"/>
        <rdfs:comment>A sao:InformnationElement which records information describing a certificate (e.g. an ISO certificate) that is granted during the implementation (or deployment or use and maintenance) life cycle stages.</rdfs:comment>
        <rdfs:label>Certificate</rdfs:label>
    </owl:Class>
    


    <!-- https://w3id.org/rains#CertificationDecision -->


    <owl:Class rdf:about="https://w3id.org/rains#CertificationDecision">
        <rdfs:subClassOf rdf:resource="https://w3id.org/rains#ComplianceAssuranceDecision"/>
        <rdfs:subClassOf>
            <owl:Restriction>
                <owl:onProperty rdf:resource="https://w3id.org/ep-plan#isElementOfPlan"/>
                <owl:allValuesFrom>
                    <owl:Class>
                        <owl:unionOf rdf:parseType="Collection">
                            <rdf:Description rdf:about="https://w3id.org/rains#DeploymentStageAccountabilityPlan"/>
                            <rdf:Description rdf:about="https://w3id.org/rains#DesignStageAccountabilityPlan"/>
                            <rdf:Description rdf:about="https://w3id.org/rains#ImplementationStageAccountabilityPlan"/>
                            <rdf:Description rdf:about="https://w3id.org/rains#InstallationAccountabilityPlan"/>
                            <rdf:Description rdf:about="https://w3id.org/rains#MaintenanceAccountabilityPlan"/>
                            <rdf:Description rdf:about="https://w3id.org/rains#ManualProductionAccountabilityPlan"/>
                            <rdf:Description rdf:about="https://w3id.org/rains#OperationStageAccountabilityPlan"/>
                            <rdf:Description rdf:about="https://w3id.org/rains#UserTrainingAccountabilityPlan"/>
                        </owl:unionOf>
                    </owl:Class>
                </owl:allValuesFrom>
            </owl:Restriction>
        </rdfs:subClassOf>
        <rdfs:subClassOf>
            <owl:Restriction>
                <owl:onProperty rdf:resource="https://w3id.org/ep-plan#isOutputVariableOf"/>
                <owl:allValuesFrom rdf:resource="https://w3id.org/rains#Decide"/>
            </owl:Restriction>
        </rdfs:subClassOf>
        <rdfs:subClassOf>
            <owl:Restriction>
                <owl:onProperty rdf:resource="https://w3id.org/ep-plan#isVariableOfPlan"/>
                <owl:allValuesFrom>
                    <owl:Class>
                        <owl:unionOf rdf:parseType="Collection">
                            <rdf:Description rdf:about="https://w3id.org/rains#DeploymentStageAccountabilityPlan"/>
                            <rdf:Description rdf:about="https://w3id.org/rains#DesignStageAccountabilityPlan"/>
                            <rdf:Description rdf:about="https://w3id.org/rains#ImplementationStageAccountabilityPlan"/>
                            <rdf:Description rdf:about="https://w3id.org/rains#InstallationAccountabilityPlan"/>
                            <rdf:Description rdf:about="https://w3id.org/rains#MaintenanceAccountabilityPlan"/>
                            <rdf:Description rdf:about="https://w3id.org/rains#ManualProductionAccountabilityPlan"/>
                            <rdf:Description rdf:about="https://w3id.org/rains#OperationStageAccountabilityPlan"/>
                            <rdf:Description rdf:about="https://w3id.org/rains#UserTrainingAccountabilityPlan"/>
                        </owl:unionOf>
                    </owl:Class>
                </owl:allValuesFrom>
            </owl:Restriction>
        </rdfs:subClassOf>
        <rdfs:comment>A specific type of a planned human compliance assurance decision representing certification granting. This is usually done by third parties, but may also be done inhouse to prove that the AI System abides by internal policies.</rdfs:comment>
        <rdfs:label>Certification Decision</rdfs:label>
    </owl:Class>
    


    <!-- https://w3id.org/rains#Change -->


    <owl:Class rdf:about="https://w3id.org/rains#Change">
        <rdfs:subClassOf rdf:resource="https://w3id.org/sao#InformationElement"/>
        <rdfs:comment>A sao:InformnationElement which records information describing the deviation from the Design Specification or a Guideline.</rdfs:comment>
        <rdfs:label>Change</rdfs:label>
    </owl:Class>
    


    <!-- https://w3id.org/rains#ChangeJustification -->


    <owl:Class rdf:about="https://w3id.org/rains#ChangeJustification">
        <rdfs:subClassOf rdf:resource="https://w3id.org/sao#InformationElement"/>
        <rdfs:comment>A sao:InformnationElement which records information describing the justification behind a deviation from the Design Specification or a Guideline, or behind overruling the output of the AI System. For example, the reason behind realizing a dataset other than the one indicated by the Dataset Design Specification was used, or why an evaluation measure was recorded which differed from the one indicated to be expected in an Evaluation Specification, or why a user overrode an AI System&apos;s action/decision/recommendation.</rdfs:comment>
        <rdfs:label>Change Justification</rdfs:label>
    </owl:Class>
    


    <!-- https://w3id.org/rains#ChangeLog -->


    <owl:Class rdf:about="https://w3id.org/rains#ChangeLog">
        <rdfs:subClassOf rdf:resource="https://w3id.org/rains#Log"/>
        <rdfs:subClassOf>
            <owl:Restriction>
                <owl:onProperty rdf:resource="https://w3id.org/ep-plan#isElementOfPlan"/>
                <owl:allValuesFrom>
                    <owl:Class>
                        <owl:unionOf rdf:parseType="Collection">
                            <rdf:Description rdf:about="https://w3id.org/rains#ConfigurationAccountabilityPlan"/>
                            <rdf:Description rdf:about="https://w3id.org/rains#DeploymentStageAccountabilityPlan"/>
                            <rdf:Description rdf:about="https://w3id.org/rains#ImplementationStageAccountabilityPlan"/>
                            <rdf:Description rdf:about="https://w3id.org/rains#InstallationAccountabilityPlan"/>
                            <rdf:Description rdf:about="https://w3id.org/rains#MaintenanceAccountabilityPlan"/>
                            <rdf:Description rdf:about="https://w3id.org/rains#ManualProductionAccountabilityPlan"/>
                            <rdf:Description rdf:about="https://w3id.org/rains#OperationStageAccountabilityPlan"/>
                            <rdf:Description rdf:about="https://w3id.org/rains#RuntimeAccountabilityPlan"/>
                            <rdf:Description rdf:about="https://w3id.org/rains#UserTrainingAccountabilityPlan"/>
                        </owl:unionOf>
                    </owl:Class>
                </owl:allValuesFrom>
            </owl:Restriction>
        </rdfs:subClassOf>
        <rdfs:subClassOf>
            <owl:Restriction>
                <owl:onProperty rdf:resource="https://w3id.org/ep-plan#isOutputVariableOf"/>
                <owl:allValuesFrom>
                    <owl:Class>
                        <owl:unionOf rdf:parseType="Collection">
                            <rdf:Description rdf:about="https://w3id.org/rains#Aggregate"/>
                            <rdf:Description rdf:about="https://w3id.org/rains#Configure"/>
                            <rdf:Description rdf:about="https://w3id.org/rains#Evaluate"/>
                            <rdf:Description rdf:about="https://w3id.org/rains#GenerateGuideline"/>
                            <rdf:Description rdf:about="https://w3id.org/rains#Install"/>
                            <rdf:Description rdf:about="https://w3id.org/rains#Justify"/>
                            <rdf:Description rdf:about="https://w3id.org/rains#MergeAndSplitDataset"/>
                            <rdf:Description rdf:about="https://w3id.org/rains#Override"/>
                            <rdf:Description rdf:about="https://w3id.org/rains#RealizeComponent"/>
                            <rdf:Description rdf:about="https://w3id.org/rains#TrainUser"/>
                        </owl:unionOf>
                    </owl:Class>
                </owl:allValuesFrom>
            </owl:Restriction>
        </rdfs:subClassOf>
        <rdfs:subClassOf>
            <owl:Restriction>
                <owl:onProperty rdf:resource="https://w3id.org/ep-plan#isVariableOfPlan"/>
                <owl:allValuesFrom>
                    <owl:Class>
                        <owl:unionOf rdf:parseType="Collection">
                            <rdf:Description rdf:about="https://w3id.org/rains#ConfigurationAccountabilityPlan"/>
                            <rdf:Description rdf:about="https://w3id.org/rains#DeploymentStageAccountabilityPlan"/>
                            <rdf:Description rdf:about="https://w3id.org/rains#ImplementationStageAccountabilityPlan"/>
                            <rdf:Description rdf:about="https://w3id.org/rains#InstallationAccountabilityPlan"/>
                            <rdf:Description rdf:about="https://w3id.org/rains#MaintenanceAccountabilityPlan"/>
                            <rdf:Description rdf:about="https://w3id.org/rains#ManualProductionAccountabilityPlan"/>
                            <rdf:Description rdf:about="https://w3id.org/rains#OperationStageAccountabilityPlan"/>
                            <rdf:Description rdf:about="https://w3id.org/rains#RuntimeAccountabilityPlan"/>
                            <rdf:Description rdf:about="https://w3id.org/rains#UserTrainingAccountabilityPlan"/>
                        </owl:unionOf>
                    </owl:Class>
                </owl:allValuesFrom>
            </owl:Restriction>
        </rdfs:subClassOf>
        <owl:disjointWith rdf:resource="https://w3id.org/rains#InstallationLog"/>
        <rdfs:comment>A specific type of planned Log that describes any change from a design specification or guideline or suggested action/recommendation/decision by the AI system. It is expected to be the result of any accountable action that has an input a design specification or a guideline or specified expected outcome.

It is advisable that the information realization corresponding to the Change Log contains the following information elements:
1.  Change
2. ChangeJustification.</rdfs:comment>
        <rdfs:label>Change Log</rdfs:label>
    </owl:Class>
    


    <!-- https://w3id.org/rains#CollectUserFeedback -->


    <owl:Class rdf:about="https://w3id.org/rains#CollectUserFeedback">
        <rdfs:subClassOf rdf:resource="https://w3id.org/rains#SystemAction"/>
        <rdfs:subClassOf>
            <owl:Restriction>
                <owl:onProperty rdf:resource="https://w3id.org/ep-plan#hasOutputVariable"/>
                <owl:allValuesFrom rdf:resource="https://w3id.org/rains#UserReview"/>
            </owl:Restriction>
        </rdfs:subClassOf>
        <rdfs:subClassOf>
            <owl:Restriction>
                <owl:onProperty rdf:resource="https://w3id.org/ep-plan#isElementOfPlan"/>
                <owl:allValuesFrom>
                    <owl:Class>
                        <owl:unionOf rdf:parseType="Collection">
                            <rdf:Description rdf:about="https://w3id.org/rains#OperationStageAccountabilityPlan"/>
                            <rdf:Description rdf:about="https://w3id.org/rains#RuntimeAccountabilityPlan"/>
                        </owl:unionOf>
                    </owl:Class>
                </owl:allValuesFrom>
            </owl:Restriction>
        </rdfs:subClassOf>
        <rdfs:subClassOf>
            <owl:Restriction>
                <owl:onProperty rdf:resource="https://w3id.org/ep-plan#isStepOfPlan"/>
                <owl:allValuesFrom>
                    <owl:Class>
                        <owl:unionOf rdf:parseType="Collection">
                            <rdf:Description rdf:about="https://w3id.org/rains#OperationStageAccountabilityPlan"/>
                            <rdf:Description rdf:about="https://w3id.org/rains#RuntimeAccountabilityPlan"/>
                        </owl:unionOf>
                    </owl:Class>
                </owl:allValuesFrom>
            </owl:Restriction>
        </rdfs:subClassOf>
        <owl:disjointWith rdf:resource="https://w3id.org/rains#Configure"/>
        <owl:disjointWith rdf:resource="https://w3id.org/rains#Consent"/>
        <owl:disjointWith rdf:resource="https://w3id.org/rains#Explain"/>
        <owl:disjointWith rdf:resource="https://w3id.org/rains#GenerateOutput"/>
        <owl:disjointWith rdf:resource="https://w3id.org/rains#Justify"/>
        <owl:disjointWith rdf:resource="https://w3id.org/rains#NotifyUser"/>
        <owl:disjointWith rdf:resource="https://w3id.org/rains#PreprocessInputData"/>
        <owl:disjointWith rdf:resource="https://w3id.org/rains#ProvideSystemInputData"/>
        <owl:disjointWith rdf:resource="https://w3id.org/rains#ReturnOutput"/>
        <owl:disjointWith rdf:resource="https://w3id.org/rains#Validate"/>
        <rdfs:comment>A planned step that describes receiving a feedback or review from the user of the AI system based on the final system output. (While this is a subclass of System Action, defined as a step that has some impact on some component or output of the AI System, in the current scope of RAInS, the user feedback is not fed back to the AI System. This step is typically part of the Operation stage (specifically Runtime Stage) and has a member of the class User Review as its expected output.</rdfs:comment>
        <rdfs:label>Collect User Feedback</rdfs:label>
    </owl:Class>
    


    <!-- https://w3id.org/rains#ComplianceAssuranceDecision -->


    <owl:Class rdf:about="https://w3id.org/rains#ComplianceAssuranceDecision">
        <rdfs:subClassOf rdf:resource="https://w3id.org/rains#HumanDecision"/>
        <rdfs:subClassOf>
            <owl:Restriction>
                <owl:onProperty rdf:resource="https://w3id.org/ep-plan#isElementOfPlan"/>
                <owl:allValuesFrom>
                    <owl:Class>
                        <owl:unionOf rdf:parseType="Collection">
                            <rdf:Description rdf:about="https://w3id.org/rains#DeploymentStageAccountabilityPlan"/>
                            <rdf:Description rdf:about="https://w3id.org/rains#DesignStageAccountabilityPlan"/>
                            <rdf:Description rdf:about="https://w3id.org/rains#ImplementationStageAccountabilityPlan"/>
                            <rdf:Description rdf:about="https://w3id.org/rains#InstallationAccountabilityPlan"/>
                            <rdf:Description rdf:about="https://w3id.org/rains#MaintenanceAccountabilityPlan"/>
                            <rdf:Description rdf:about="https://w3id.org/rains#ManualProductionAccountabilityPlan"/>
                            <rdf:Description rdf:about="https://w3id.org/rains#OperationStageAccountabilityPlan"/>
                            <rdf:Description rdf:about="https://w3id.org/rains#UserTrainingAccountabilityPlan"/>
                        </owl:unionOf>
                    </owl:Class>
                </owl:allValuesFrom>
            </owl:Restriction>
        </rdfs:subClassOf>
        <rdfs:subClassOf>
            <owl:Restriction>
                <owl:onProperty rdf:resource="https://w3id.org/ep-plan#isOutputVariableOf"/>
                <owl:allValuesFrom rdf:resource="https://w3id.org/rains#Decide"/>
            </owl:Restriction>
        </rdfs:subClassOf>
        <rdfs:subClassOf>
            <owl:Restriction>
                <owl:onProperty rdf:resource="https://w3id.org/ep-plan#isVariableOfPlan"/>
                <owl:allValuesFrom>
                    <owl:Class>
                        <owl:unionOf rdf:parseType="Collection">
                            <rdf:Description rdf:about="https://w3id.org/rains#DeploymentStageAccountabilityPlan"/>
                            <rdf:Description rdf:about="https://w3id.org/rains#DesignStageAccountabilityPlan"/>
                            <rdf:Description rdf:about="https://w3id.org/rains#ImplementationStageAccountabilityPlan"/>
                            <rdf:Description rdf:about="https://w3id.org/rains#InstallationAccountabilityPlan"/>
                            <rdf:Description rdf:about="https://w3id.org/rains#MaintenanceAccountabilityPlan"/>
                            <rdf:Description rdf:about="https://w3id.org/rains#ManualProductionAccountabilityPlan"/>
                            <rdf:Description rdf:about="https://w3id.org/rains#OperationStageAccountabilityPlan"/>
                            <rdf:Description rdf:about="https://w3id.org/rains#UserTrainingAccountabilityPlan"/>
                        </owl:unionOf>
                    </owl:Class>
                </owl:allValuesFrom>
            </owl:Restriction>
        </rdfs:subClassOf>
        <rdfs:comment>A specific type of a planned human decision representing confirmation of compliance of some sao:AccountableResult (e.g., a model specification) with its compliance requirements.</rdfs:comment>
        <rdfs:label>Compliance Assurance Decision</rdfs:label>
    </owl:Class>
    


    <!-- https://w3id.org/rains#ComplianceEntity -->


    <owl:Class rdf:about="https://w3id.org/rains#ComplianceEntity">
        <rdfs:subClassOf rdf:resource="https://w3id.org/sao#InformationElement"/>
        <rdfs:comment>A specific type of sao:InformationElement which records a specific piece of  information about  a compliance requirement that is to be complied with as part of an information realization collection.</rdfs:comment>
        <rdfs:label>Compliance Entity</rdfs:label>
    </owl:Class>
    


    <!-- https://w3id.org/rains#ComplianceSpecification -->


    <owl:Class rdf:about="https://w3id.org/rains#ComplianceSpecification">
        <rdfs:subClassOf rdf:resource="https://w3id.org/rains#DesignSpecification"/>
        <rdfs:subClassOf>
            <owl:Restriction>
                <owl:onProperty rdf:resource="https://w3id.org/ep-plan#isElementOfPlan"/>
                <owl:allValuesFrom>
                    <owl:Class>
                        <owl:unionOf rdf:parseType="Collection">
                            <rdf:Description rdf:about="https://w3id.org/rains#DesignStageAccountabilityPlan"/>
                            <rdf:Description rdf:about="https://w3id.org/rains#ImplementationStageAccountabilityPlan"/>
                            <rdf:Description rdf:about="https://w3id.org/rains#InstallationAccountabilityPlan"/>
                            <rdf:Description rdf:about="https://w3id.org/rains#MaintenanceAccountabilityPlan"/>
                            <rdf:Description rdf:about="https://w3id.org/rains#ManualProductionAccountabilityPlan"/>
                            <rdf:Description rdf:about="https://w3id.org/rains#OperationStageAccountabilityPlan"/>
                            <rdf:Description rdf:about="https://w3id.org/rains#UserTrainingAccountabilityPlan"/>
                        </owl:unionOf>
                    </owl:Class>
                </owl:allValuesFrom>
            </owl:Restriction>
        </rdfs:subClassOf>
        <rdfs:subClassOf>
            <owl:Restriction>
                <owl:onProperty rdf:resource="https://w3id.org/ep-plan#isOutputVariableOf"/>
                <owl:allValuesFrom rdf:resource="https://w3id.org/rains#ProduceSpecification"/>
            </owl:Restriction>
        </rdfs:subClassOf>
        <rdfs:subClassOf>
            <owl:Restriction>
                <owl:onProperty rdf:resource="https://w3id.org/ep-plan#isVariableOfPlan"/>
                <owl:allValuesFrom>
                    <owl:Class>
                        <owl:unionOf rdf:parseType="Collection">
                            <rdf:Description rdf:about="https://w3id.org/rains#DesignStageAccountabilityPlan"/>
                            <rdf:Description rdf:about="https://w3id.org/rains#ImplementationStageAccountabilityPlan"/>
                            <rdf:Description rdf:about="https://w3id.org/rains#InstallationAccountabilityPlan"/>
                            <rdf:Description rdf:about="https://w3id.org/rains#MaintenanceAccountabilityPlan"/>
                            <rdf:Description rdf:about="https://w3id.org/rains#ManualProductionAccountabilityPlan"/>
                            <rdf:Description rdf:about="https://w3id.org/rains#OperationStageAccountabilityPlan"/>
                            <rdf:Description rdf:about="https://w3id.org/rains#UserTrainingAccountabilityPlan"/>
                        </owl:unionOf>
                    </owl:Class>
                </owl:allValuesFrom>
            </owl:Restriction>
        </rdfs:subClassOf>
        <owl:disjointWith rdf:resource="https://w3id.org/rains#DatasetSpecification"/>
        <owl:disjointWith rdf:resource="https://w3id.org/rains#EvaluationSpecification"/>
        <owl:disjointWith rdf:resource="https://w3id.org/rains#ModelSpecification"/>
        <owl:disjointWith rdf:resource="https://w3id.org/rains#SupportingInfrastructureSpecification"/>
        <owl:disjointWith rdf:resource="https://w3id.org/rains#SystemPurposeSpecification"/>
        <rdfs:comment>A specific type of design specification  which represents the  description of a compliance requirement.

It is advisable that the information realization corresponding to SystemPurposeSpecification contains the following information elements
1. HardLaw
2. SoftLaw</rdfs:comment>
        <rdfs:label>Compliance Specification</rdfs:label>
    </owl:Class>
    


    <!-- https://w3id.org/rains#ConfigurationAccountabilityPlan -->


    <owl:Class rdf:about="https://w3id.org/rains#ConfigurationAccountabilityPlan">
        <rdfs:subClassOf rdf:resource="https://w3id.org/rains#OperationStageAccountabilityPlan"/>
        <rdfs:comment>A plan that identifies sao:AccountableAction(s) and sao:AccountableResult(s) relevant to configuring the system as part of the operation stage of an AI system and  which are required to be documented for accountability purposes. This plan is a subplan of the Operation Stage Accountability Plan. The Accountable Actions that can be done at this stage are: Notify User, Consent, Provide System Input Data, Preprocess Input Data, Validate, Configure, Generate Model Output, Explain, and Generate Output</rdfs:comment>
        <rdfs:label>Configuration Accountability Plan</rdfs:label>
    </owl:Class>
    


    <!-- https://w3id.org/rains#ConfigurationData -->


    <owl:Class rdf:about="https://w3id.org/rains#ConfigurationData">
        <rdfs:subClassOf rdf:resource="https://w3id.org/rains#SystemData"/>
        <rdfs:subClassOf>
            <owl:Restriction>
                <owl:onProperty rdf:resource="https://w3id.org/ep-plan#isElementOfPlan"/>
                <owl:allValuesFrom>
                    <owl:Class>
                        <owl:unionOf rdf:parseType="Collection">
                            <rdf:Description rdf:about="https://w3id.org/rains#ConfigurationAccountabilityPlan"/>
                            <rdf:Description rdf:about="https://w3id.org/rains#DeploymentStageAccountabilityPlan"/>
                            <rdf:Description rdf:about="https://w3id.org/rains#InstallationAccountabilityPlan"/>
                            <rdf:Description rdf:about="https://w3id.org/rains#OperationStageAccountabilityPlan"/>
                        </owl:unionOf>
                    </owl:Class>
                </owl:allValuesFrom>
            </owl:Restriction>
        </rdfs:subClassOf>
        <rdfs:subClassOf>
            <owl:Restriction>
                <owl:onProperty rdf:resource="https://w3id.org/ep-plan#isOutputVariableOf"/>
                <owl:allValuesFrom>
                    <owl:Class>
                        <owl:unionOf rdf:parseType="Collection">
                            <rdf:Description rdf:about="https://w3id.org/rains#PreprocessInputData"/>
                            <rdf:Description rdf:about="https://w3id.org/rains#ProvideSystemInputData"/>
                        </owl:unionOf>
                    </owl:Class>
                </owl:allValuesFrom>
            </owl:Restriction>
        </rdfs:subClassOf>
        <rdfs:subClassOf>
            <owl:Restriction>
                <owl:onProperty rdf:resource="https://w3id.org/ep-plan#isVariableOfPlan"/>
                <owl:allValuesFrom>
                    <owl:Class>
                        <owl:unionOf rdf:parseType="Collection">
                            <rdf:Description rdf:about="https://w3id.org/rains#ConfigurationAccountabilityPlan"/>
                            <rdf:Description rdf:about="https://w3id.org/rains#DeploymentStageAccountabilityPlan"/>
                            <rdf:Description rdf:about="https://w3id.org/rains#InstallationAccountabilityPlan"/>
                            <rdf:Description rdf:about="https://w3id.org/rains#OperationStageAccountabilityPlan"/>
                        </owl:unionOf>
                    </owl:Class>
                </owl:allValuesFrom>
            </owl:Restriction>
        </rdfs:subClassOf>
        <owl:disjointWith rdf:resource="https://w3id.org/rains#Explanation"/>
        <owl:disjointWith rdf:resource="https://w3id.org/rains#Notification"/>
        <owl:disjointWith rdf:resource="https://w3id.org/rains#RuntimeInputData"/>
        <owl:disjointWith rdf:resource="https://w3id.org/rains#SystemOutput"/>
        <owl:disjointWith rdf:resource="https://w3id.org/rains#UserConsent"/>
        <owl:disjointWith rdf:resource="https://w3id.org/rains#UserReview"/>
        <owl:disjointWith rdf:resource="https://w3id.org/rains#Validation"/>
        <rdfs:comment>A specific type of planned System Data which represents the data used to configure the AI System, either during the Operation stage or after the system has been installed during the Deployment Stage. For example, in a facial recognition AI system, the configuration data may be the WiFi password or a picture of the user. 

It is advisable that the information realization corresponding to the Configuration Data variable contains the following information elements:
1. Data Item
2. DataCollectionProcedure
3. DataPreprocesingProcedure.
4. Affected Agent if the AI System is involved in making decisions/recommendations/actions affecting human users and the configuration data can be linked to the affected human (e.g. in a facial recognition AI System, the Affected Agent is also the user who configured the AI System to recognise their face).</rdfs:comment>
        <rdfs:label>Configuration Data</rdfs:label>
    </owl:Class>
    


    <!-- https://w3id.org/rains#Configure -->


    <owl:Class rdf:about="https://w3id.org/rains#Configure">
        <rdfs:subClassOf rdf:resource="https://w3id.org/rains#SystemAction"/>
        <rdfs:subClassOf>
            <owl:Restriction>
                <owl:onProperty rdf:resource="https://w3id.org/ep-plan#hasOutputVariable"/>
                <owl:allValuesFrom>
                    <owl:Class>
                        <owl:unionOf rdf:parseType="Collection">
                            <rdf:Description rdf:about="https://w3id.org/rains#ChangeLog"/>
                            <rdf:Description rdf:about="https://w3id.org/rains#ModelComponent"/>
                            <rdf:Description rdf:about="https://w3id.org/rains#SupportingInfrastructureComponent"/>
                        </owl:unionOf>
                    </owl:Class>
                </owl:allValuesFrom>
            </owl:Restriction>
        </rdfs:subClassOf>
        <rdfs:subClassOf>
            <owl:Restriction>
                <owl:onProperty rdf:resource="https://w3id.org/ep-plan#isElementOfPlan"/>
                <owl:allValuesFrom>
                    <owl:Class>
                        <owl:unionOf rdf:parseType="Collection">
                            <rdf:Description rdf:about="https://w3id.org/rains#ConfigurationAccountabilityPlan"/>
                            <rdf:Description rdf:about="https://w3id.org/rains#DeploymentStageAccountabilityPlan"/>
                            <rdf:Description rdf:about="https://w3id.org/rains#InstallationAccountabilityPlan"/>
                            <rdf:Description rdf:about="https://w3id.org/rains#OperationStageAccountabilityPlan"/>
                        </owl:unionOf>
                    </owl:Class>
                </owl:allValuesFrom>
            </owl:Restriction>
        </rdfs:subClassOf>
        <rdfs:subClassOf>
            <owl:Restriction>
                <owl:onProperty rdf:resource="https://w3id.org/ep-plan#isStepOfPlan"/>
                <owl:allValuesFrom>
                    <owl:Class>
                        <owl:unionOf rdf:parseType="Collection">
                            <rdf:Description rdf:about="https://w3id.org/rains#ConfigurationAccountabilityPlan"/>
                            <rdf:Description rdf:about="https://w3id.org/rains#DeploymentStageAccountabilityPlan"/>
                            <rdf:Description rdf:about="https://w3id.org/rains#InstallationAccountabilityPlan"/>
                            <rdf:Description rdf:about="https://w3id.org/rains#OperationStageAccountabilityPlan"/>
                        </owl:unionOf>
                    </owl:Class>
                </owl:allValuesFrom>
            </owl:Restriction>
        </rdfs:subClassOf>
        <owl:disjointWith rdf:resource="https://w3id.org/rains#Consent"/>
        <owl:disjointWith rdf:resource="https://w3id.org/rains#Explain"/>
        <owl:disjointWith rdf:resource="https://w3id.org/rains#GenerateOutput"/>
        <owl:disjointWith rdf:resource="https://w3id.org/rains#Justify"/>
        <owl:disjointWith rdf:resource="https://w3id.org/rains#NotifyUser"/>
        <owl:disjointWith rdf:resource="https://w3id.org/rains#PreprocessInputData"/>
        <owl:disjointWith rdf:resource="https://w3id.org/rains#ProvideSystemInputData"/>
        <owl:disjointWith rdf:resource="https://w3id.org/rains#ReturnOutput"/>
        <owl:disjointWith rdf:resource="https://w3id.org/rains#Validate"/>
        <rdfs:comment>A planned step describing how the AI system is configured during the Deployment or Operation stage of the life cycle (specifically, the Installation or Configuration stages). If this step is done during the Deployment stage, it needs to be done after the system has been installed. This step has members of the classes Model Component and Supporting Infrastructure Component as its expected outputs.  If a deviation from the guidelines takes place, then the step will also have as an output a member of the class Change Log.</rdfs:comment>
        <rdfs:label>Configure</rdfs:label>
    </owl:Class>
    


    <!-- https://w3id.org/rains#Consent -->


    <owl:Class rdf:about="https://w3id.org/rains#Consent">
        <rdfs:subClassOf rdf:resource="https://w3id.org/rains#SystemAction"/>
        <rdfs:subClassOf>
            <owl:Restriction>
                <owl:onProperty rdf:resource="https://w3id.org/ep-plan#hasOutputVariable"/>
                <owl:allValuesFrom rdf:resource="https://w3id.org/rains#UserConsent"/>
            </owl:Restriction>
        </rdfs:subClassOf>
        <rdfs:subClassOf>
            <owl:Restriction>
                <owl:onProperty rdf:resource="https://w3id.org/ep-plan#isElementOfPlan"/>
                <owl:allValuesFrom>
                    <owl:Class>
                        <owl:unionOf rdf:parseType="Collection">
                            <rdf:Description rdf:about="https://w3id.org/rains#ConfigurationAccountabilityPlan"/>
                            <rdf:Description rdf:about="https://w3id.org/rains#OperationStageAccountabilityPlan"/>
                            <rdf:Description rdf:about="https://w3id.org/rains#RuntimeAccountabilityPlan"/>
                        </owl:unionOf>
                    </owl:Class>
                </owl:allValuesFrom>
            </owl:Restriction>
        </rdfs:subClassOf>
        <rdfs:subClassOf>
            <owl:Restriction>
                <owl:onProperty rdf:resource="https://w3id.org/ep-plan#isStepOfPlan"/>
                <owl:allValuesFrom>
                    <owl:Class>
                        <owl:unionOf rdf:parseType="Collection">
                            <rdf:Description rdf:about="https://w3id.org/rains#ConfigurationAccountabilityPlan"/>
                            <rdf:Description rdf:about="https://w3id.org/rains#OperationStageAccountabilityPlan"/>
                            <rdf:Description rdf:about="https://w3id.org/rains#RuntimeAccountabilityPlan"/>
                        </owl:unionOf>
                    </owl:Class>
                </owl:allValuesFrom>
            </owl:Restriction>
        </rdfs:subClassOf>
        <owl:disjointWith rdf:resource="https://w3id.org/rains#Explain"/>
        <owl:disjointWith rdf:resource="https://w3id.org/rains#GenerateOutput"/>
        <owl:disjointWith rdf:resource="https://w3id.org/rains#Justify"/>
        <owl:disjointWith rdf:resource="https://w3id.org/rains#NotifyUser"/>
        <owl:disjointWith rdf:resource="https://w3id.org/rains#PreprocessInputData"/>
        <owl:disjointWith rdf:resource="https://w3id.org/rains#ProvideSystemInputData"/>
        <owl:disjointWith rdf:resource="https://w3id.org/rains#ReturnOutput"/>
        <owl:disjointWith rdf:resource="https://w3id.org/rains#Validate"/>
        <rdfs:comment>A planned step that records a user&apos;s consent to using the AI system. This step is typically part of the Operation stage (specifically Configuration or Runtime stages) and has a member of the class User Consent as its expected output.</rdfs:comment>
        <rdfs:label>Consent</rdfs:label>
    </owl:Class>
    


    <!-- https://w3id.org/rains#DataCollectionProcedure -->


    <owl:Class rdf:about="https://w3id.org/rains#DataCollectionProcedure">
        <rdfs:subClassOf rdf:resource="https://w3id.org/sao#InformationElement"/>
        <rdfs:comment>A specific type of sao:InformationElement which records a specific piece of  information detailing how the data is collected. This includes the information about mechanism used for collecting data (e.g. hardware sensors, software program, or manually), the timeframe over which the data was collected, any consent reporting, etc. 

There is a separate concept that represents the data collection software see rainsDataCollectionSoftware.</rdfs:comment>
        <rdfs:label>Data Collection Procedure</rdfs:label>
    </owl:Class>
    


    <!-- https://w3id.org/rains#DataCollectionSoftware -->


    <owl:Class rdf:about="https://w3id.org/rains#DataCollectionSoftware">
        <rdfs:subClassOf rdf:resource="http://ontosoft.org/software#Software"/>
        <rdfs:comment>A sao:InformationElement (which is also an osw:Software and a prov:SoftwareAgent)  which records  information detailing  a software that was used to collect data that formed the dataset which was used to train the ML Model</rdfs:comment>
        <rdfs:label>Data Collection Software</rdfs:label>
    </owl:Class>
    


    <!-- https://w3id.org/rains#DataItem -->


    <owl:Class rdf:about="https://w3id.org/rains#DataItem">
        <rdfs:subClassOf rdf:resource="https://w3id.org/sao#InformationElement"/>
        <rdfs:comment>A sao:InformnationElement which records information describing a piece of data, e.g. user&apos;s picture or user&apos;s passcode as part of the Configuration Data or Runtime Input Data of a facial recognition AI System.</rdfs:comment>
        <rdfs:label>Data Item</rdfs:label>
    </owl:Class>
    


    <!-- https://w3id.org/rains#DataPreprocessingProcedure -->


    <owl:Class rdf:about="https://w3id.org/rains#DataPreprocessingProcedure">
        <rdfs:subClassOf rdf:resource="https://w3id.org/sao#InformationElement"/>
        <rdfs:comment>A specific type of sao:InformationElement which records a specific piece of  information detailing how the data is preprocessed. This includes information on what is done to the data (e.g., cleaning, sampling, filtering, feature engineering, etc) and how it is done (e.g., manually, programmatically, or using feature engineering software).

There is a separate concept that represents the data preprocessing software.</rdfs:comment>
        <rdfs:label>Data Preprocessing Procedure</rdfs:label>
    </owl:Class>
    


    <!-- https://w3id.org/rains#DataPreprocessingSoftware -->


    <owl:Class rdf:about="https://w3id.org/rains#DataPreprocessingSoftware">
        <rdfs:subClassOf rdf:resource="http://ontosoft.org/software#Software"/>
        <rdfs:comment>A sao:InformationElement (which is also an osw:Software and a prov:SoftwareAgent)  which records  information detailing  a software  that was used to preprocess the dataset using to train the ML Model</rdfs:comment>
        <rdfs:label>Data Preprocessing Software</rdfs:label>
    </owl:Class>
    


    <!-- https://w3id.org/rains#DatasetComponent -->


    <owl:Class rdf:about="https://w3id.org/rains#DatasetComponent">
        <rdfs:subClassOf rdf:resource="https://w3id.org/sao#AccountableResult"/>
        <rdfs:subClassOf>
            <owl:Restriction>
                <owl:onProperty rdf:resource="https://w3id.org/ep-plan#isElementOfPlan"/>
                <owl:allValuesFrom>
                    <owl:Class>
                        <owl:unionOf rdf:parseType="Collection">
                            <rdf:Description rdf:about="https://w3id.org/rains#DeploymentStageAccountabilityPlan"/>
                            <rdf:Description rdf:about="https://w3id.org/rains#ImplementationStageAccountabilityPlan"/>
                            <rdf:Description rdf:about="https://w3id.org/rains#InstallationAccountabilityPlan"/>
                            <rdf:Description rdf:about="https://w3id.org/rains#MaintenanceAccountabilityPlan"/>
                            <rdf:Description rdf:about="https://w3id.org/rains#RuntimeAccountabilityPlan"/>
                        </owl:unionOf>
                    </owl:Class>
                </owl:allValuesFrom>
            </owl:Restriction>
        </rdfs:subClassOf>
        <rdfs:subClassOf>
            <owl:Restriction>
                <owl:onProperty rdf:resource="https://w3id.org/ep-plan#isOutputVariableOf"/>
                <owl:allValuesFrom>
                    <owl:Class>
                        <owl:unionOf rdf:parseType="Collection">
                            <rdf:Description rdf:about="https://w3id.org/rains#MergeAndSplitDataset"/>
                            <rdf:Description rdf:about="https://w3id.org/rains#RealizeComponent"/>
                        </owl:unionOf>
                    </owl:Class>
                </owl:allValuesFrom>
            </owl:Restriction>
        </rdfs:subClassOf>
        <rdfs:subClassOf>
            <owl:Restriction>
                <owl:onProperty rdf:resource="https://w3id.org/ep-plan#isVariableOfPlan"/>
                <owl:allValuesFrom>
                    <owl:Class>
                        <owl:unionOf rdf:parseType="Collection">
                            <rdf:Description rdf:about="https://w3id.org/rains#DeploymentStageAccountabilityPlan"/>
                            <rdf:Description rdf:about="https://w3id.org/rains#ImplementationStageAccountabilityPlan"/>
                            <rdf:Description rdf:about="https://w3id.org/rains#InstallationAccountabilityPlan"/>
                            <rdf:Description rdf:about="https://w3id.org/rains#MaintenanceAccountabilityPlan"/>
                            <rdf:Description rdf:about="https://w3id.org/rains#RuntimeAccountabilityPlan"/>
                        </owl:unionOf>
                    </owl:Class>
                </owl:allValuesFrom>
            </owl:Restriction>
        </rdfs:subClassOf>
        <owl:disjointWith rdf:resource="https://w3id.org/rains#DesignSpecification"/>
        <owl:disjointWith rdf:resource="https://w3id.org/rains#Guideline"/>
        <owl:disjointWith rdf:resource="https://w3id.org/rains#HumanDecision"/>
        <owl:disjointWith rdf:resource="https://w3id.org/rains#Log"/>
        <owl:disjointWith rdf:resource="https://w3id.org/rains#SupportingInfrastructureComponent"/>
        <owl:disjointWith rdf:resource="https://w3id.org/rains#SystemData"/>
        <owl:disjointWith rdf:resource="https://w3id.org/rains#UserTrainingReport"/>
        <rdfs:comment>A specific type of planned sao:AccountableResult  which represents the description of an realized dataset, including its characteristics, how it was collected, its risks, etc. The dataset component represents a collection of collected and pre-processed data. Once it is split, the subclasses TestingDataset, ValidationDataset, and EvaluationDataset can be used.

It is advisable that the information realization corresponding to the DatasetComponent variable contains the following information elements:
1. Dataset, the realized dataset should be an instance of RealizedObject. If the implementation deviates from the design, then an additional dataset should be indicated as an instance of ExcludedObject.
2. Data Item
3. DatasetCharacteristic
4. DataCollectionProcedure
5. DataPreprocesingProcedure
6. Funding
7. Limitation
8. Risk and its subclass Bias
9. Tradeoff
10. The subclasses of Use Case, namely IncorrectUseCase and IntendedUseCase
11. IntendedUserGroup
12. The subclasses of Compliance Entity, namely, Hard Law and SoftLaw
13. LicenseDocument

It is discouraged that the information realization corresponding to the DatasetComponent variable contains the following information elements:
1. Model
2. SupportingInfrastructure
3. The following subclasses of Realizable Object Characteristic: Algorithm, ModelCharacteristic, SystemAuditMechanism, SystemExplanationMechanism, System Feedback from User Mechanism, System Human Oversight Mechanism, and SystemSecurityMechanism
4. The subclasses of Guidance,namely, System Deployment Guidance, SystemInstallationGuidance, UserTrainingGuidance, SystemOperationGuidance, SystemUsageGuidance, and SystemMaintenanceGuidance
5. NotificationProof</rdfs:comment>
        <rdfs:label>Dataset Component</rdfs:label>
    </owl:Class>
    


    <!-- https://w3id.org/rains#DatasetSpecification -->


    <owl:Class rdf:about="https://w3id.org/rains#DatasetSpecification">
        <rdfs:subClassOf rdf:resource="https://w3id.org/rains#DesignSpecification"/>
        <rdfs:subClassOf>
            <owl:Restriction>
                <owl:onProperty rdf:resource="https://w3id.org/ep-plan#isElementOfPlan"/>
                <owl:allValuesFrom>
                    <owl:Class>
                        <owl:unionOf rdf:parseType="Collection">
                            <rdf:Description rdf:about="https://w3id.org/rains#DeploymentStageAccountabilityPlan"/>
                            <rdf:Description rdf:about="https://w3id.org/rains#DesignStageAccountabilityPlan"/>
                            <rdf:Description rdf:about="https://w3id.org/rains#ImplementationStageAccountabilityPlan"/>
                            <rdf:Description rdf:about="https://w3id.org/rains#InstallationAccountabilityPlan"/>
                            <rdf:Description rdf:about="https://w3id.org/rains#MaintenanceAccountabilityPlan"/>
                            <rdf:Description rdf:about="https://w3id.org/rains#OperationStageAccountabilityPlan"/>
                        </owl:unionOf>
                    </owl:Class>
                </owl:allValuesFrom>
            </owl:Restriction>
        </rdfs:subClassOf>
        <rdfs:subClassOf>
            <owl:Restriction>
                <owl:onProperty rdf:resource="https://w3id.org/ep-plan#isOutputVariableOf"/>
                <owl:allValuesFrom rdf:resource="https://w3id.org/rains#ProduceSpecification"/>
            </owl:Restriction>
        </rdfs:subClassOf>
        <rdfs:subClassOf>
            <owl:Restriction>
                <owl:onProperty rdf:resource="https://w3id.org/ep-plan#isVariableOfPlan"/>
                <owl:allValuesFrom>
                    <owl:Class>
                        <owl:unionOf rdf:parseType="Collection">
                            <rdf:Description rdf:about="https://w3id.org/rains#DeploymentStageAccountabilityPlan"/>
                            <rdf:Description rdf:about="https://w3id.org/rains#DesignStageAccountabilityPlan"/>
                            <rdf:Description rdf:about="https://w3id.org/rains#ImplementationStageAccountabilityPlan"/>
                            <rdf:Description rdf:about="https://w3id.org/rains#InstallationAccountabilityPlan"/>
                            <rdf:Description rdf:about="https://w3id.org/rains#MaintenanceAccountabilityPlan"/>
                            <rdf:Description rdf:about="https://w3id.org/rains#OperationStageAccountabilityPlan"/>
                        </owl:unionOf>
                    </owl:Class>
                </owl:allValuesFrom>
            </owl:Restriction>
        </rdfs:subClassOf>
        <owl:disjointWith rdf:resource="https://w3id.org/rains#SupportingInfrastructureSpecification"/>
        <owl:disjointWith rdf:resource="https://w3id.org/rains#SystemPurposeSpecification"/>
        <rdfs:comment>A specific type of design specification  which represents the description of planned requirements, characteristics, risks, etc. related to a dataset (e.g., a training dataset for ML model) expected to be used as part of the AI system life cycle.

It is advisable that the information realization corresponding to DatasetSpecification contains the following information elements 
1. Dataset 
2. DataItem
3. DatasetCharacteristic
3. DataCollectionProcedure and and if applicable DataCollectionSoftware
4. DataPreprocesingProcedure and if applicable DataPreprocessingSoftware
5. Funding
6. Limitation
7. Risk and its subclass Bias, and if applicable FairnessOrBiasDetectionSoftware
8. Tradeoff
9. IntendedUserGroup
10. The subclasses of Use Case, namely IncorrectUseCase and IntendedUseCase
11. The subclasses of Compliance Entity, namely, Hard Law and SoftLaw
12. LicenseDocument

It is discouraged that the information realization corresponding to the Dataset Specification contains the following information elements:
1. Model
2. SupportingInfrastructure
3. The following subclasses of Realizable Object Characteristic: Algorithm, ModelCharacteristic, SystemAuditMechanism, SystemExplanationMechanism, System Feedback from User Mechanism, System Human Oversight Mechanism, and SystemSecurityMechanism
4. The subclasses of Guidance,namely, System Deployment Guidance, SystemInstallationGuidance, UserTrainingGuidance, SystemOperationGuidance, SystemUsageGuidance, and SystemMaintenanceGuidance
5. NotificationProof</rdfs:comment>
        <rdfs:label>Dataset Specification</rdfs:label>
    </owl:Class>
    


    <!-- https://w3id.org/rains#Decide -->


    <owl:Class rdf:about="https://w3id.org/rains#Decide">
        <rdfs:subClassOf rdf:resource="https://w3id.org/sao#AccountableAction"/>
        <rdfs:subClassOf>
            <owl:Restriction>
                <owl:onProperty rdf:resource="https://w3id.org/ep-plan#hasOutputVariable"/>
                <owl:allValuesFrom>
                    <owl:Class>
                        <owl:unionOf rdf:parseType="Collection">
                            <rdf:Description rdf:about="https://w3id.org/rains#ApprovalDecision"/>
                            <rdf:Description rdf:about="https://w3id.org/rains#CertificationDecision"/>
                            <rdf:Description rdf:about="https://w3id.org/rains#ComplianceAssuranceDecision"/>
                            <rdf:Description rdf:about="https://w3id.org/rains#FitnessConfirmationDecision"/>
                            <rdf:Description rdf:about="https://w3id.org/rains#HumanDecision"/>
                        </owl:unionOf>
                    </owl:Class>
                </owl:allValuesFrom>
            </owl:Restriction>
        </rdfs:subClassOf>
        <rdfs:subClassOf>
            <owl:Restriction>
                <owl:onProperty rdf:resource="https://w3id.org/ep-plan#isElementOfPlan"/>
                <owl:allValuesFrom>
                    <owl:Class>
                        <owl:unionOf rdf:parseType="Collection">
                            <rdf:Description rdf:about="https://w3id.org/rains#DeploymentStageAccountabilityPlan"/>
                            <rdf:Description rdf:about="https://w3id.org/rains#DesignStageAccountabilityPlan"/>
                            <rdf:Description rdf:about="https://w3id.org/rains#ImplementationStageAccountabilityPlan"/>
                            <rdf:Description rdf:about="https://w3id.org/rains#InstallationAccountabilityPlan"/>
                            <rdf:Description rdf:about="https://w3id.org/rains#MaintenanceAccountabilityPlan"/>
                            <rdf:Description rdf:about="https://w3id.org/rains#ManualProductionAccountabilityPlan"/>
                            <rdf:Description rdf:about="https://w3id.org/rains#OperationStageAccountabilityPlan"/>
                            <rdf:Description rdf:about="https://w3id.org/rains#UserTrainingAccountabilityPlan"/>
                        </owl:unionOf>
                    </owl:Class>
                </owl:allValuesFrom>
            </owl:Restriction>
        </rdfs:subClassOf>
        <rdfs:subClassOf>
            <owl:Restriction>
                <owl:onProperty rdf:resource="https://w3id.org/ep-plan#isStepOfPlan"/>
                <owl:allValuesFrom>
                    <owl:Class>
                        <owl:unionOf rdf:parseType="Collection">
                            <rdf:Description rdf:about="https://w3id.org/rains#DeploymentStageAccountabilityPlan"/>
                            <rdf:Description rdf:about="https://w3id.org/rains#DesignStageAccountabilityPlan"/>
                            <rdf:Description rdf:about="https://w3id.org/rains#ImplementationStageAccountabilityPlan"/>
                            <rdf:Description rdf:about="https://w3id.org/rains#InstallationAccountabilityPlan"/>
                            <rdf:Description rdf:about="https://w3id.org/rains#MaintenanceAccountabilityPlan"/>
                            <rdf:Description rdf:about="https://w3id.org/rains#ManualProductionAccountabilityPlan"/>
                            <rdf:Description rdf:about="https://w3id.org/rains#OperationStageAccountabilityPlan"/>
                            <rdf:Description rdf:about="https://w3id.org/rains#UserTrainingAccountabilityPlan"/>
                        </owl:unionOf>
                    </owl:Class>
                </owl:allValuesFrom>
            </owl:Restriction>
        </rdfs:subClassOf>
        <owl:disjointWith rdf:resource="https://w3id.org/rains#Evaluate"/>
        <owl:disjointWith rdf:resource="https://w3id.org/rains#GenerateGuideline"/>
        <owl:disjointWith rdf:resource="https://w3id.org/rains#Install"/>
        <owl:disjointWith rdf:resource="https://w3id.org/rains#MergeAndSplitDataset"/>
        <owl:disjointWith rdf:resource="https://w3id.org/rains#ProduceSpecification"/>
        <owl:disjointWith rdf:resource="https://w3id.org/rains#RealizeComponent"/>
        <owl:disjointWith rdf:resource="https://w3id.org/rains#SystemAction"/>
        <owl:disjointWith rdf:resource="https://w3id.org/rains#TrainUser"/>
        <rdfs:comment>A planned step describing a decision to be taken by a human when incorporating accountability in AI Systems, e.g. approve the design of an ML Model. This step has members of the class Human Decision (and its subclasses) as its expected outputs.</rdfs:comment>
        <rdfs:label>Decide</rdfs:label>
    </owl:Class>
    


    <!-- https://w3id.org/rains#DeploymentStageAccountabilityPlan -->


    <owl:Class rdf:about="https://w3id.org/rains#DeploymentStageAccountabilityPlan">
        <rdfs:subClassOf rdf:resource="https://w3id.org/sao#AccountabilityPlan"/>
        <rdfs:comment>A plan that identifies sao:AccountableAction(s) and sao:AccountableResult(s) relevant to the deployment stage of an AI system and  which are required to be documented for accountability purposes. This plan may be split into one of three sub-plans: Manual Production Accountability Plan, Installation Accountability Plan, and User Training Accountability Plan. The Accountable Actions that can be done at this stage are: Install (subsumes integration and configuration), Generate Guideline, Train User, Evaluate, Decide. If there is additional configuration to be done after the Install action has been performed, then the following Accountable Actions can also be performed at this stage: Provide System Input Data, Preprocess Input Data, Configure, and Validate.</rdfs:comment>
        <rdfs:label>Deployment Stage Accountability Plan</rdfs:label>
    </owl:Class>
    


    <!-- https://w3id.org/rains#DesignSpecification -->


    <owl:Class rdf:about="https://w3id.org/rains#DesignSpecification">
        <rdfs:subClassOf rdf:resource="https://w3id.org/sao#AccountableResult"/>
        <rdfs:subClassOf>
            <owl:Restriction>
                <owl:onProperty rdf:resource="https://w3id.org/ep-plan#isElementOfPlan"/>
                <owl:allValuesFrom>
                    <owl:Class>
                        <owl:unionOf rdf:parseType="Collection">
                            <rdf:Description rdf:about="https://w3id.org/rains#DeploymentStageAccountabilityPlan"/>
                            <rdf:Description rdf:about="https://w3id.org/rains#DesignStageAccountabilityPlan"/>
                            <rdf:Description rdf:about="https://w3id.org/rains#ImplementationStageAccountabilityPlan"/>
                            <rdf:Description rdf:about="https://w3id.org/rains#InstallationAccountabilityPlan"/>
                            <rdf:Description rdf:about="https://w3id.org/rains#MaintenanceAccountabilityPlan"/>
                            <rdf:Description rdf:about="https://w3id.org/rains#ManualProductionAccountabilityPlan"/>
                            <rdf:Description rdf:about="https://w3id.org/rains#OperationStageAccountabilityPlan"/>
                            <rdf:Description rdf:about="https://w3id.org/rains#UserTrainingAccountabilityPlan"/>
                        </owl:unionOf>
                    </owl:Class>
                </owl:allValuesFrom>
            </owl:Restriction>
        </rdfs:subClassOf>
        <rdfs:subClassOf>
            <owl:Restriction>
                <owl:onProperty rdf:resource="https://w3id.org/ep-plan#isOutputVariableOf"/>
                <owl:allValuesFrom rdf:resource="https://w3id.org/rains#ProduceSpecification"/>
            </owl:Restriction>
        </rdfs:subClassOf>
        <rdfs:subClassOf>
            <owl:Restriction>
                <owl:onProperty rdf:resource="https://w3id.org/ep-plan#isVariableOfPlan"/>
                <owl:allValuesFrom>
                    <owl:Class>
                        <owl:unionOf rdf:parseType="Collection">
                            <rdf:Description rdf:about="https://w3id.org/rains#DeploymentStageAccountabilityPlan"/>
                            <rdf:Description rdf:about="https://w3id.org/rains#DesignStageAccountabilityPlan"/>
                            <rdf:Description rdf:about="https://w3id.org/rains#ImplementationStageAccountabilityPlan"/>
                            <rdf:Description rdf:about="https://w3id.org/rains#InstallationAccountabilityPlan"/>
                            <rdf:Description rdf:about="https://w3id.org/rains#MaintenanceAccountabilityPlan"/>
                            <rdf:Description rdf:about="https://w3id.org/rains#ManualProductionAccountabilityPlan"/>
                            <rdf:Description rdf:about="https://w3id.org/rains#OperationStageAccountabilityPlan"/>
                            <rdf:Description rdf:about="https://w3id.org/rains#UserTrainingAccountabilityPlan"/>
                        </owl:unionOf>
                    </owl:Class>
                </owl:allValuesFrom>
            </owl:Restriction>
        </rdfs:subClassOf>
        <owl:disjointWith rdf:resource="https://w3id.org/rains#Evaluation"/>
        <owl:disjointWith rdf:resource="https://w3id.org/rains#Guideline"/>
        <owl:disjointWith rdf:resource="https://w3id.org/rains#HumanDecision"/>
        <owl:disjointWith rdf:resource="https://w3id.org/rains#Log"/>
        <owl:disjointWith rdf:resource="https://w3id.org/rains#ModelComponent"/>
        <owl:disjointWith rdf:resource="https://w3id.org/rains#SupportingInfrastructureComponent"/>
        <owl:disjointWith rdf:resource="https://w3id.org/rains#SystemData"/>
        <owl:disjointWith rdf:resource="https://w3id.org/rains#UserTrainingReport"/>
        <rdfs:comment>A specific type of planned sao:AccountableResult which represents a high level reference to a specification  (e.g. a specification report) that is expected to be produced during the design stage in order to inform the future AI system lifecycle stages (e.g. implementation).</rdfs:comment>
        <rdfs:label>Design Specification</rdfs:label>
    </owl:Class>
    


    <!-- https://w3id.org/rains#DesignStageAccountabilityPlan -->


    <owl:Class rdf:about="https://w3id.org/rains#DesignStageAccountabilityPlan">
        <rdfs:subClassOf rdf:resource="https://w3id.org/sao#AccountabilityPlan"/>
        <rdfs:subClassOf>
            <owl:Restriction>
                <owl:onProperty rdf:resource="https://w3id.org/ep-plan#includesStep"/>
                <owl:allValuesFrom>
                    <owl:Class>
                        <owl:unionOf rdf:parseType="Collection">
                            <rdf:Description rdf:about="https://w3id.org/rains#Decide"/>
                            <rdf:Description rdf:about="https://w3id.org/rains#GrantCertification"/>
                            <rdf:Description rdf:about="https://w3id.org/rains#ProduceSpecification"/>
                        </owl:unionOf>
                    </owl:Class>
                </owl:allValuesFrom>
            </owl:Restriction>
        </rdfs:subClassOf>
        <rdfs:subClassOf>
            <owl:Restriction>
                <owl:onProperty rdf:resource="https://w3id.org/ep-plan#includesVariable"/>
                <owl:allValuesFrom>
                    <owl:Class>
                        <owl:unionOf rdf:parseType="Collection">
                            <rdf:Description rdf:about="https://w3id.org/rains#ApprovalDecision"/>
                            <rdf:Description rdf:about="https://w3id.org/rains#CertificationDecision"/>
                            <rdf:Description rdf:about="https://w3id.org/rains#ComplianceAssuranceDecision"/>
                            <rdf:Description rdf:about="https://w3id.org/rains#ComplianceSpecification"/>
                            <rdf:Description rdf:about="https://w3id.org/rains#DatasetSpecification"/>
                            <rdf:Description rdf:about="https://w3id.org/rains#DesignSpecification"/>
                            <rdf:Description rdf:about="https://w3id.org/rains#EvaluationSpecification"/>
                            <rdf:Description rdf:about="https://w3id.org/rains#FitnessConfirmationDecision"/>
                            <rdf:Description rdf:about="https://w3id.org/rains#HumanDecision"/>
                            <rdf:Description rdf:about="https://w3id.org/rains#ModelSpecification"/>
                            <rdf:Description rdf:about="https://w3id.org/rains#SupportingInfrastructureSpecification"/>
                            <rdf:Description rdf:about="https://w3id.org/rains#SystemPurposeSpecification"/>
                        </owl:unionOf>
                    </owl:Class>
                </owl:allValuesFrom>
            </owl:Restriction>
        </rdfs:subClassOf>
        <rdfs:comment>A plan that identifies sao:AccountableAction(s) and sao:AccountableResult(s) relevant to the design stage of an AI system and  which are required to be documented for accountability purposes. The Accountable Actions that can be done at this stage are: Produce Specification and Decide.</rdfs:comment>
        <rdfs:label>Design Stage Accountability Plan</rdfs:label>
    </owl:Class>
    


    <!-- https://w3id.org/rains#DisclaimerNotification -->


    <owl:Class rdf:about="https://w3id.org/rains#DisclaimerNotification">
        <rdfs:subClassOf rdf:resource="https://w3id.org/rains#Notification"/>
        <rdfs:subClassOf>
            <owl:Restriction>
                <owl:onProperty rdf:resource="https://w3id.org/ep-plan#isElementOfPlan"/>
                <owl:allValuesFrom>
                    <owl:Class>
                        <owl:unionOf rdf:parseType="Collection">
                            <rdf:Description rdf:about="https://w3id.org/rains#ConfigurationAccountabilityPlan"/>
                            <rdf:Description rdf:about="https://w3id.org/rains#OperationStageAccountabilityPlan"/>
                            <rdf:Description rdf:about="https://w3id.org/rains#RuntimeAccountabilityPlan"/>
                        </owl:unionOf>
                    </owl:Class>
                </owl:allValuesFrom>
            </owl:Restriction>
        </rdfs:subClassOf>
        <rdfs:subClassOf>
            <owl:Restriction>
                <owl:onProperty rdf:resource="https://w3id.org/ep-plan#isOutputVariableOf"/>
                <owl:allValuesFrom rdf:resource="https://w3id.org/rains#NotifyUser"/>
            </owl:Restriction>
        </rdfs:subClassOf>
        <rdfs:subClassOf>
            <owl:Restriction>
                <owl:onProperty rdf:resource="https://w3id.org/ep-plan#isVariableOfPlan"/>
                <owl:allValuesFrom>
                    <owl:Class>
                        <owl:unionOf rdf:parseType="Collection">
                            <rdf:Description rdf:about="https://w3id.org/rains#ConfigurationAccountabilityPlan"/>
                            <rdf:Description rdf:about="https://w3id.org/rains#OperationStageAccountabilityPlan"/>
                            <rdf:Description rdf:about="https://w3id.org/rains#RuntimeAccountabilityPlan"/>
                        </owl:unionOf>
                    </owl:Class>
                </owl:allValuesFrom>
            </owl:Restriction>
        </rdfs:subClassOf>
        <rdfs:comment>A specific type of Notification which describes a disclaimer that the user is using or interacting with an AI System.

Similar to Notification, it is advisable that the information realization corresponding to the Disclaimer Notification variable contains the following information elements:
1. Affected Agent, describing the user who was notified.
2. Notification Proof, documenting how the user was notified, e.g. a screenshot of the disclaimer shown to the user.</rdfs:comment>
        <rdfs:label>Disclaimer Notification</rdfs:label>
    </owl:Class>
    


    <!-- https://w3id.org/rains#ErrorNotification -->


    <owl:Class rdf:about="https://w3id.org/rains#ErrorNotification">
        <rdfs:subClassOf rdf:resource="https://w3id.org/rains#Notification"/>
        <rdfs:subClassOf>
            <owl:Restriction>
                <owl:onProperty rdf:resource="https://w3id.org/ep-plan#isElementOfPlan"/>
                <owl:allValuesFrom>
                    <owl:Class>
                        <owl:unionOf rdf:parseType="Collection">
                            <rdf:Description rdf:about="https://w3id.org/rains#ConfigurationAccountabilityPlan"/>
                            <rdf:Description rdf:about="https://w3id.org/rains#DeploymentStageAccountabilityPlan"/>
                            <rdf:Description rdf:about="https://w3id.org/rains#InstallationAccountabilityPlan"/>
                            <rdf:Description rdf:about="https://w3id.org/rains#OperationStageAccountabilityPlan"/>
                            <rdf:Description rdf:about="https://w3id.org/rains#RuntimeAccountabilityPlan"/>
                        </owl:unionOf>
                    </owl:Class>
                </owl:allValuesFrom>
            </owl:Restriction>
        </rdfs:subClassOf>
        <rdfs:subClassOf>
            <owl:Restriction>
                <owl:onProperty rdf:resource="https://w3id.org/ep-plan#isOutputVariableOf"/>
                <owl:allValuesFrom rdf:resource="https://w3id.org/rains#NotifyUser"/>
            </owl:Restriction>
        </rdfs:subClassOf>
        <rdfs:subClassOf>
            <owl:Restriction>
                <owl:onProperty rdf:resource="https://w3id.org/ep-plan#isVariableOfPlan"/>
                <owl:allValuesFrom>
                    <owl:Class>
                        <owl:unionOf rdf:parseType="Collection">
                            <rdf:Description rdf:about="https://w3id.org/rains#ConfigurationAccountabilityPlan"/>
                            <rdf:Description rdf:about="https://w3id.org/rains#DeploymentStageAccountabilityPlan"/>
                            <rdf:Description rdf:about="https://w3id.org/rains#InstallationAccountabilityPlan"/>
                            <rdf:Description rdf:about="https://w3id.org/rains#OperationStageAccountabilityPlan"/>
                            <rdf:Description rdf:about="https://w3id.org/rains#RuntimeAccountabilityPlan"/>
                        </owl:unionOf>
                    </owl:Class>
                </owl:allValuesFrom>
            </owl:Restriction>
        </rdfs:subClassOf>
        <rdfs:comment>A specific type of Notification which represents a notification of an error which has occurred to the user. For example, if the input data could not be validated then this class is used to model the notification of the validation error to the user.

Similar to Notification, it is advisable that the information realization corresponding to the Error Notification variable contains the following information elements:
1. Affected Agent, describing the user who was notified.
2. Notification Proof, documenting how the user was notified, e.g. a screenshot of the error notification shown to the user.</rdfs:comment>
        <rdfs:label>Error Notification</rdfs:label>
    </owl:Class>
    


    <!-- https://w3id.org/rains#Evaluate -->


    <owl:Class rdf:about="https://w3id.org/rains#Evaluate">
        <rdfs:subClassOf rdf:resource="https://w3id.org/sao#AccountableAction"/>
        <rdfs:subClassOf>
            <owl:Restriction>
                <owl:onProperty rdf:resource="https://w3id.org/ep-plan#hasOutputVariable"/>
                <owl:allValuesFrom>
                    <owl:Class>
                        <owl:unionOf rdf:parseType="Collection">
                            <rdf:Description rdf:about="https://w3id.org/rains#ChangeLog"/>
                            <rdf:Description rdf:about="https://w3id.org/rains#Evaluation"/>
                            <rdf:Description rdf:about="https://w3id.org/rains#ThirdPartyEvaluation"/>
                        </owl:unionOf>
                    </owl:Class>
                </owl:allValuesFrom>
            </owl:Restriction>
        </rdfs:subClassOf>
        <rdfs:subClassOf>
            <owl:Restriction>
                <owl:onProperty rdf:resource="https://w3id.org/ep-plan#isElementOfPlan"/>
                <owl:allValuesFrom>
                    <owl:Class>
                        <owl:unionOf rdf:parseType="Collection">
                            <rdf:Description rdf:about="https://w3id.org/rains#DeploymentStageAccountabilityPlan"/>
                            <rdf:Description rdf:about="https://w3id.org/rains#ImplementationStageAccountabilityPlan"/>
                            <rdf:Description rdf:about="https://w3id.org/rains#InstallationAccountabilityPlan"/>
                            <rdf:Description rdf:about="https://w3id.org/rains#MaintenanceAccountabilityPlan"/>
                            <rdf:Description rdf:about="https://w3id.org/rains#OperationStageAccountabilityPlan"/>
                        </owl:unionOf>
                    </owl:Class>
                </owl:allValuesFrom>
            </owl:Restriction>
        </rdfs:subClassOf>
        <rdfs:subClassOf>
            <owl:Restriction>
                <owl:onProperty rdf:resource="https://w3id.org/ep-plan#isStepOfPlan"/>
                <owl:allValuesFrom>
                    <owl:Class>
                        <owl:unionOf rdf:parseType="Collection">
                            <rdf:Description rdf:about="https://w3id.org/rains#DeploymentStageAccountabilityPlan"/>
                            <rdf:Description rdf:about="https://w3id.org/rains#ImplementationStageAccountabilityPlan"/>
                            <rdf:Description rdf:about="https://w3id.org/rains#InstallationAccountabilityPlan"/>
                            <rdf:Description rdf:about="https://w3id.org/rains#MaintenanceAccountabilityPlan"/>
                            <rdf:Description rdf:about="https://w3id.org/rains#OperationStageAccountabilityPlan"/>
                        </owl:unionOf>
                    </owl:Class>
                </owl:allValuesFrom>
            </owl:Restriction>
        </rdfs:subClassOf>
        <owl:disjointWith rdf:resource="https://w3id.org/rains#GenerateGuideline"/>
        <owl:disjointWith rdf:resource="https://w3id.org/rains#Install"/>
        <owl:disjointWith rdf:resource="https://w3id.org/rains#MergeAndSplitDataset"/>
        <owl:disjointWith rdf:resource="https://w3id.org/rains#ProduceSpecification"/>
        <owl:disjointWith rdf:resource="https://w3id.org/rains#RealizeComponent"/>
        <owl:disjointWith rdf:resource="https://w3id.org/rains#SystemAction"/>
        <owl:disjointWith rdf:resource="https://w3id.org/rains#TrainUser"/>
        <rdfs:comment>A planned step describing an evaluation, i.e. testing  and producing evaluation metrics, that has some impact on the AI System, e.g. the evaluation of the ML model using a specified Dataset or the AI System undergoing a third party evaluation. This step has a member of the class Evaluation (or its subclass Third Party Evaluation) its expected output.  If a deviation from the design specification(s) or guideline(s) takes place, then this step will also have as an output a member of the class Change Log.</rdfs:comment>
        <rdfs:label>Evaluate</rdfs:label>
    </owl:Class>
    


    <!-- https://w3id.org/rains#Evaluation -->


    <owl:Class rdf:about="https://w3id.org/rains#Evaluation">
        <rdfs:subClassOf rdf:resource="https://w3id.org/sao#AccountableResult"/>
        <rdfs:subClassOf>
            <owl:Restriction>
                <owl:onProperty rdf:resource="https://w3id.org/ep-plan#isElementOfPlan"/>
                <owl:allValuesFrom>
                    <owl:Class>
                        <owl:unionOf rdf:parseType="Collection">
                            <rdf:Description rdf:about="https://w3id.org/rains#DeploymentStageAccountabilityPlan"/>
                            <rdf:Description rdf:about="https://w3id.org/rains#ImplementationStageAccountabilityPlan"/>
                            <rdf:Description rdf:about="https://w3id.org/rains#InstallationAccountabilityPlan"/>
                            <rdf:Description rdf:about="https://w3id.org/rains#MaintenanceAccountabilityPlan"/>
                            <rdf:Description rdf:about="https://w3id.org/rains#OperationStageAccountabilityPlan"/>
                        </owl:unionOf>
                    </owl:Class>
                </owl:allValuesFrom>
            </owl:Restriction>
        </rdfs:subClassOf>
        <rdfs:subClassOf>
            <owl:Restriction>
                <owl:onProperty rdf:resource="https://w3id.org/ep-plan#isOutputVariableOf"/>
                <owl:allValuesFrom rdf:resource="https://w3id.org/rains#Evaluate"/>
            </owl:Restriction>
        </rdfs:subClassOf>
        <rdfs:subClassOf>
            <owl:Restriction>
                <owl:onProperty rdf:resource="https://w3id.org/ep-plan#isVariableOfPlan"/>
                <owl:allValuesFrom>
                    <owl:Class>
                        <owl:unionOf rdf:parseType="Collection">
                            <rdf:Description rdf:about="https://w3id.org/rains#DeploymentStageAccountabilityPlan"/>
                            <rdf:Description rdf:about="https://w3id.org/rains#ImplementationStageAccountabilityPlan"/>
                            <rdf:Description rdf:about="https://w3id.org/rains#InstallationAccountabilityPlan"/>
                            <rdf:Description rdf:about="https://w3id.org/rains#MaintenanceAccountabilityPlan"/>
                            <rdf:Description rdf:about="https://w3id.org/rains#OperationStageAccountabilityPlan"/>
                        </owl:unionOf>
                    </owl:Class>
                </owl:allValuesFrom>
            </owl:Restriction>
        </rdfs:subClassOf>
        <owl:disjointWith rdf:resource="https://w3id.org/rains#Guideline"/>
        <owl:disjointWith rdf:resource="https://w3id.org/rains#HumanDecision"/>
        <owl:disjointWith rdf:resource="https://w3id.org/rains#Log"/>
        <owl:disjointWith rdf:resource="https://w3id.org/rains#SystemData"/>
        <owl:disjointWith rdf:resource="https://w3id.org/rains#UserTrainingReport"/>
        <rdfs:comment>A specific type of planned sao:AccountableResult which represents a high level reference to testing at least one component and recording the results of the test(s) (e.g. testing the model with a specified dataset) that is expected to be produced during the implementation stage.

It is advisable that the information realization corresponding to the Evaluation variable contains the following information elements:
1. Either an instance of mls:EvaluationProcedure (if it is the model being evaluated) or EvaluationProcedure (if it is not the ML model being evaluated). Either should also be an instance of RealizedObject. If the evaluation deviates from the design, then an additional instance of mls:EvaluationProcedure or EvaluationProcedure should be indicated as an instance of ExcludedObject.
2. Either an instance of mls:EvaluationMeasure (if it is the model being evaluated) or EvaluationMeasure(if it is not the ML model being evaluated). If the evaluation deviates from the design, then an additional instance of mls:EvaluationMeasure or EvaluationMeasure should be indicated as an instance of ExcludedObject.
3. Either an instance of mls:ModelEvaluation (if it is the model being evaluated) or EvaluationResult (if it is not the ML model being evaluated). If the evaluation deviates from the design, then an additional instance of mls:ModelEvaluation or EvaluationResult should be indicated as an instance of ExcludedObject.
4. The subclasses of Compliance Entity, namely, Hard Law and SoftLaw

It is discouraged that the information realization corresponding to the Evaluation variable contains the following information elements:
1. The subclasses of Guidance, namely, System Deployment Guidance, SystemInstallationGuidance, UserTrainingGuidance, SystemOperationGuidance, SystemUsageGuidance, and SystemMaintenanceGuidance
2. Notification Proof</rdfs:comment>
        <rdfs:label>Evaluation</rdfs:label>
    </owl:Class>
    


    <!-- https://w3id.org/rains#EvaluationDataset -->


    <owl:Class rdf:about="https://w3id.org/rains#EvaluationDataset">
        <rdfs:subClassOf rdf:resource="https://w3id.org/rains#DatasetComponent"/>
        <rdfs:subClassOf>
            <owl:Restriction>
                <owl:onProperty rdf:resource="https://w3id.org/ep-plan#isElementOfPlan"/>
                <owl:allValuesFrom>
                    <owl:Class>
                        <owl:unionOf rdf:parseType="Collection">
                            <rdf:Description rdf:about="https://w3id.org/rains#DeploymentStageAccountabilityPlan"/>
                            <rdf:Description rdf:about="https://w3id.org/rains#ImplementationStageAccountabilityPlan"/>
                            <rdf:Description rdf:about="https://w3id.org/rains#InstallationAccountabilityPlan"/>
                            <rdf:Description rdf:about="https://w3id.org/rains#MaintenanceAccountabilityPlan"/>
                            <rdf:Description rdf:about="https://w3id.org/rains#OperationStageAccountabilityPlan"/>
                        </owl:unionOf>
                    </owl:Class>
                </owl:allValuesFrom>
            </owl:Restriction>
        </rdfs:subClassOf>
        <rdfs:subClassOf>
            <owl:Restriction>
                <owl:onProperty rdf:resource="https://w3id.org/ep-plan#isOutputVariableOf"/>
                <owl:allValuesFrom>
                    <owl:Class>
                        <owl:unionOf rdf:parseType="Collection">
                            <rdf:Description rdf:about="https://w3id.org/rains#MergeAndSplitDataset"/>
                            <rdf:Description rdf:about="https://w3id.org/rains#RealizeComponent"/>
                        </owl:unionOf>
                    </owl:Class>
                </owl:allValuesFrom>
            </owl:Restriction>
        </rdfs:subClassOf>
        <rdfs:subClassOf>
            <owl:Restriction>
                <owl:onProperty rdf:resource="https://w3id.org/ep-plan#isVariableOfPlan"/>
                <owl:allValuesFrom>
                    <owl:Class>
                        <owl:unionOf rdf:parseType="Collection">
                            <rdf:Description rdf:about="https://w3id.org/rains#DeploymentStageAccountabilityPlan"/>
                            <rdf:Description rdf:about="https://w3id.org/rains#ImplementationStageAccountabilityPlan"/>
                            <rdf:Description rdf:about="https://w3id.org/rains#InstallationAccountabilityPlan"/>
                            <rdf:Description rdf:about="https://w3id.org/rains#MaintenanceAccountabilityPlan"/>
                            <rdf:Description rdf:about="https://w3id.org/rains#OperationStageAccountabilityPlan"/>
                        </owl:unionOf>
                    </owl:Class>
                </owl:allValuesFrom>
            </owl:Restriction>
        </rdfs:subClassOf>
        <rdfs:comment>A specific type of a Dataset Component  which represents a subset of the whole collected and pre-processed datasets after they were merged then split to be fed into the ML Model. This specific type represents the data used to evaluate the ML Model. The other subsets are used to train and evaluate the model. This type can also represent a standalone dataset used to evaluate the model independent of the datasets used to train and validate it.</rdfs:comment>
        <rdfs:label>Evaluation Dataset</rdfs:label>
    </owl:Class>
    


    <!-- https://w3id.org/rains#EvaluationMeassure -->


    <owl:Class rdf:about="https://w3id.org/rains#EvaluationMeassure">
        <rdfs:subClassOf rdf:resource="https://w3id.org/sao#InformationElement"/>
        <rdfs:comment>A  sao:InformationElement which records a specific piece of  information detailing some measure used as part of an evaluation process. This is broader than mls:EvaluationMeassure which describes a measure related to a model performance.</rdfs:comment>
        <rdfs:label>Evaluation Measure</rdfs:label>
    </owl:Class>
    


    <!-- https://w3id.org/rains#EvaluationProcedure -->


    <owl:Class rdf:about="https://w3id.org/rains#EvaluationProcedure">
        <rdfs:subClassOf rdf:resource="https://w3id.org/sao#InformationElement"/>
        <rdfs:comment>A sao:InformationElement  which records a specific piece of  information detailing the procedure by which some aspects of an :AI_Sytem were evaluated. This is broader than mls:EvaluationProcedure which relates to model evaluation.</rdfs:comment>
        <rdfs:label>Evaluation Procedure</rdfs:label>
    </owl:Class>
    


    <!-- https://w3id.org/rains#EvaluationResult -->


    <owl:Class rdf:about="https://w3id.org/rains#EvaluationResult">
        <rdfs:subClassOf rdf:resource="https://w3id.org/sao#InformationElement"/>
        <rdfs:comment>A  sao:InformationElement which records a specific piece of  information detailing the result of an evaluation process. This is broader than mls:EvaluationMeassure which describes a result related to a specific model evaluation.</rdfs:comment>
        <rdfs:label>Evaluation Result</rdfs:label>
    </owl:Class>
    


    <!-- https://w3id.org/rains#EvaluationSpecification -->


    <owl:Class rdf:about="https://w3id.org/rains#EvaluationSpecification">
        <rdfs:subClassOf rdf:resource="https://w3id.org/rains#DesignSpecification"/>
        <rdfs:subClassOf>
            <owl:Restriction>
                <owl:onProperty rdf:resource="https://w3id.org/ep-plan#isElementOfPlan"/>
                <owl:allValuesFrom>
                    <owl:Class>
                        <owl:unionOf rdf:parseType="Collection">
                            <rdf:Description rdf:about="https://w3id.org/rains#DesignStageAccountabilityPlan"/>
                            <rdf:Description rdf:about="https://w3id.org/rains#ImplementationStageAccountabilityPlan"/>
                        </owl:unionOf>
                    </owl:Class>
                </owl:allValuesFrom>
            </owl:Restriction>
        </rdfs:subClassOf>
        <rdfs:subClassOf>
            <owl:Restriction>
                <owl:onProperty rdf:resource="https://w3id.org/ep-plan#isOutputVariableOf"/>
                <owl:allValuesFrom rdf:resource="https://w3id.org/rains#ProduceSpecification"/>
            </owl:Restriction>
        </rdfs:subClassOf>
        <rdfs:subClassOf>
            <owl:Restriction>
                <owl:onProperty rdf:resource="https://w3id.org/ep-plan#isVariableOfPlan"/>
                <owl:allValuesFrom>
                    <owl:Class>
                        <owl:unionOf rdf:parseType="Collection">
                            <rdf:Description rdf:about="https://w3id.org/rains#DesignStageAccountabilityPlan"/>
                            <rdf:Description rdf:about="https://w3id.org/rains#ImplementationStageAccountabilityPlan"/>
                        </owl:unionOf>
                    </owl:Class>
                </owl:allValuesFrom>
            </owl:Restriction>
        </rdfs:subClassOf>
        <owl:disjointWith rdf:resource="https://w3id.org/rains#SystemPurposeSpecification"/>
        <rdfs:comment>A specific type of design specification which represents the description  of a planned evaluation process.

It is advisable that the information realization corresponding to EvaluationSpecification contains the following information elements:
1. Either an instance of mls:EvaluationProcedure (if it is the model being evaluated) or EvaluationProcedure (if it is not the ML model being evaluated). 
2. Either an instance of mls: EvaluationMeasure (if it is the model being evaluated) or EvaluationMeasure (if it is not the ML model being evaluated).
3. If available: Either an instance of mls:ModelEvaluation (if it is the model being evaluated) or EvaluationResult (if it is not the ML model being evaluated).
4. HardLaw
5. SoftLaw

It is discouraged that the information realization corresponding to the Evaluation Specification contains the following information elements:
1. SystemIntegrationGuidance
2. SystemDeploymentGuidance
3. SystemDocumentationGuidance
4. SystemIntegrationGuidance
5. SystemUsageGuidance</rdfs:comment>
        <rdfs:label>Evaluation Specification</rdfs:label>
    </owl:Class>
    


    <!-- https://w3id.org/rains#ExcludedObject -->


    <owl:Class rdf:about="https://w3id.org/rains#ExcludedObject">
        <rdfs:subClassOf rdf:resource="https://w3id.org/sao#InformationElement"/>
        <owl:disjointWith rdf:resource="https://w3id.org/rains#RealizededObject"/>
        <rdfs:comment>A sao:InformationElement which records information detailing a piece of data, software or hardware that should have been realized but was not.

For example, assume the dataset design specification specifies that dataset foobar is to be realised (to be used to train the model), but the implementation team realises dataset xyzzy instead. In this case, the dataset foobar should be indicated by the implementation team as an Excluded Object - whereas the dataset xyzzy should be created as an instance of :RealizedObject.</rdfs:comment>
        <rdfs:label>Excluded Object</rdfs:label>
    </owl:Class>
    


    <!-- https://w3id.org/rains#Explain -->


    <owl:Class rdf:about="https://w3id.org/rains#Explain">
        <rdfs:subClassOf rdf:resource="https://w3id.org/rains#SystemAction"/>
        <rdfs:subClassOf>
            <owl:Restriction>
                <owl:onProperty rdf:resource="https://w3id.org/ep-plan#hasOutputVariable"/>
                <owl:allValuesFrom rdf:resource="https://w3id.org/rains#Explanation"/>
            </owl:Restriction>
        </rdfs:subClassOf>
        <rdfs:subClassOf>
            <owl:Restriction>
                <owl:onProperty rdf:resource="https://w3id.org/ep-plan#isElementOfPlan"/>
                <owl:allValuesFrom>
                    <owl:Class>
                        <owl:unionOf rdf:parseType="Collection">
                            <rdf:Description rdf:about="https://w3id.org/rains#ConfigurationAccountabilityPlan"/>
                            <rdf:Description rdf:about="https://w3id.org/rains#OperationStageAccountabilityPlan"/>
                            <rdf:Description rdf:about="https://w3id.org/rains#RuntimeAccountabilityPlan"/>
                        </owl:unionOf>
                    </owl:Class>
                </owl:allValuesFrom>
            </owl:Restriction>
        </rdfs:subClassOf>
        <rdfs:subClassOf>
            <owl:Restriction>
                <owl:onProperty rdf:resource="https://w3id.org/ep-plan#isStepOfPlan"/>
                <owl:allValuesFrom>
                    <owl:Class>
                        <owl:unionOf rdf:parseType="Collection">
                            <rdf:Description rdf:about="https://w3id.org/rains#ConfigurationAccountabilityPlan"/>
                            <rdf:Description rdf:about="https://w3id.org/rains#OperationStageAccountabilityPlan"/>
                            <rdf:Description rdf:about="https://w3id.org/rains#RuntimeAccountabilityPlan"/>
                        </owl:unionOf>
                    </owl:Class>
                </owl:allValuesFrom>
            </owl:Restriction>
        </rdfs:subClassOf>
        <owl:disjointWith rdf:resource="https://w3id.org/rains#GenerateOutput"/>
        <owl:disjointWith rdf:resource="https://w3id.org/rains#Justify"/>
        <owl:disjointWith rdf:resource="https://w3id.org/rains#NotifyUser"/>
        <owl:disjointWith rdf:resource="https://w3id.org/rains#PreprocessInputData"/>
        <owl:disjointWith rdf:resource="https://w3id.org/rains#ProvideSystemInputData"/>
        <owl:disjointWith rdf:resource="https://w3id.org/rains#ReturnOutput"/>
        <owl:disjointWith rdf:resource="https://w3id.org/rains#Validate"/>
        <rdfs:comment>A planned step that has some impact on the output of AI System where a Supporting Infrastrcuture component explains an output produced either by a Model Component or a Supporting Infrastructure Component. This step is typically part of the Operation stage (specifically Configuration or Runtime stages) and has a member of the class Explanation as its expected output. This steps  is not needed for model or supporting infrastructure components which can produce their own explanation. If a model or supporting infrastructure component can generate its own explanation, then they do by generating an explanation along with their outputs.</rdfs:comment>
        <rdfs:label>Explain</rdfs:label>
    </owl:Class>
    


    <!-- https://w3id.org/rains#Explanation -->


    <owl:Class rdf:about="https://w3id.org/rains#Explanation">
        <rdfs:subClassOf rdf:resource="https://w3id.org/rains#SystemData"/>
        <rdfs:subClassOf>
            <owl:Restriction>
                <owl:onProperty rdf:resource="https://w3id.org/ep-plan#isElementOfPlan"/>
                <owl:allValuesFrom>
                    <owl:Class>
                        <owl:unionOf rdf:parseType="Collection">
                            <rdf:Description rdf:about="https://w3id.org/rains#ConfigurationAccountabilityPlan"/>
                            <rdf:Description rdf:about="https://w3id.org/rains#OperationStageAccountabilityPlan"/>
                            <rdf:Description rdf:about="https://w3id.org/rains#RuntimeAccountabilityPlan"/>
                        </owl:unionOf>
                    </owl:Class>
                </owl:allValuesFrom>
            </owl:Restriction>
        </rdfs:subClassOf>
        <rdfs:subClassOf>
            <owl:Restriction>
                <owl:onProperty rdf:resource="https://w3id.org/ep-plan#isOutputVariableOf"/>
                <owl:allValuesFrom>
                    <owl:Class>
                        <owl:unionOf rdf:parseType="Collection">
                            <rdf:Description rdf:about="https://w3id.org/rains#Aggregate"/>
                            <rdf:Description rdf:about="https://w3id.org/rains#Explain"/>
                            <rdf:Description rdf:about="https://w3id.org/rains#GenerateModelOutput"/>
                            <rdf:Description rdf:about="https://w3id.org/rains#GenerateOutput"/>
                        </owl:unionOf>
                    </owl:Class>
                </owl:allValuesFrom>
            </owl:Restriction>
        </rdfs:subClassOf>
        <rdfs:subClassOf>
            <owl:Restriction>
                <owl:onProperty rdf:resource="https://w3id.org/ep-plan#isVariableOfPlan"/>
                <owl:allValuesFrom>
                    <owl:Class>
                        <owl:unionOf rdf:parseType="Collection">
                            <rdf:Description rdf:about="https://w3id.org/rains#ConfigurationAccountabilityPlan"/>
                            <rdf:Description rdf:about="https://w3id.org/rains#OperationStageAccountabilityPlan"/>
                            <rdf:Description rdf:about="https://w3id.org/rains#RuntimeAccountabilityPlan"/>
                        </owl:unionOf>
                    </owl:Class>
                </owl:allValuesFrom>
            </owl:Restriction>
        </rdfs:subClassOf>
        <owl:disjointWith rdf:resource="https://w3id.org/rains#Notification"/>
        <owl:disjointWith rdf:resource="https://w3id.org/rains#RuntimeInputData"/>
        <owl:disjointWith rdf:resource="https://w3id.org/rains#UserConsent"/>
        <owl:disjointWith rdf:resource="https://w3id.org/rains#UserReview"/>
        <owl:disjointWith rdf:resource="https://w3id.org/rains#Validation"/>
        <rdfs:comment>A specific type of planned System Data which represents an explanation of an output produced either by a Model Component or a Supporting Infrastructure Component. The Model Component may produced its own explanation and a Supporting Infrastrcuture component may produce an explanation for its own output, another Supporting Infrastrcuture component&apos;s output, or a Model component&apos;s output.

If the AI System is involved in making decisions/recommendations/actions affecting human users, then it is advisable that the information realization corresponding to the Explanation variable contains the following information elements: Affected Agent.</rdfs:comment>
        <rdfs:label>Explanation</rdfs:label>
    </owl:Class>
    


    <!-- https://w3id.org/rains#ExplanationNotification -->


    <owl:Class rdf:about="https://w3id.org/rains#ExplanationNotification">
        <rdfs:subClassOf rdf:resource="https://w3id.org/rains#Notification"/>
        <rdfs:subClassOf>
            <owl:Restriction>
                <owl:onProperty rdf:resource="https://w3id.org/ep-plan#isElementOfPlan"/>
                <owl:allValuesFrom>
                    <owl:Class>
                        <owl:unionOf rdf:parseType="Collection">
                            <rdf:Description rdf:about="https://w3id.org/rains#ConfigurationAccountabilityPlan"/>
                            <rdf:Description rdf:about="https://w3id.org/rains#OperationStageAccountabilityPlan"/>
                            <rdf:Description rdf:about="https://w3id.org/rains#RuntimeAccountabilityPlan"/>
                        </owl:unionOf>
                    </owl:Class>
                </owl:allValuesFrom>
            </owl:Restriction>
        </rdfs:subClassOf>
        <rdfs:subClassOf>
            <owl:Restriction>
                <owl:onProperty rdf:resource="https://w3id.org/ep-plan#isOutputVariableOf"/>
                <owl:allValuesFrom rdf:resource="https://w3id.org/rains#NotifyUser"/>
            </owl:Restriction>
        </rdfs:subClassOf>
        <rdfs:subClassOf>
            <owl:Restriction>
                <owl:onProperty rdf:resource="https://w3id.org/ep-plan#isVariableOfPlan"/>
                <owl:allValuesFrom>
                    <owl:Class>
                        <owl:unionOf rdf:parseType="Collection">
                            <rdf:Description rdf:about="https://w3id.org/rains#ConfigurationAccountabilityPlan"/>
                            <rdf:Description rdf:about="https://w3id.org/rains#OperationStageAccountabilityPlan"/>
                            <rdf:Description rdf:about="https://w3id.org/rains#RuntimeAccountabilityPlan"/>
                        </owl:unionOf>
                    </owl:Class>
                </owl:allValuesFrom>
            </owl:Restriction>
        </rdfs:subClassOf>
        <rdfs:comment>A specific type of Notification which represents a notification of the explanation of an output to the user.

Similar to Notification, it is advisable that the information realization corresponding to the Explanation Notification variable contains the following information elements:
1. Affected Agent, describing the user who was notified.
2. Notification Proof, documenting how the user was notified, e.g. a screenshot of the explanation shown to the user.</rdfs:comment>
        <rdfs:label>Explanation Notification</rdfs:label>
    </owl:Class>
    


    <!-- https://w3id.org/rains#FairnessOrBiasDetectionSoftware -->


    <owl:Class rdf:about="https://w3id.org/rains#FairnessOrBiasDetectionSoftware">
        <rdfs:subClassOf rdf:resource="http://ontosoft.org/software#Software"/>
        <rdfs:comment>A sao:InformationElement (which is also an osw:Software and a prov:SoftwareAgent)  which records  information detailing  a software that was used to detect bias or check for fairness in both the dataset which was used to train the ML Model as well as the ML model itself</rdfs:comment>
        <rdfs:label>Fairness Or Bias Detection Software</rdfs:label>
    </owl:Class>
    


    <!-- https://w3id.org/rains#FitnessConfirmationDecision -->


    <owl:Class rdf:about="https://w3id.org/rains#FitnessConfirmationDecision">
        <rdfs:subClassOf rdf:resource="https://w3id.org/rains#HumanDecision"/>
        <rdfs:subClassOf>
            <owl:Restriction>
                <owl:onProperty rdf:resource="https://w3id.org/ep-plan#isElementOfPlan"/>
                <owl:allValuesFrom>
                    <owl:Class>
                        <owl:unionOf rdf:parseType="Collection">
                            <rdf:Description rdf:about="https://w3id.org/rains#DeploymentStageAccountabilityPlan"/>
                            <rdf:Description rdf:about="https://w3id.org/rains#DesignStageAccountabilityPlan"/>
                            <rdf:Description rdf:about="https://w3id.org/rains#ImplementationStageAccountabilityPlan"/>
                            <rdf:Description rdf:about="https://w3id.org/rains#InstallationAccountabilityPlan"/>
                            <rdf:Description rdf:about="https://w3id.org/rains#MaintenanceAccountabilityPlan"/>
                            <rdf:Description rdf:about="https://w3id.org/rains#ManualProductionAccountabilityPlan"/>
                            <rdf:Description rdf:about="https://w3id.org/rains#OperationStageAccountabilityPlan"/>
                            <rdf:Description rdf:about="https://w3id.org/rains#UserTrainingAccountabilityPlan"/>
                        </owl:unionOf>
                    </owl:Class>
                </owl:allValuesFrom>
            </owl:Restriction>
        </rdfs:subClassOf>
        <rdfs:subClassOf>
            <owl:Restriction>
                <owl:onProperty rdf:resource="https://w3id.org/ep-plan#isOutputVariableOf"/>
                <owl:allValuesFrom rdf:resource="https://w3id.org/rains#Decide"/>
            </owl:Restriction>
        </rdfs:subClassOf>
        <rdfs:subClassOf>
            <owl:Restriction>
                <owl:onProperty rdf:resource="https://w3id.org/ep-plan#isVariableOfPlan"/>
                <owl:allValuesFrom>
                    <owl:Class>
                        <owl:unionOf rdf:parseType="Collection">
                            <rdf:Description rdf:about="https://w3id.org/rains#DeploymentStageAccountabilityPlan"/>
                            <rdf:Description rdf:about="https://w3id.org/rains#DesignStageAccountabilityPlan"/>
                            <rdf:Description rdf:about="https://w3id.org/rains#ImplementationStageAccountabilityPlan"/>
                            <rdf:Description rdf:about="https://w3id.org/rains#InstallationAccountabilityPlan"/>
                            <rdf:Description rdf:about="https://w3id.org/rains#MaintenanceAccountabilityPlan"/>
                            <rdf:Description rdf:about="https://w3id.org/rains#ManualProductionAccountabilityPlan"/>
                            <rdf:Description rdf:about="https://w3id.org/rains#OperationStageAccountabilityPlan"/>
                            <rdf:Description rdf:about="https://w3id.org/rains#UserTrainingAccountabilityPlan"/>
                        </owl:unionOf>
                    </owl:Class>
                </owl:allValuesFrom>
            </owl:Restriction>
        </rdfs:subClassOf>
        <rdfs:comment>A specific type of planned human decision representing confirmation of fitness of some sao:AccountableResult t to its purpose.</rdfs:comment>
        <rdfs:label>Fitness Confirmation Decision</rdfs:label>
    </owl:Class>
    


    <!-- https://w3id.org/rains#Funding -->


    <owl:Class rdf:about="https://w3id.org/rains#Funding">
        <rdfs:subClassOf rdf:resource="https://w3id.org/sao#InformationElement"/>
        <rdfs:comment>A sao:InformationElement  which records a specific piece of  information detailing a funding source.</rdfs:comment>
        <rdfs:label>Funding</rdfs:label>
    </owl:Class>
    


    <!-- https://w3id.org/rains#GenerateGuideline -->


    <owl:Class rdf:about="https://w3id.org/rains#GenerateGuideline">
        <rdfs:subClassOf rdf:resource="https://w3id.org/sao#AccountableAction"/>
        <rdfs:subClassOf>
            <owl:Restriction>
                <owl:onProperty rdf:resource="https://w3id.org/ep-plan#hasOutputVariable"/>
                <owl:allValuesFrom>
                    <owl:Class>
                        <owl:unionOf rdf:parseType="Collection">
                            <rdf:Description rdf:about="https://w3id.org/rains#ChangeLog"/>
                            <rdf:Description rdf:about="https://w3id.org/rains#Guideline"/>
                            <rdf:Description rdf:about="https://w3id.org/rains#SystemDeploymentGuideline"/>
                            <rdf:Description rdf:about="https://w3id.org/rains#SystemInstallationGuideline"/>
                            <rdf:Description rdf:about="https://w3id.org/rains#SystemMaintenanceGuideline"/>
                            <rdf:Description rdf:about="https://w3id.org/rains#SystemOperationGuideline"/>
                            <rdf:Description rdf:about="https://w3id.org/rains#SystemUsageGuideline"/>
                            <rdf:Description rdf:about="https://w3id.org/rains#UserTrainingGuideline"/>
                        </owl:unionOf>
                    </owl:Class>
                </owl:allValuesFrom>
            </owl:Restriction>
        </rdfs:subClassOf>
        <rdfs:subClassOf>
            <owl:Restriction>
                <owl:onProperty rdf:resource="https://w3id.org/ep-plan#isElementOfPlan"/>
                <owl:allValuesFrom>
                    <owl:Class>
                        <owl:unionOf rdf:parseType="Collection">
                            <rdf:Description rdf:about="https://w3id.org/rains#DeploymentStageAccountabilityPlan"/>
                            <rdf:Description rdf:about="https://w3id.org/rains#ImplementationStageAccountabilityPlan"/>
                            <rdf:Description rdf:about="https://w3id.org/rains#ManualProductionAccountabilityPlan"/>
                        </owl:unionOf>
                    </owl:Class>
                </owl:allValuesFrom>
            </owl:Restriction>
        </rdfs:subClassOf>
        <rdfs:subClassOf>
            <owl:Restriction>
                <owl:onProperty rdf:resource="https://w3id.org/ep-plan#isStepOfPlan"/>
                <owl:allValuesFrom>
                    <owl:Class>
                        <owl:unionOf rdf:parseType="Collection">
                            <rdf:Description rdf:about="https://w3id.org/rains#DeploymentStageAccountabilityPlan"/>
                            <rdf:Description rdf:about="https://w3id.org/rains#ImplementationStageAccountabilityPlan"/>
                            <rdf:Description rdf:about="https://w3id.org/rains#ManualProductionAccountabilityPlan"/>
                        </owl:unionOf>
                    </owl:Class>
                </owl:allValuesFrom>
            </owl:Restriction>
        </rdfs:subClassOf>
        <owl:disjointWith rdf:resource="https://w3id.org/rains#Install"/>
        <owl:disjointWith rdf:resource="https://w3id.org/rains#MergeAndSplitDataset"/>
        <owl:disjointWith rdf:resource="https://w3id.org/rains#ProduceSpecification"/>
        <owl:disjointWith rdf:resource="https://w3id.org/rains#RealizeComponent"/>
        <owl:disjointWith rdf:resource="https://w3id.org/rains#SystemAction"/>
        <owl:disjointWith rdf:resource="https://w3id.org/rains#TrainUser"/>
        <rdfs:comment>A planned step describing the creation or editing of a guideline that has some impact on the AI System, e.g. the production of the deployment guideline describing how the AI System is to be deployed on-site or the editing of the maintenance guideline describing how the AI System is to be maintained. This step is typically part of the Implementation stage or the Deployment of an AI System&apos;s life cycle. It has members of the subclasses of Guideline as its expected output(s).  If the step describes the editing of a previously-generated guideline, then it will also have as an output a member of the class Change Log.</rdfs:comment>
        <rdfs:label>Generate Guideline</rdfs:label>
    </owl:Class>
    


    <!-- https://w3id.org/rains#GenerateModelOutput -->


    <owl:Class rdf:about="https://w3id.org/rains#GenerateModelOutput">
        <rdfs:subClassOf rdf:resource="https://w3id.org/rains#GenerateOutput"/>
        <rdfs:subClassOf>
            <owl:Restriction>
                <owl:onProperty rdf:resource="https://w3id.org/ep-plan#hasOutputVariable"/>
                <owl:allValuesFrom>
                    <owl:Class>
                        <owl:unionOf rdf:parseType="Collection">
                            <rdf:Description rdf:about="https://w3id.org/rains#Explanation"/>
                            <rdf:Description rdf:about="https://w3id.org/rains#ModelOutput"/>
                        </owl:unionOf>
                    </owl:Class>
                </owl:allValuesFrom>
            </owl:Restriction>
        </rdfs:subClassOf>
        <rdfs:subClassOf>
            <owl:Restriction>
                <owl:onProperty rdf:resource="https://w3id.org/ep-plan#isElementOfPlan"/>
                <owl:allValuesFrom>
                    <owl:Class>
                        <owl:unionOf rdf:parseType="Collection">
                            <rdf:Description rdf:about="https://w3id.org/rains#ConfigurationAccountabilityPlan"/>
                            <rdf:Description rdf:about="https://w3id.org/rains#DeploymentStageAccountabilityPlan"/>
                            <rdf:Description rdf:about="https://w3id.org/rains#InstallationAccountabilityPlan"/>
                            <rdf:Description rdf:about="https://w3id.org/rains#OperationStageAccountabilityPlan"/>
                            <rdf:Description rdf:about="https://w3id.org/rains#RuntimeAccountabilityPlan"/>
                        </owl:unionOf>
                    </owl:Class>
                </owl:allValuesFrom>
            </owl:Restriction>
        </rdfs:subClassOf>
        <rdfs:subClassOf>
            <owl:Restriction>
                <owl:onProperty rdf:resource="https://w3id.org/ep-plan#isStepOfPlan"/>
                <owl:allValuesFrom>
                    <owl:Class>
                        <owl:unionOf rdf:parseType="Collection">
                            <rdf:Description rdf:about="https://w3id.org/rains#ConfigurationAccountabilityPlan"/>
                            <rdf:Description rdf:about="https://w3id.org/rains#DeploymentStageAccountabilityPlan"/>
                            <rdf:Description rdf:about="https://w3id.org/rains#InstallationAccountabilityPlan"/>
                            <rdf:Description rdf:about="https://w3id.org/rains#OperationStageAccountabilityPlan"/>
                            <rdf:Description rdf:about="https://w3id.org/rains#RuntimeAccountabilityPlan"/>
                        </owl:unionOf>
                    </owl:Class>
                </owl:allValuesFrom>
            </owl:Restriction>
        </rdfs:subClassOf>
        <owl:disjointWith rdf:resource="https://w3id.org/rains#Override"/>
        <rdfs:comment>A planned step that  describes the generation of an output by a Model component of the AI System. This step is typically part of the Deployment or Operation Stages (specifically Installation or Configuration or Runtime stages) and has a member of the class Model Output as its expected output. It may also generate a member of the class Explanation as its output if it produces an explanation along with the output.</rdfs:comment>
        <rdfs:label>Generate Model Output</rdfs:label>
    </owl:Class>
    


    <!-- https://w3id.org/rains#GenerateOutput -->


    <owl:Class rdf:about="https://w3id.org/rains#GenerateOutput">
        <rdfs:subClassOf rdf:resource="https://w3id.org/rains#SystemAction"/>
        <rdfs:subClassOf>
            <owl:Restriction>
                <owl:onProperty rdf:resource="https://w3id.org/ep-plan#hasOutputVariable"/>
                <owl:allValuesFrom>
                    <owl:Class>
                        <owl:unionOf rdf:parseType="Collection">
                            <rdf:Description rdf:about="https://w3id.org/rains#Explanation"/>
                            <rdf:Description rdf:about="https://w3id.org/rains#SystemOutput"/>
                        </owl:unionOf>
                    </owl:Class>
                </owl:allValuesFrom>
            </owl:Restriction>
        </rdfs:subClassOf>
        <rdfs:subClassOf>
            <owl:Restriction>
                <owl:onProperty rdf:resource="https://w3id.org/ep-plan#isElementOfPlan"/>
                <owl:allValuesFrom>
                    <owl:Class>
                        <owl:unionOf rdf:parseType="Collection">
                            <rdf:Description rdf:about="https://w3id.org/rains#ConfigurationAccountabilityPlan"/>
                            <rdf:Description rdf:about="https://w3id.org/rains#DeploymentStageAccountabilityPlan"/>
                            <rdf:Description rdf:about="https://w3id.org/rains#InstallationAccountabilityPlan"/>
                            <rdf:Description rdf:about="https://w3id.org/rains#OperationStageAccountabilityPlan"/>
                            <rdf:Description rdf:about="https://w3id.org/rains#RuntimeAccountabilityPlan"/>
                        </owl:unionOf>
                    </owl:Class>
                </owl:allValuesFrom>
            </owl:Restriction>
        </rdfs:subClassOf>
        <rdfs:subClassOf>
            <owl:Restriction>
                <owl:onProperty rdf:resource="https://w3id.org/ep-plan#isStepOfPlan"/>
                <owl:allValuesFrom>
                    <owl:Class>
                        <owl:unionOf rdf:parseType="Collection">
                            <rdf:Description rdf:about="https://w3id.org/rains#ConfigurationAccountabilityPlan"/>
                            <rdf:Description rdf:about="https://w3id.org/rains#DeploymentStageAccountabilityPlan"/>
                            <rdf:Description rdf:about="https://w3id.org/rains#InstallationAccountabilityPlan"/>
                            <rdf:Description rdf:about="https://w3id.org/rains#OperationStageAccountabilityPlan"/>
                            <rdf:Description rdf:about="https://w3id.org/rains#RuntimeAccountabilityPlan"/>
                        </owl:unionOf>
                    </owl:Class>
                </owl:allValuesFrom>
            </owl:Restriction>
        </rdfs:subClassOf>
        <owl:disjointWith rdf:resource="https://w3id.org/rains#Justify"/>
        <owl:disjointWith rdf:resource="https://w3id.org/rains#NotifyUser"/>
        <owl:disjointWith rdf:resource="https://w3id.org/rains#PreprocessInputData"/>
        <owl:disjointWith rdf:resource="https://w3id.org/rains#ProvideSystemInputData"/>
        <owl:disjointWith rdf:resource="https://w3id.org/rains#ReturnOutput"/>
        <owl:disjointWith rdf:resource="https://w3id.org/rains#Validate"/>
        <rdfs:comment>A planned step that  describes the generation of an output or its explanation by the user or a component of the AI System, specifically a Supporting Infrastructure Component. While the Model Component may perform this step, it is advisable that it would perform its subclass Generate Model Component. This step is typically part of the Deployment or Operation Stages (specifically Installation or Configuration or Runtime stages) and has members of the class System Output or Explanation as its expected output.</rdfs:comment>
        <rdfs:label>Generate Output</rdfs:label>
    </owl:Class>
    


    <!-- https://w3id.org/rains#GrantCertification -->


    <owl:Class rdf:about="https://w3id.org/rains#GrantCertification">
        <rdfs:subClassOf rdf:resource="https://w3id.org/rains#Decide"/>
        <rdfs:subClassOf>
            <owl:Restriction>
                <owl:onProperty rdf:resource="https://w3id.org/ep-plan#hasOutputVariable"/>
                <owl:allValuesFrom rdf:resource="https://w3id.org/rains#CertificationDecision"/>
            </owl:Restriction>
        </rdfs:subClassOf>
        <rdfs:subClassOf>
            <owl:Restriction>
                <owl:onProperty rdf:resource="https://w3id.org/ep-plan#isElementOfPlan"/>
                <owl:allValuesFrom>
                    <owl:Class>
                        <owl:unionOf rdf:parseType="Collection">
                            <rdf:Description rdf:about="https://w3id.org/rains#DeploymentStageAccountabilityPlan"/>
                            <rdf:Description rdf:about="https://w3id.org/rains#DesignStageAccountabilityPlan"/>
                            <rdf:Description rdf:about="https://w3id.org/rains#ImplementationStageAccountabilityPlan"/>
                            <rdf:Description rdf:about="https://w3id.org/rains#InstallationAccountabilityPlan"/>
                            <rdf:Description rdf:about="https://w3id.org/rains#MaintenanceAccountabilityPlan"/>
                            <rdf:Description rdf:about="https://w3id.org/rains#ManualProductionAccountabilityPlan"/>
                            <rdf:Description rdf:about="https://w3id.org/rains#OperationStageAccountabilityPlan"/>
                            <rdf:Description rdf:about="https://w3id.org/rains#UserTrainingAccountabilityPlan"/>
                        </owl:unionOf>
                    </owl:Class>
                </owl:allValuesFrom>
            </owl:Restriction>
        </rdfs:subClassOf>
        <rdfs:subClassOf>
            <owl:Restriction>
                <owl:onProperty rdf:resource="https://w3id.org/ep-plan#isStepOfPlan"/>
                <owl:allValuesFrom>
                    <owl:Class>
                        <owl:unionOf rdf:parseType="Collection">
                            <rdf:Description rdf:about="https://w3id.org/rains#DeploymentStageAccountabilityPlan"/>
                            <rdf:Description rdf:about="https://w3id.org/rains#DesignStageAccountabilityPlan"/>
                            <rdf:Description rdf:about="https://w3id.org/rains#ImplementationStageAccountabilityPlan"/>
                            <rdf:Description rdf:about="https://w3id.org/rains#InstallationAccountabilityPlan"/>
                            <rdf:Description rdf:about="https://w3id.org/rains#MaintenanceAccountabilityPlan"/>
                            <rdf:Description rdf:about="https://w3id.org/rains#ManualProductionAccountabilityPlan"/>
                            <rdf:Description rdf:about="https://w3id.org/rains#OperationStageAccountabilityPlan"/>
                            <rdf:Description rdf:about="https://w3id.org/rains#UserTrainingAccountabilityPlan"/>
                        </owl:unionOf>
                    </owl:Class>
                </owl:allValuesFrom>
            </owl:Restriction>
        </rdfs:subClassOf>
        <rdfs:comment>A planned step describing a certification granting decision to be taken by a human when incorporating accountability in AI Systems, e.g. grant an ISO certificate. This step has members of the class Certification Decision as its expected output.</rdfs:comment>
        <rdfs:label>Grant Certification</rdfs:label>
    </owl:Class>
    


    <!-- https://w3id.org/rains#Guidance -->


    <owl:Class rdf:about="https://w3id.org/rains#Guidance">
        <rdfs:subClassOf rdf:resource="https://w3id.org/sao#InformationElement"/>
        <rdfs:comment>A sao:InformationElement  which records a specific piece of  information detailing instructions that should be followed during the deployment or operation stage of the :AI_System lifecycle.</rdfs:comment>
        <rdfs:label>Guidance</rdfs:label>
    </owl:Class>
    


    <!-- https://w3id.org/rains#Guideline -->


    <owl:Class rdf:about="https://w3id.org/rains#Guideline">
        <rdfs:subClassOf rdf:resource="https://w3id.org/sao#AccountableResult"/>
        <rdfs:subClassOf>
            <owl:Restriction>
                <owl:onProperty rdf:resource="https://w3id.org/ep-plan#isElementOfPlan"/>
                <owl:allValuesFrom>
                    <owl:Class>
                        <owl:unionOf rdf:parseType="Collection">
                            <rdf:Description rdf:about="https://w3id.org/rains#DeploymentStageAccountabilityPlan"/>
                            <rdf:Description rdf:about="https://w3id.org/rains#ImplementationStageAccountabilityPlan"/>
                            <rdf:Description rdf:about="https://w3id.org/rains#InstallationAccountabilityPlan"/>
                            <rdf:Description rdf:about="https://w3id.org/rains#MaintenanceAccountabilityPlan"/>
                            <rdf:Description rdf:about="https://w3id.org/rains#ManualProductionAccountabilityPlan"/>
                            <rdf:Description rdf:about="https://w3id.org/rains#OperationStageAccountabilityPlan"/>
                            <rdf:Description rdf:about="https://w3id.org/rains#RuntimeAccountabilityPlan"/>
                            <rdf:Description rdf:about="https://w3id.org/rains#UserTrainingAccountabilityPlan"/>
                        </owl:unionOf>
                    </owl:Class>
                </owl:allValuesFrom>
            </owl:Restriction>
        </rdfs:subClassOf>
        <rdfs:subClassOf>
            <owl:Restriction>
                <owl:onProperty rdf:resource="https://w3id.org/ep-plan#isOutputVariableOf"/>
                <owl:allValuesFrom rdf:resource="https://w3id.org/rains#GenerateGuideline"/>
            </owl:Restriction>
        </rdfs:subClassOf>
        <rdfs:subClassOf>
            <owl:Restriction>
                <owl:onProperty rdf:resource="https://w3id.org/ep-plan#isVariableOfPlan"/>
                <owl:allValuesFrom>
                    <owl:Class>
                        <owl:unionOf rdf:parseType="Collection">
                            <rdf:Description rdf:about="https://w3id.org/rains#DeploymentStageAccountabilityPlan"/>
                            <rdf:Description rdf:about="https://w3id.org/rains#ImplementationStageAccountabilityPlan"/>
                            <rdf:Description rdf:about="https://w3id.org/rains#InstallationAccountabilityPlan"/>
                            <rdf:Description rdf:about="https://w3id.org/rains#MaintenanceAccountabilityPlan"/>
                            <rdf:Description rdf:about="https://w3id.org/rains#ManualProductionAccountabilityPlan"/>
                            <rdf:Description rdf:about="https://w3id.org/rains#OperationStageAccountabilityPlan"/>
                            <rdf:Description rdf:about="https://w3id.org/rains#RuntimeAccountabilityPlan"/>
                            <rdf:Description rdf:about="https://w3id.org/rains#UserTrainingAccountabilityPlan"/>
                        </owl:unionOf>
                    </owl:Class>
                </owl:allValuesFrom>
            </owl:Restriction>
        </rdfs:subClassOf>
        <owl:disjointWith rdf:resource="https://w3id.org/rains#HumanDecision"/>
        <owl:disjointWith rdf:resource="https://w3id.org/rains#Log"/>
        <owl:disjointWith rdf:resource="https://w3id.org/rains#ModelComponent"/>
        <owl:disjointWith rdf:resource="https://w3id.org/rains#SupportingInfrastructureComponent"/>
        <owl:disjointWith rdf:resource="https://w3id.org/rains#SystemData"/>
        <owl:disjointWith rdf:resource="https://w3id.org/rains#UserTrainingReport"/>
        <rdfs:comment>A specific type of planned sao:AccountableResult which represents a high level reference to a guideline (e.g. a guideline document) that is expected to be produced during the implementation in order to inform on the correct procedure for deploying, using and maintaining the system or any of its components.</rdfs:comment>
        <rdfs:label>Guideline</rdfs:label>
    </owl:Class>
    


    <!-- https://w3id.org/rains#HardLaw -->


    <owl:Class rdf:about="https://w3id.org/rains#HardLaw">
        <rdfs:subClassOf rdf:resource="https://w3id.org/rains#ComplianceEntity"/>
        <owl:disjointWith rdf:resource="https://w3id.org/rains#SoftLaw"/>
        <rdfs:comment>A specific type of compliance entity which records a specific piece of  information about the laws and regulations that must be, or are, complied with as part of an information realization collection.

When used as part of an information realization corresponding to a design specification, it describes the hard laws that must be complied with. When used as part of an information realization corresponding to an realized component, it describes the hard laws that the component complies with.</rdfs:comment>
        <rdfs:label>Hard Law</rdfs:label>
    </owl:Class>
    


    <!-- https://w3id.org/rains#HumanConstraint -->


    <owl:Class rdf:about="https://w3id.org/rains#HumanConstraint">
        <rdfs:subClassOf rdf:resource="https://w3id.org/ep-plan#Constraint"/>
        <rdfs:comment>A specific type of planned ep-plan:Constraint that describes some constraint which cannot be evaluated automatically against the accountability trace. This can be, for example, because the constraint is too high level or difficult to express as a rule. Such constraint would be typically expected to be evaluated manually by a human.</rdfs:comment>
        <rdfs:label>Human Constraint</rdfs:label>
    </owl:Class>
    


    <!-- https://w3id.org/rains#HumanDecision -->


    <owl:Class rdf:about="https://w3id.org/rains#HumanDecision">
        <rdfs:subClassOf rdf:resource="https://w3id.org/sao#AccountableResult"/>
        <rdfs:subClassOf>
            <owl:Restriction>
                <owl:onProperty rdf:resource="https://w3id.org/ep-plan#isElementOfPlan"/>
                <owl:allValuesFrom>
                    <owl:Class>
                        <owl:unionOf rdf:parseType="Collection">
                            <rdf:Description rdf:about="https://w3id.org/rains#DeploymentStageAccountabilityPlan"/>
                            <rdf:Description rdf:about="https://w3id.org/rains#DesignStageAccountabilityPlan"/>
                            <rdf:Description rdf:about="https://w3id.org/rains#ImplementationStageAccountabilityPlan"/>
                            <rdf:Description rdf:about="https://w3id.org/rains#OperationStageAccountabilityPlan"/>
                        </owl:unionOf>
                    </owl:Class>
                </owl:allValuesFrom>
            </owl:Restriction>
        </rdfs:subClassOf>
        <rdfs:subClassOf>
            <owl:Restriction>
                <owl:onProperty rdf:resource="https://w3id.org/ep-plan#isOutputVariableOf"/>
                <owl:allValuesFrom rdf:resource="https://w3id.org/rains#Decide"/>
            </owl:Restriction>
        </rdfs:subClassOf>
        <rdfs:subClassOf>
            <owl:Restriction>
                <owl:onProperty rdf:resource="https://w3id.org/ep-plan#isVariableOfPlan"/>
                <owl:allValuesFrom>
                    <owl:Class>
                        <owl:unionOf rdf:parseType="Collection">
                            <rdf:Description rdf:about="https://w3id.org/rains#DeploymentStageAccountabilityPlan"/>
                            <rdf:Description rdf:about="https://w3id.org/rains#DesignStageAccountabilityPlan"/>
                            <rdf:Description rdf:about="https://w3id.org/rains#ImplementationStageAccountabilityPlan"/>
                            <rdf:Description rdf:about="https://w3id.org/rains#OperationStageAccountabilityPlan"/>
                        </owl:unionOf>
                    </owl:Class>
                </owl:allValuesFrom>
            </owl:Restriction>
        </rdfs:subClassOf>
        <owl:disjointWith rdf:resource="https://w3id.org/rains#Log"/>
        <owl:disjointWith rdf:resource="https://w3id.org/rains#ModelComponent"/>
        <owl:disjointWith rdf:resource="https://w3id.org/rains#SupportingInfrastructureComponent"/>
        <owl:disjointWith rdf:resource="https://w3id.org/rains#SystemData"/>
        <owl:disjointWith rdf:resource="https://w3id.org/rains#UserTrainingReport"/>
        <rdfs:comment>A specific type of a planned sao:AccountableResult which represents a decision made by a human.</rdfs:comment>
        <rdfs:label>Human Decision</rdfs:label>
    </owl:Class>
    


    <!-- https://w3id.org/rains#ImplementationStageAccountabilityPlan -->


    <owl:Class rdf:about="https://w3id.org/rains#ImplementationStageAccountabilityPlan">
        <rdfs:subClassOf rdf:resource="https://w3id.org/sao#AccountabilityPlan"/>
        <rdfs:subClassOf>
            <owl:Restriction>
                <owl:onProperty rdf:resource="https://w3id.org/ep-plan#includesStep"/>
                <owl:allValuesFrom>
                    <owl:Class>
                        <owl:unionOf rdf:parseType="Collection">
                            <rdf:Description rdf:about="https://w3id.org/rains#Decide"/>
                            <rdf:Description rdf:about="https://w3id.org/rains#Evaluate"/>
                            <rdf:Description rdf:about="https://w3id.org/rains#GenerateGuideline"/>
                            <rdf:Description rdf:about="https://w3id.org/rains#GrantCertification"/>
                            <rdf:Description rdf:about="https://w3id.org/rains#MergeAndSplitDataset"/>
                            <rdf:Description rdf:about="https://w3id.org/rains#RealizeComponent"/>
                        </owl:unionOf>
                    </owl:Class>
                </owl:allValuesFrom>
            </owl:Restriction>
        </rdfs:subClassOf>
        <rdfs:subClassOf>
            <owl:Restriction>
                <owl:onProperty rdf:resource="https://w3id.org/ep-plan#includesVariable"/>
                <owl:allValuesFrom>
                    <owl:Class>
                        <owl:unionOf rdf:parseType="Collection">
                            <rdf:Description rdf:about="https://w3id.org/rains#ApprovalDecision"/>
                            <rdf:Description rdf:about="https://w3id.org/rains#CertificationDecision"/>
                            <rdf:Description rdf:about="https://w3id.org/rains#ChangeLog"/>
                            <rdf:Description rdf:about="https://w3id.org/rains#ComplianceAssuranceDecision"/>
                            <rdf:Description rdf:about="https://w3id.org/rains#DatasetComponent"/>
                            <rdf:Description rdf:about="https://w3id.org/rains#Evaluation"/>
                            <rdf:Description rdf:about="https://w3id.org/rains#EvaluationDataset"/>
                            <rdf:Description rdf:about="https://w3id.org/rains#FitnessConfirmationDecision"/>
                            <rdf:Description rdf:about="https://w3id.org/rains#Guideline"/>
                            <rdf:Description rdf:about="https://w3id.org/rains#HumanDecision"/>
                            <rdf:Description rdf:about="https://w3id.org/rains#ModelComponent"/>
                            <rdf:Description rdf:about="https://w3id.org/rains#SupportingInfrastructureComponent"/>
                            <rdf:Description rdf:about="https://w3id.org/rains#SystemDeploymentGuideline"/>
                            <rdf:Description rdf:about="https://w3id.org/rains#SystemOperationGuideline"/>
                            <rdf:Description rdf:about="https://w3id.org/rains#ThirdPartyEvaluation"/>
                            <rdf:Description rdf:about="https://w3id.org/rains#TrainingDataset"/>
                            <rdf:Description rdf:about="https://w3id.org/rains#ValidationDataset"/>
                        </owl:unionOf>
                    </owl:Class>
                </owl:allValuesFrom>
            </owl:Restriction>
        </rdfs:subClassOf>
        <rdfs:comment>A plan that identifies sao:AccountableAction(s) and sao:AccountableResult(s) relevant to the implementation stage of an AI system and  which are required to be documented for accountability purposes. The Accountable Actions that can be done at this stage are: Realize Component, Merge and Split Dataset, Evaluate, Generate Guideline, Grant Certification, and Decide.</rdfs:comment>
        <rdfs:label>Implementation Stage Accountability Plan</rdfs:label>
    </owl:Class>
    


    <!-- https://w3id.org/rains#IncorrectUseCase -->


    <owl:Class rdf:about="https://w3id.org/rains#IncorrectUseCase">
        <rdfs:subClassOf rdf:resource="https://w3id.org/rains#UseCase"/>
        <owl:disjointWith rdf:resource="https://w3id.org/rains#IntendedUseCase"/>
        <rdfs:comment>A type of :UseCase detailing a situation in which any component of :AI_System or the system as whole should not be used.</rdfs:comment>
        <rdfs:label>Incorrect Use Case</rdfs:label>
    </owl:Class>
    


    <!-- https://w3id.org/rains#Install -->


    <owl:Class rdf:about="https://w3id.org/rains#Install">
        <rdfs:subClassOf rdf:resource="https://w3id.org/sao#AccountableAction"/>
        <rdfs:subClassOf>
            <owl:Restriction>
                <owl:onProperty rdf:resource="https://w3id.org/ep-plan#hasOutputVariable"/>
                <owl:allValuesFrom>
                    <owl:Class>
                        <owl:unionOf rdf:parseType="Collection">
                            <rdf:Description rdf:about="https://w3id.org/rains#ChangeLog"/>
                            <rdf:Description rdf:about="https://w3id.org/rains#InstallationLog"/>
                            <rdf:Description rdf:about="https://w3id.org/rains#ModelComponent"/>
                            <rdf:Description rdf:about="https://w3id.org/rains#SupportingInfrastructureComponent"/>
                        </owl:unionOf>
                    </owl:Class>
                </owl:allValuesFrom>
            </owl:Restriction>
        </rdfs:subClassOf>
        <rdfs:subClassOf>
            <owl:Restriction>
                <owl:onProperty rdf:resource="https://w3id.org/ep-plan#isElementOfPlan"/>
                <owl:allValuesFrom>
                    <owl:Class>
                        <owl:unionOf rdf:parseType="Collection">
                            <rdf:Description rdf:about="https://w3id.org/rains#DeploymentStageAccountabilityPlan"/>
                            <rdf:Description rdf:about="https://w3id.org/rains#InstallationAccountabilityPlan"/>
                        </owl:unionOf>
                    </owl:Class>
                </owl:allValuesFrom>
            </owl:Restriction>
        </rdfs:subClassOf>
        <rdfs:subClassOf>
            <owl:Restriction>
                <owl:onProperty rdf:resource="https://w3id.org/ep-plan#isStepOfPlan"/>
                <owl:allValuesFrom>
                    <owl:Class>
                        <owl:unionOf rdf:parseType="Collection">
                            <rdf:Description rdf:about="https://w3id.org/rains#DeploymentStageAccountabilityPlan"/>
                            <rdf:Description rdf:about="https://w3id.org/rains#InstallationAccountabilityPlan"/>
                        </owl:unionOf>
                    </owl:Class>
                </owl:allValuesFrom>
            </owl:Restriction>
        </rdfs:subClassOf>
        <owl:disjointWith rdf:resource="https://w3id.org/rains#MergeAndSplitDataset"/>
        <owl:disjointWith rdf:resource="https://w3id.org/rains#ProduceSpecification"/>
        <owl:disjointWith rdf:resource="https://w3id.org/rains#RealizeComponent"/>
        <owl:disjointWith rdf:resource="https://w3id.org/rains#SystemAction"/>
        <owl:disjointWith rdf:resource="https://w3id.org/rains#TrainUser"/>
        <rdfs:comment>A planned step describing how the AI system is installed during the Deployment stage. This action subsumes any integrations and configurations done as part of the installation. If any configurations are done after the system has been installed but before the Operation Stage, then the Accountable Action Configure is to be used to describe such configurations. This step has members of the classes Model Component, Supporting Infrastructure Component, Installation Log as its expected outputs.  If a deviation from the guidelines takes place, then the step will also have as an output a member of the class Change Log.</rdfs:comment>
        <rdfs:label>Install</rdfs:label>
    </owl:Class>
    


    <!-- https://w3id.org/rains#InstallationAccountabilityPlan -->


    <owl:Class rdf:about="https://w3id.org/rains#InstallationAccountabilityPlan">
        <rdfs:subClassOf rdf:resource="https://w3id.org/rains#DeploymentStageAccountabilityPlan"/>
        <rdfs:comment>A plan that identifies sao:AccountableAction(s) and sao:AccountableResult(s) relevant to installing the system as part of the deployment stage of an AI system and  which are required to be documented for accountability purposes. Installation includes integration and any configuration done afterwards (but before any users run the system during the Operation Stage). This plan is a subplan of the Deployment Stage Accountability Plan. The Accountable Actions that can be done at this stage are: Install, Configure, Provide System Input Data, Validate, Preprocess Input Data, Evaluate, and Decide.</rdfs:comment>
        <rdfs:label>Installation Accountability Plan</rdfs:label>
    </owl:Class>
    


    <!-- https://w3id.org/rains#InstallationLog -->


    <owl:Class rdf:about="https://w3id.org/rains#InstallationLog">
        <rdfs:subClassOf rdf:resource="https://w3id.org/rains#Log"/>
        <rdfs:subClassOf>
            <owl:Restriction>
                <owl:onProperty rdf:resource="https://w3id.org/ep-plan#isElementOfPlan"/>
                <owl:allValuesFrom>
                    <owl:Class>
                        <owl:unionOf rdf:parseType="Collection">
                            <rdf:Description rdf:about="https://w3id.org/rains#DeploymentStageAccountabilityPlan"/>
                            <rdf:Description rdf:about="https://w3id.org/rains#InstallationAccountabilityPlan"/>
                        </owl:unionOf>
                    </owl:Class>
                </owl:allValuesFrom>
            </owl:Restriction>
        </rdfs:subClassOf>
        <rdfs:subClassOf>
            <owl:Restriction>
                <owl:onProperty rdf:resource="https://w3id.org/ep-plan#isOutputVariableOf"/>
                <owl:allValuesFrom rdf:resource="https://w3id.org/rains#Install"/>
            </owl:Restriction>
        </rdfs:subClassOf>
        <rdfs:subClassOf>
            <owl:Restriction>
                <owl:onProperty rdf:resource="https://w3id.org/ep-plan#isVariableOfPlan"/>
                <owl:allValuesFrom>
                    <owl:Class>
                        <owl:unionOf rdf:parseType="Collection">
                            <rdf:Description rdf:about="https://w3id.org/rains#DeploymentStageAccountabilityPlan"/>
                            <rdf:Description rdf:about="https://w3id.org/rains#InstallationAccountabilityPlan"/>
                        </owl:unionOf>
                    </owl:Class>
                </owl:allValuesFrom>
            </owl:Restriction>
        </rdfs:subClassOf>
        <rdfs:comment>A specific type of planned Log that describes how the AI system installation (and related integration and configuration) was done during the Deployment Stage.</rdfs:comment>
        <rdfs:label>Installation Log</rdfs:label>
    </owl:Class>
    


    <!-- https://w3id.org/rains#IntendedUseCase -->


    <owl:Class rdf:about="https://w3id.org/rains#IntendedUseCase">
        <rdfs:subClassOf rdf:resource="https://w3id.org/rains#UseCase"/>
        <rdfs:comment>A type of :UseCase detailing a situation in which any component of :AI_System or the system as whole is expected to be used.</rdfs:comment>
        <rdfs:label>Intended Use Case</rdfs:label>
    </owl:Class>
    


    <!-- https://w3id.org/rains#IntendedUserGroup -->


    <owl:Class rdf:about="https://w3id.org/rains#IntendedUserGroup">
        <rdfs:subClassOf rdf:resource="https://w3id.org/sao#InformationElement"/>
        <rdfs:comment>A sao:InformationElement  which records a specific piece of  information detailing the target user audience for the functionality of the overall :AI_System or the components used to develop such system (e.g., a reused public training dataset or a model would be associated with this information).</rdfs:comment>
        <rdfs:label>Intended User Group</rdfs:label>
    </owl:Class>
    


    <!-- https://w3id.org/rains#Justify -->


    <owl:Class rdf:about="https://w3id.org/rains#Justify">
        <rdfs:subClassOf rdf:resource="https://w3id.org/rains#SystemAction"/>
        <rdfs:subClassOf>
            <owl:Restriction>
                <owl:onProperty rdf:resource="https://w3id.org/ep-plan#hasOutputVariable"/>
                <owl:allValuesFrom rdf:resource="https://w3id.org/rains#ChangeLog"/>
            </owl:Restriction>
        </rdfs:subClassOf>
        <rdfs:subClassOf>
            <owl:Restriction>
                <owl:onProperty rdf:resource="https://w3id.org/ep-plan#isElementOfPlan"/>
                <owl:allValuesFrom>
                    <owl:Class>
                        <owl:unionOf rdf:parseType="Collection">
                            <rdf:Description rdf:about="https://w3id.org/rains#OperationStageAccountabilityPlan"/>
                            <rdf:Description rdf:about="https://w3id.org/rains#RuntimeAccountabilityPlan"/>
                        </owl:unionOf>
                    </owl:Class>
                </owl:allValuesFrom>
            </owl:Restriction>
        </rdfs:subClassOf>
        <rdfs:subClassOf>
            <owl:Restriction>
                <owl:onProperty rdf:resource="https://w3id.org/ep-plan#isStepOfPlan"/>
                <owl:allValuesFrom>
                    <owl:Class>
                        <owl:unionOf rdf:parseType="Collection">
                            <rdf:Description rdf:about="https://w3id.org/rains#OperationStageAccountabilityPlan"/>
                            <rdf:Description rdf:about="https://w3id.org/rains#RuntimeAccountabilityPlan"/>
                        </owl:unionOf>
                    </owl:Class>
                </owl:allValuesFrom>
            </owl:Restriction>
        </rdfs:subClassOf>
        <owl:disjointWith rdf:resource="https://w3id.org/rains#NotifyUser"/>
        <owl:disjointWith rdf:resource="https://w3id.org/rains#PreprocessInputData"/>
        <owl:disjointWith rdf:resource="https://w3id.org/rains#ProvideSystemInputData"/>
        <owl:disjointWith rdf:resource="https://w3id.org/rains#ReturnOutput"/>
        <owl:disjointWith rdf:resource="https://w3id.org/rains#Validate"/>
        <rdfs:comment>A planned step that records a user&apos;s justification to actions performed when operating the AI system, e.g. overriding a system output or a model output. This step is typically part of the Operation stage (specifically Runtime stage) and has a member of the class Change Log as its expected output.</rdfs:comment>
        <rdfs:label>Justify</rdfs:label>
    </owl:Class>
    


    <!-- https://w3id.org/rains#Limitation -->


    <owl:Class rdf:about="https://w3id.org/rains#Limitation">
        <rdfs:subClassOf rdf:resource="https://w3id.org/sao#InformationElement"/>
        <rdfs:comment>A sao:InformationElement  which records a specific piece of  information detailing the limitations of any aspect related to an :AI_System including the system as whole, its components (e.g., ML model),  or associated processes (e.g., evaluation).</rdfs:comment>
        <rdfs:label>Limitation</rdfs:label>
    </owl:Class>
    


    <!-- https://w3id.org/rains#Log -->


    <owl:Class rdf:about="https://w3id.org/rains#Log">
        <rdfs:subClassOf rdf:resource="https://w3id.org/sao#AccountableResult"/>
        <rdfs:subClassOf>
            <owl:Restriction>
                <owl:onProperty rdf:resource="https://w3id.org/ep-plan#isElementOfPlan"/>
                <owl:allValuesFrom>
                    <owl:Class>
                        <owl:unionOf rdf:parseType="Collection">
                            <rdf:Description rdf:about="https://w3id.org/rains#DeploymentStageAccountabilityPlan"/>
                            <rdf:Description rdf:about="https://w3id.org/rains#ImplementationStageAccountabilityPlan"/>
                            <rdf:Description rdf:about="https://w3id.org/rains#OperationStageAccountabilityPlan"/>
                        </owl:unionOf>
                    </owl:Class>
                </owl:allValuesFrom>
            </owl:Restriction>
        </rdfs:subClassOf>
        <rdfs:subClassOf>
            <owl:Restriction>
                <owl:onProperty rdf:resource="https://w3id.org/ep-plan#isOutputVariableOf"/>
                <owl:allValuesFrom>
                    <owl:Class>
                        <owl:unionOf rdf:parseType="Collection">
                            <rdf:Description rdf:about="https://w3id.org/rains#Aggregate"/>
                            <rdf:Description rdf:about="https://w3id.org/rains#Configure"/>
                            <rdf:Description rdf:about="https://w3id.org/rains#Evaluate"/>
                            <rdf:Description rdf:about="https://w3id.org/rains#GenerateGuideline"/>
                            <rdf:Description rdf:about="https://w3id.org/rains#Install"/>
                            <rdf:Description rdf:about="https://w3id.org/rains#Justify"/>
                            <rdf:Description rdf:about="https://w3id.org/rains#MergeAndSplitDataset"/>
                            <rdf:Description rdf:about="https://w3id.org/rains#Override"/>
                            <rdf:Description rdf:about="https://w3id.org/rains#RealizeComponent"/>
                            <rdf:Description rdf:about="https://w3id.org/rains#TrainUser"/>
                        </owl:unionOf>
                    </owl:Class>
                </owl:allValuesFrom>
            </owl:Restriction>
        </rdfs:subClassOf>
        <rdfs:subClassOf>
            <owl:Restriction>
                <owl:onProperty rdf:resource="https://w3id.org/ep-plan#isVariableOfPlan"/>
                <owl:allValuesFrom>
                    <owl:Class>
                        <owl:unionOf rdf:parseType="Collection">
                            <rdf:Description rdf:about="https://w3id.org/rains#DeploymentStageAccountabilityPlan"/>
                            <rdf:Description rdf:about="https://w3id.org/rains#ImplementationStageAccountabilityPlan"/>
                            <rdf:Description rdf:about="https://w3id.org/rains#OperationStageAccountabilityPlan"/>
                        </owl:unionOf>
                    </owl:Class>
                </owl:allValuesFrom>
            </owl:Restriction>
        </rdfs:subClassOf>
        <owl:disjointWith rdf:resource="https://w3id.org/rains#ModelComponent"/>
        <owl:disjointWith rdf:resource="https://w3id.org/rains#SupportingInfrastructureComponent"/>
        <owl:disjointWith rdf:resource="https://w3id.org/rains#SystemData"/>
        <owl:disjointWith rdf:resource="https://w3id.org/rains#UserTrainingReport"/>
        <rdfs:comment>A specific type of planned sao:AccountableResult which represents a high level reference to logs of information pertaining either to Installation or Changes. This class has two subclasses: Installation Log and Change Log.The former is the result of the installation taking place during the Deployment stage (specifically Installation stage), and the latter of reflects changes which occur throughtout the Implementation, Deployment, and Operation Stages.</rdfs:comment>
        <rdfs:label>Log</rdfs:label>
    </owl:Class>
    


    <!-- https://w3id.org/rains#MaintenanceAccountabilityPlan -->


    <owl:Class rdf:about="https://w3id.org/rains#MaintenanceAccountabilityPlan">
        <rdfs:subClassOf rdf:resource="https://w3id.org/rains#OperationStageAccountabilityPlan"/>
        <rdfs:comment>A plan that identifies sao:AccountableAction(s) and sao:AccountableResult(s) relevant to performing routine maintenance evaluations on  the system as part of the operation stage of an AI system and  which are required to be documented for accountability purposes. This plan is a subplan of the Operation Stage Accountability Plan.
The Accountable Actions that can be done at this stage are: Evaluate and Decide.</rdfs:comment>
        <rdfs:label>Maintenance Accountability Plan</rdfs:label>
    </owl:Class>
    


    <!-- https://w3id.org/rains#ManualProductionAccountabilityPlan -->


    <owl:Class rdf:about="https://w3id.org/rains#ManualProductionAccountabilityPlan">
        <rdfs:subClassOf rdf:resource="https://w3id.org/rains#DeploymentStageAccountabilityPlan"/>
        <rdfs:comment>A plan that identifies sao:AccountableAction(s) and sao:AccountableResult(s) relevant to the producing manuals for usage and maintenance as part of the deployment stage of an AI system and  which are required to be documented for accountability purposes. This plan is a subplan of the Deployment Stage Accountability Plan. The Accountable Actions that can be done at this stage are: Generate Guideline and Decide.</rdfs:comment>
        <rdfs:label>Manual Production Accountability Plan</rdfs:label>
    </owl:Class>
    


    <!-- https://w3id.org/rains#MergeAndSplitDataset -->


    <owl:Class rdf:about="https://w3id.org/rains#MergeAndSplitDataset">
        <rdfs:subClassOf rdf:resource="https://w3id.org/sao#AccountableAction"/>
        <rdfs:subClassOf>
            <owl:Restriction>
                <owl:onProperty rdf:resource="https://w3id.org/ep-plan#hasOutputVariable"/>
                <owl:allValuesFrom>
                    <owl:Class>
                        <owl:unionOf rdf:parseType="Collection">
                            <rdf:Description rdf:about="https://w3id.org/rains#ChangeLog"/>
                            <rdf:Description rdf:about="https://w3id.org/rains#DatasetComponent"/>
                            <rdf:Description rdf:about="https://w3id.org/rains#EvaluationDataset"/>
                            <rdf:Description rdf:about="https://w3id.org/rains#TrainingDataset"/>
                            <rdf:Description rdf:about="https://w3id.org/rains#ValidationDataset"/>
                        </owl:unionOf>
                    </owl:Class>
                </owl:allValuesFrom>
            </owl:Restriction>
        </rdfs:subClassOf>
        <rdfs:subClassOf>
            <owl:Restriction>
                <owl:onProperty rdf:resource="https://w3id.org/ep-plan#isElementOfPlan"/>
                <owl:allValuesFrom rdf:resource="https://w3id.org/rains#ImplementationStageAccountabilityPlan"/>
            </owl:Restriction>
        </rdfs:subClassOf>
        <rdfs:subClassOf>
            <owl:Restriction>
                <owl:onProperty rdf:resource="https://w3id.org/ep-plan#isStepOfPlan"/>
                <owl:allValuesFrom rdf:resource="https://w3id.org/rains#ImplementationStageAccountabilityPlan"/>
            </owl:Restriction>
        </rdfs:subClassOf>
        <owl:disjointWith rdf:resource="https://w3id.org/rains#ProduceSpecification"/>
        <owl:disjointWith rdf:resource="https://w3id.org/rains#RealizeComponent"/>
        <owl:disjointWith rdf:resource="https://w3id.org/rains#SystemAction"/>
        <owl:disjointWith rdf:resource="https://w3id.org/rains#TrainUser"/>
        <rdfs:comment>A planned step that has some impact on the AI System where the dataset(s) used to produce the ML Model are merged and/or split. Merging takes place when there is more than one dataset in use. Typically, splitting a dataset component results in three subsets: Training Dataset, Validation Dataset, and Testing Dataset. This step is typically part of the Implementation stage of an AI System&apos;s life cycle. If a deviation from the design specification takes place, then the step will also have as an output a member of the class Change Log.</rdfs:comment>
        <rdfs:label>Merge and Split Dataset</rdfs:label>
    </owl:Class>
    


    <!-- https://w3id.org/rains#ModelComponent -->


    <owl:Class rdf:about="https://w3id.org/rains#ModelComponent">
        <rdfs:subClassOf rdf:resource="https://w3id.org/sao#AccountableResult"/>
        <rdfs:subClassOf>
            <owl:Restriction>
                <owl:onProperty rdf:resource="https://w3id.org/ep-plan#isElementOfPlan"/>
                <owl:allValuesFrom>
                    <owl:Class>
                        <owl:unionOf rdf:parseType="Collection">
                            <rdf:Description rdf:about="https://w3id.org/rains#ConfigurationAccountabilityPlan"/>
                            <rdf:Description rdf:about="https://w3id.org/rains#DeploymentStageAccountabilityPlan"/>
                            <rdf:Description rdf:about="https://w3id.org/rains#ImplementationStageAccountabilityPlan"/>
                            <rdf:Description rdf:about="https://w3id.org/rains#InstallationAccountabilityPlan"/>
                            <rdf:Description rdf:about="https://w3id.org/rains#MaintenanceAccountabilityPlan"/>
                            <rdf:Description rdf:about="https://w3id.org/rains#OperationStageAccountabilityPlan"/>
                            <rdf:Description rdf:about="https://w3id.org/rains#RuntimeAccountabilityPlan"/>
                        </owl:unionOf>
                    </owl:Class>
                </owl:allValuesFrom>
            </owl:Restriction>
        </rdfs:subClassOf>
        <rdfs:subClassOf>
            <owl:Restriction>
                <owl:onProperty rdf:resource="https://w3id.org/ep-plan#isOutputVariableOf"/>
                <owl:allValuesFrom>
                    <owl:Class>
                        <owl:unionOf rdf:parseType="Collection">
                            <rdf:Description rdf:about="https://w3id.org/rains#Configure"/>
                            <rdf:Description rdf:about="https://w3id.org/rains#Install"/>
                            <rdf:Description rdf:about="https://w3id.org/rains#RealizeComponent"/>
                        </owl:unionOf>
                    </owl:Class>
                </owl:allValuesFrom>
            </owl:Restriction>
        </rdfs:subClassOf>
        <rdfs:subClassOf>
            <owl:Restriction>
                <owl:onProperty rdf:resource="https://w3id.org/ep-plan#isVariableOfPlan"/>
                <owl:allValuesFrom>
                    <owl:Class>
                        <owl:unionOf rdf:parseType="Collection">
                            <rdf:Description rdf:about="https://w3id.org/rains#ConfigurationAccountabilityPlan"/>
                            <rdf:Description rdf:about="https://w3id.org/rains#DeploymentStageAccountabilityPlan"/>
                            <rdf:Description rdf:about="https://w3id.org/rains#ImplementationStageAccountabilityPlan"/>
                            <rdf:Description rdf:about="https://w3id.org/rains#InstallationAccountabilityPlan"/>
                            <rdf:Description rdf:about="https://w3id.org/rains#MaintenanceAccountabilityPlan"/>
                            <rdf:Description rdf:about="https://w3id.org/rains#OperationStageAccountabilityPlan"/>
                            <rdf:Description rdf:about="https://w3id.org/rains#RuntimeAccountabilityPlan"/>
                        </owl:unionOf>
                    </owl:Class>
                </owl:allValuesFrom>
            </owl:Restriction>
        </rdfs:subClassOf>
        <owl:disjointWith rdf:resource="https://w3id.org/rains#SupportingInfrastructureComponent"/>
        <owl:disjointWith rdf:resource="https://w3id.org/rains#SystemData"/>
        <owl:disjointWith rdf:resource="https://w3id.org/rains#UserTrainingReport"/>
        <rdfs:comment>A specific type of planned sao:AccountableResult which represents the description of a realized ML Model, including it characteristics, performance, etc.

It is advisable that the information realization corresponding to the ModelComponent variable contains the following information elements:
1. Model: the realized model should be an instance of RealizedObject. If the implementation deviates from the design, then an additional model should be indicated as an instance of ExcludedObject. 
2. ModelCharacteristic
3. Algorithm
4. Limitation
5. Risk and its subclass Bias
6.Tradeoff
7. IntendedUserGroup
8. Parameter and its subclass Hyperparameter
9. The subclasses of Use Case, namely IncorrectUseCase and IntendedUseCase
10. The subclasses of Compliance Entity, namely, Hard Law and SoftLaw 
11. LicenseDocument
 12. Funding

It is discouraged that the information realization corresponding to the ModelComponent variable contains the following information elements:
1. The following subclasses of Realizable Object Characteristic: SystemAuditMechanism, SystemExplanationMechanism, System Feedback from User Mechanism, System Human Oversight Mechanism, and SystemSecurityMechanism
2. The subclasses of Guidance, namely, System Deployment Guidance, SystemInstallationGuidance, UserTrainingGuidance, SystemOperationGuidance, SystemUsageGuidance, and SystemMaintenanceGuidance
3. Notification Proof</rdfs:comment>
        <rdfs:label>Model Component</rdfs:label>
    </owl:Class>
    


    <!-- https://w3id.org/rains#ModelOutput -->


    <owl:Class rdf:about="https://w3id.org/rains#ModelOutput">
        <rdfs:subClassOf rdf:resource="https://w3id.org/rains#SystemOutput"/>
        <rdfs:subClassOf>
            <owl:Restriction>
                <owl:onProperty rdf:resource="https://w3id.org/ep-plan#isElementOfPlan"/>
                <owl:allValuesFrom>
                    <owl:Class>
                        <owl:unionOf rdf:parseType="Collection">
                            <rdf:Description rdf:about="https://w3id.org/rains#ConfigurationAccountabilityPlan"/>
                            <rdf:Description rdf:about="https://w3id.org/rains#DeploymentStageAccountabilityPlan"/>
                            <rdf:Description rdf:about="https://w3id.org/rains#InstallationAccountabilityPlan"/>
                            <rdf:Description rdf:about="https://w3id.org/rains#OperationStageAccountabilityPlan"/>
                            <rdf:Description rdf:about="https://w3id.org/rains#RuntimeAccountabilityPlan"/>
                        </owl:unionOf>
                    </owl:Class>
                </owl:allValuesFrom>
            </owl:Restriction>
        </rdfs:subClassOf>
        <rdfs:subClassOf>
            <owl:Restriction>
                <owl:onProperty rdf:resource="https://w3id.org/ep-plan#isOutputVariableOf"/>
                <owl:allValuesFrom rdf:resource="https://w3id.org/rains#GenerateModelOutput"/>
            </owl:Restriction>
        </rdfs:subClassOf>
        <rdfs:subClassOf>
            <owl:Restriction>
                <owl:onProperty rdf:resource="https://w3id.org/ep-plan#isVariableOfPlan"/>
                <owl:allValuesFrom>
                    <owl:Class>
                        <owl:unionOf rdf:parseType="Collection">
                            <rdf:Description rdf:about="https://w3id.org/rains#ConfigurationAccountabilityPlan"/>
                            <rdf:Description rdf:about="https://w3id.org/rains#DeploymentStageAccountabilityPlan"/>
                            <rdf:Description rdf:about="https://w3id.org/rains#InstallationAccountabilityPlan"/>
                            <rdf:Description rdf:about="https://w3id.org/rains#OperationStageAccountabilityPlan"/>
                            <rdf:Description rdf:about="https://w3id.org/rains#RuntimeAccountabilityPlan"/>
                        </owl:unionOf>
                    </owl:Class>
                </owl:allValuesFrom>
            </owl:Restriction>
        </rdfs:subClassOf>
        <owl:disjointWith rdf:resource="https://w3id.org/rains#OverrideResult"/>
        <rdfs:comment>A specific type of planned System Output which describes an output generated by a Model Component. This does not represent explanations, so if the Model Component can also generate its own explanation for its outputs, then this Model compoenent will generate both a Model Output and an Explanation.

If the AI System is involved in making decisions/recommendations/actions affecting human users, then it is advisable that the information realization corresponding to the Model Output variable contains the following information elements: Affected Agent.</rdfs:comment>
        <rdfs:label>Model Output</rdfs:label>
    </owl:Class>
    


    <!-- https://w3id.org/rains#ModelSpecification -->


    <owl:Class rdf:about="https://w3id.org/rains#ModelSpecification">
        <rdfs:subClassOf rdf:resource="https://w3id.org/rains#DesignSpecification"/>
        <rdfs:subClassOf>
            <owl:Restriction>
                <owl:onProperty rdf:resource="https://w3id.org/ep-plan#isElementOfPlan"/>
                <owl:allValuesFrom>
                    <owl:Class>
                        <owl:unionOf rdf:parseType="Collection">
                            <rdf:Description rdf:about="https://w3id.org/rains#DesignStageAccountabilityPlan"/>
                            <rdf:Description rdf:about="https://w3id.org/rains#ImplementationStageAccountabilityPlan"/>
                        </owl:unionOf>
                    </owl:Class>
                </owl:allValuesFrom>
            </owl:Restriction>
        </rdfs:subClassOf>
        <rdfs:subClassOf>
            <owl:Restriction>
                <owl:onProperty rdf:resource="https://w3id.org/ep-plan#isOutputVariableOf"/>
                <owl:allValuesFrom rdf:resource="https://w3id.org/rains#ProduceSpecification"/>
            </owl:Restriction>
        </rdfs:subClassOf>
        <rdfs:subClassOf>
            <owl:Restriction>
                <owl:onProperty rdf:resource="https://w3id.org/ep-plan#isVariableOfPlan"/>
                <owl:allValuesFrom>
                    <owl:Class>
                        <owl:unionOf rdf:parseType="Collection">
                            <rdf:Description rdf:about="https://w3id.org/rains#DesignStageAccountabilityPlan"/>
                            <rdf:Description rdf:about="https://w3id.org/rains#ImplementationStageAccountabilityPlan"/>
                        </owl:unionOf>
                    </owl:Class>
                </owl:allValuesFrom>
            </owl:Restriction>
        </rdfs:subClassOf>
        <owl:disjointWith rdf:resource="https://w3id.org/rains#SupportingInfrastructureSpecification"/>
        <owl:disjointWith rdf:resource="https://w3id.org/rains#SystemPurposeSpecification"/>
        <rdfs:comment>A specific type of design specification  which represents the description of planned requirements, characteristics, performance, etc. related to an AI model.

It is advisable that the information realization corresponding to ModelSpecification contains the following information elements:
1. Model 
2. ModelCharacteristic
3. Algorithm
4. Limitation
5. Risk and its subclass Bias, and if applicable FairnessOrBiasDetectionSoftware
6.Tradeoff
7. IntendedUserGroup
8. Parameter and its subclass Hyperparameter
9. The subclasses of Use Case, namely IncorrectUseCase and IntendedUseCase
10. The subclasses of Compliance Entity, namely, Hard Law and SoftLaw
11. LicenseDocument
12. Funding

It is discouraged that the information realization corresponding to the ModelSpecification contains the following information elements:
1. The following subclasses of Realizable Object Characteristic: SystemAuditMechanism, SystemExplanationMechanism, System Feedback from User Mechanism, System Human Oversight Mechanism, and SystemSecurityMechanism
2. The subclasses of Guidance, namely, System Deployment Guidance, SystemInstallationGuidance, UserTrainingGuidance, SystemOperationGuidance, SystemUsageGuidance, and SystemMaintenanceGuidance
3. Notification Proof
4. Installation Log</rdfs:comment>
        <rdfs:label>Model Specification</rdfs:label>
    </owl:Class>
    


    <!-- https://w3id.org/rains#Notification -->


    <owl:Class rdf:about="https://w3id.org/rains#Notification">
        <rdfs:subClassOf rdf:resource="https://w3id.org/rains#SystemData"/>
        <rdfs:subClassOf>
            <owl:Restriction>
                <owl:onProperty rdf:resource="https://w3id.org/ep-plan#isElementOfPlan"/>
                <owl:allValuesFrom>
                    <owl:Class>
                        <owl:unionOf rdf:parseType="Collection">
                            <rdf:Description rdf:about="https://w3id.org/rains#ConfigurationAccountabilityPlan"/>
                            <rdf:Description rdf:about="https://w3id.org/rains#DeploymentStageAccountabilityPlan"/>
                            <rdf:Description rdf:about="https://w3id.org/rains#InstallationAccountabilityPlan"/>
                            <rdf:Description rdf:about="https://w3id.org/rains#OperationStageAccountabilityPlan"/>
                            <rdf:Description rdf:about="https://w3id.org/rains#RuntimeAccountabilityPlan"/>
                        </owl:unionOf>
                    </owl:Class>
                </owl:allValuesFrom>
            </owl:Restriction>
        </rdfs:subClassOf>
        <rdfs:subClassOf>
            <owl:Restriction>
                <owl:onProperty rdf:resource="https://w3id.org/ep-plan#isOutputVariableOf"/>
                <owl:allValuesFrom rdf:resource="https://w3id.org/rains#NotifyUser"/>
            </owl:Restriction>
        </rdfs:subClassOf>
        <rdfs:subClassOf>
            <owl:Restriction>
                <owl:onProperty rdf:resource="https://w3id.org/ep-plan#isVariableOfPlan"/>
                <owl:allValuesFrom>
                    <owl:Class>
                        <owl:unionOf rdf:parseType="Collection">
                            <rdf:Description rdf:about="https://w3id.org/rains#ConfigurationAccountabilityPlan"/>
                            <rdf:Description rdf:about="https://w3id.org/rains#DeploymentStageAccountabilityPlan"/>
                            <rdf:Description rdf:about="https://w3id.org/rains#InstallationAccountabilityPlan"/>
                            <rdf:Description rdf:about="https://w3id.org/rains#OperationStageAccountabilityPlan"/>
                            <rdf:Description rdf:about="https://w3id.org/rains#RuntimeAccountabilityPlan"/>
                        </owl:unionOf>
                    </owl:Class>
                </owl:allValuesFrom>
            </owl:Restriction>
        </rdfs:subClassOf>
        <owl:disjointWith rdf:resource="https://w3id.org/rains#RuntimeInputData"/>
        <owl:disjointWith rdf:resource="https://w3id.org/rains#SystemOutput"/>
        <owl:disjointWith rdf:resource="https://w3id.org/rains#UserConsent"/>
        <owl:disjointWith rdf:resource="https://w3id.org/rains#UserReview"/>
        <owl:disjointWith rdf:resource="https://w3id.org/rains#Validation"/>
        <rdfs:comment>A specific type of planned System Data which describes a notification presented to the user of the AI System. This class has three subclasses: Disclaimer Notification, Error Notification, and Explanation Notification.

It is advisable that the information realization corresponding to the Notification variable contains the following information elements:
1. Affected Agent, describing the user who was notified.
2. Notification Proof, documenting how the user was notified, e.g. a screenshot of the a disclaimer shown to the user.</rdfs:comment>
        <rdfs:label>Notification</rdfs:label>
    </owl:Class>
    


    <!-- https://w3id.org/rains#NotificationProof -->


    <owl:Class rdf:about="https://w3id.org/rains#NotificationProof">
        <rdfs:subClassOf rdf:resource="https://w3id.org/sao#InformationElement"/>
        <rdfs:comment>A sao:InformnationElement which records information describing the proof of a notification delivered to the user of the AI System, e.g. a screenshots of the a displayed diclaimer.</rdfs:comment>
        <rdfs:label>Notification Proof</rdfs:label>
    </owl:Class>
    


    <!-- https://w3id.org/rains#NotifyUser -->


    <owl:Class rdf:about="https://w3id.org/rains#NotifyUser">
        <rdfs:subClassOf rdf:resource="https://w3id.org/rains#SystemAction"/>
        <rdfs:subClassOf>
            <owl:Restriction>
                <owl:onProperty rdf:resource="https://w3id.org/ep-plan#hasOutputVariable"/>
                <owl:allValuesFrom>
                    <owl:Class>
                        <owl:unionOf rdf:parseType="Collection">
                            <rdf:Description rdf:about="https://w3id.org/rains#DisclaimerNotification"/>
                            <rdf:Description rdf:about="https://w3id.org/rains#ErrorNotification"/>
                            <rdf:Description rdf:about="https://w3id.org/rains#ExplanationNotification"/>
                            <rdf:Description rdf:about="https://w3id.org/rains#Notification"/>
                        </owl:unionOf>
                    </owl:Class>
                </owl:allValuesFrom>
            </owl:Restriction>
        </rdfs:subClassOf>
        <rdfs:subClassOf>
            <owl:Restriction>
                <owl:onProperty rdf:resource="https://w3id.org/ep-plan#isElementOfPlan"/>
                <owl:allValuesFrom>
                    <owl:Class>
                        <owl:unionOf rdf:parseType="Collection">
                            <rdf:Description rdf:about="https://w3id.org/rains#ConfigurationAccountabilityPlan"/>
                            <rdf:Description rdf:about="https://w3id.org/rains#OperationStageAccountabilityPlan"/>
                            <rdf:Description rdf:about="https://w3id.org/rains#RuntimeAccountabilityPlan"/>
                        </owl:unionOf>
                    </owl:Class>
                </owl:allValuesFrom>
            </owl:Restriction>
        </rdfs:subClassOf>
        <rdfs:subClassOf>
            <owl:Restriction>
                <owl:onProperty rdf:resource="https://w3id.org/ep-plan#isStepOfPlan"/>
                <owl:allValuesFrom>
                    <owl:Class>
                        <owl:unionOf rdf:parseType="Collection">
                            <rdf:Description rdf:about="https://w3id.org/rains#ConfigurationAccountabilityPlan"/>
                            <rdf:Description rdf:about="https://w3id.org/rains#OperationStageAccountabilityPlan"/>
                            <rdf:Description rdf:about="https://w3id.org/rains#RuntimeAccountabilityPlan"/>
                        </owl:unionOf>
                    </owl:Class>
                </owl:allValuesFrom>
            </owl:Restriction>
        </rdfs:subClassOf>
        <owl:disjointWith rdf:resource="https://w3id.org/rains#PreprocessInputData"/>
        <owl:disjointWith rdf:resource="https://w3id.org/rains#ProvideSystemInputData"/>
        <owl:disjointWith rdf:resource="https://w3id.org/rains#ReturnOutput"/>
        <owl:disjointWith rdf:resource="https://w3id.org/rains#Validate"/>
        <rdfs:comment>A planned step that reords that the AI system&apos;s user has been provided a certain notification, e.g. disclaimer that they are using an AI system or a notification of an error. This step is typically part of the Operation stage (specifically Configuration or Runtime stages) and has a member of the subclasses of Notification as its expected output.</rdfs:comment>
        <rdfs:label>Notify User</rdfs:label>
    </owl:Class>
    


    <!-- https://w3id.org/rains#OperationStageAccountabilityPlan -->


    <owl:Class rdf:about="https://w3id.org/rains#OperationStageAccountabilityPlan">
        <rdfs:subClassOf rdf:resource="https://w3id.org/sao#AccountabilityPlan"/>
        <rdfs:comment>A plan that identifies sao:AccountableAction(s) and sao:AccountableResult(s) relevant to the operation stage of an AI system and  which are required to be documented for accountability purposes. This plan may be split into one of three sub-plans: Configuration Accountability Plan, Runtime Accountability Plan, and Maintenance Accountability Plan. The Accountable Actions that can be done at this stage are: Notify User, Consent, Provide System Input Data, Preprocess Input Data, Validate, Configure, Generate Model Output, Explain, Generate Output, Aggregate,  Override, Justify,  Approve Output, Return Output, Actuate Output, Collect User Feedback, Evaluate and Decide.</rdfs:comment>
        <rdfs:label>Operation Stage Accountability Plan</rdfs:label>
    </owl:Class>
    


    <!-- https://w3id.org/rains#Override -->


    <owl:Class rdf:about="https://w3id.org/rains#Override">
        <rdfs:subClassOf rdf:resource="https://w3id.org/rains#GenerateOutput"/>
        <rdfs:subClassOf>
            <owl:Restriction>
                <owl:onProperty rdf:resource="https://w3id.org/ep-plan#hasOutputVariable"/>
                <owl:allValuesFrom rdf:resource="https://w3id.org/rains#OverrideResult"/>
            </owl:Restriction>
        </rdfs:subClassOf>
        <rdfs:subClassOf>
            <owl:Restriction>
                <owl:onProperty rdf:resource="https://w3id.org/ep-plan#isElementOfPlan"/>
                <owl:allValuesFrom>
                    <owl:Class>
                        <owl:unionOf rdf:parseType="Collection">
                            <rdf:Description rdf:about="https://w3id.org/rains#OperationStageAccountabilityPlan"/>
                            <rdf:Description rdf:about="https://w3id.org/rains#RuntimeAccountabilityPlan"/>
                        </owl:unionOf>
                    </owl:Class>
                </owl:allValuesFrom>
            </owl:Restriction>
        </rdfs:subClassOf>
        <rdfs:subClassOf>
            <owl:Restriction>
                <owl:onProperty rdf:resource="https://w3id.org/ep-plan#isStepOfPlan"/>
                <owl:allValuesFrom>
                    <owl:Class>
                        <owl:unionOf rdf:parseType="Collection">
                            <rdf:Description rdf:about="https://w3id.org/rains#OperationStageAccountabilityPlan"/>
                            <rdf:Description rdf:about="https://w3id.org/rains#RuntimeAccountabilityPlan"/>
                        </owl:unionOf>
                    </owl:Class>
                </owl:allValuesFrom>
            </owl:Restriction>
        </rdfs:subClassOf>
        <rdfs:comment>A planned step that has some impact on the output of AI System where a user or a system component overrides some output. This step is typically part of the Operation stage (specifically Runtime Stage) and has a member of the class Override Result as its expected output. Note that this step is not related to the Decide step (which may have a member of the class Approval Decision as its expected output).</rdfs:comment>
        <rdfs:label>Override</rdfs:label>
    </owl:Class>
    


    <!-- https://w3id.org/rains#OverrideResult -->


    <owl:Class rdf:about="https://w3id.org/rains#OverrideResult">
        <rdfs:subClassOf rdf:resource="https://w3id.org/rains#SystemOutput"/>
        <rdfs:subClassOf>
            <owl:Restriction>
                <owl:onProperty rdf:resource="https://w3id.org/ep-plan#isElementOfPlan"/>
                <owl:allValuesFrom>
                    <owl:Class>
                        <owl:unionOf rdf:parseType="Collection">
                            <rdf:Description rdf:about="https://w3id.org/rains#OperationStageAccountabilityPlan"/>
                            <rdf:Description rdf:about="https://w3id.org/rains#RuntimeAccountabilityPlan"/>
                        </owl:unionOf>
                    </owl:Class>
                </owl:allValuesFrom>
            </owl:Restriction>
        </rdfs:subClassOf>
        <rdfs:subClassOf>
            <owl:Restriction>
                <owl:onProperty rdf:resource="https://w3id.org/ep-plan#isOutputVariableOf"/>
                <owl:allValuesFrom rdf:resource="https://w3id.org/rains#Override"/>
            </owl:Restriction>
        </rdfs:subClassOf>
        <rdfs:subClassOf>
            <owl:Restriction>
                <owl:onProperty rdf:resource="https://w3id.org/ep-plan#isVariableOfPlan"/>
                <owl:allValuesFrom>
                    <owl:Class>
                        <owl:unionOf rdf:parseType="Collection">
                            <rdf:Description rdf:about="https://w3id.org/rains#OperationStageAccountabilityPlan"/>
                            <rdf:Description rdf:about="https://w3id.org/rains#RuntimeAccountabilityPlan"/>
                        </owl:unionOf>
                    </owl:Class>
                </owl:allValuesFrom>
            </owl:Restriction>
        </rdfs:subClassOf>
        <rdfs:comment>A specific type of planned System Output which describes the results of overriding outputs produced by Model component(s) or Supporting Infrastrcuture component(s).

If the AI System is involved in making decisions/recommendations/actions affecting human users, then it is advisable that the information realization corresponding to the Override Result variable contains the following information elements: Affected Agent.</rdfs:comment>
        <rdfs:label>Override Result</rdfs:label>
    </owl:Class>
    


    <!-- https://w3id.org/rains#Parameter -->


    <owl:Class rdf:about="https://w3id.org/rains#Parameter">
        <rdfs:subClassOf rdf:resource="https://w3id.org/sao#InformationElement"/>
        <rdfs:comment>A  sao:InformationElement which records a specific piece of  information describing a model&apos;s parameter. This is broader than mls:HyperParameter which describes only a hyperparameter of a model.</rdfs:comment>
        <rdfs:label>Parameter</rdfs:label>
    </owl:Class>
    


    <!-- https://w3id.org/rains#PreprocessInputData -->


    <owl:Class rdf:about="https://w3id.org/rains#PreprocessInputData">
        <rdfs:subClassOf rdf:resource="https://w3id.org/rains#SystemAction"/>
        <rdfs:subClassOf>
            <owl:Restriction>
                <owl:onProperty rdf:resource="https://w3id.org/ep-plan#hasOutputVariable"/>
                <owl:allValuesFrom>
                    <owl:Class>
                        <owl:unionOf rdf:parseType="Collection">
                            <rdf:Description rdf:about="https://w3id.org/rains#ConfigurationData"/>
                            <rdf:Description rdf:about="https://w3id.org/rains#RuntimeInputData"/>
                        </owl:unionOf>
                    </owl:Class>
                </owl:allValuesFrom>
            </owl:Restriction>
        </rdfs:subClassOf>
        <rdfs:subClassOf>
            <owl:Restriction>
                <owl:onProperty rdf:resource="https://w3id.org/ep-plan#isElementOfPlan"/>
                <owl:allValuesFrom>
                    <owl:Class>
                        <owl:unionOf rdf:parseType="Collection">
                            <rdf:Description rdf:about="https://w3id.org/rains#ConfigurationAccountabilityPlan"/>
                            <rdf:Description rdf:about="https://w3id.org/rains#DeploymentStageAccountabilityPlan"/>
                            <rdf:Description rdf:about="https://w3id.org/rains#InstallationAccountabilityPlan"/>
                            <rdf:Description rdf:about="https://w3id.org/rains#OperationStageAccountabilityPlan"/>
                            <rdf:Description rdf:about="https://w3id.org/rains#RuntimeAccountabilityPlan"/>
                        </owl:unionOf>
                    </owl:Class>
                </owl:allValuesFrom>
            </owl:Restriction>
        </rdfs:subClassOf>
        <rdfs:subClassOf>
            <owl:Restriction>
                <owl:onProperty rdf:resource="https://w3id.org/ep-plan#isStepOfPlan"/>
                <owl:allValuesFrom>
                    <owl:Class>
                        <owl:unionOf rdf:parseType="Collection">
                            <rdf:Description rdf:about="https://w3id.org/rains#ConfigurationAccountabilityPlan"/>
                            <rdf:Description rdf:about="https://w3id.org/rains#DeploymentStageAccountabilityPlan"/>
                            <rdf:Description rdf:about="https://w3id.org/rains#InstallationAccountabilityPlan"/>
                            <rdf:Description rdf:about="https://w3id.org/rains#OperationStageAccountabilityPlan"/>
                            <rdf:Description rdf:about="https://w3id.org/rains#RuntimeAccountabilityPlan"/>
                        </owl:unionOf>
                    </owl:Class>
                </owl:allValuesFrom>
            </owl:Restriction>
        </rdfs:subClassOf>
        <owl:disjointWith rdf:resource="https://w3id.org/rains#ProvideSystemInputData"/>
        <owl:disjointWith rdf:resource="https://w3id.org/rains#ReturnOutput"/>
        <owl:disjointWith rdf:resource="https://w3id.org/rains#Validate"/>
        <rdfs:comment>A planned step that has some impact on the output of AI System where the input data provided to the AI system is preprocessed by a Supporting Infrastructure component. This step is typically part of the Deployment or Operation stages (specifically Installation, Configuration, or Runtime stages). Depending on whether the data was configuration data or runtime data, the output of this step is either Configuration data or Runtime Input Data.</rdfs:comment>
        <rdfs:label>Preprocess Input Data</rdfs:label>
    </owl:Class>
    


    <!-- https://w3id.org/rains#ProduceSpecification -->


    <owl:Class rdf:about="https://w3id.org/rains#ProduceSpecification">
        <rdfs:subClassOf rdf:resource="https://w3id.org/sao#AccountableAction"/>
        <rdfs:subClassOf>
            <owl:Restriction>
                <owl:onProperty rdf:resource="https://w3id.org/ep-plan#hasOutputVariable"/>
                <owl:allValuesFrom>
                    <owl:Class>
                        <owl:unionOf rdf:parseType="Collection">
                            <rdf:Description rdf:about="https://w3id.org/rains#ComplianceSpecification"/>
                            <rdf:Description rdf:about="https://w3id.org/rains#DatasetSpecification"/>
                            <rdf:Description rdf:about="https://w3id.org/rains#DesignSpecification"/>
                            <rdf:Description rdf:about="https://w3id.org/rains#EvaluationSpecification"/>
                            <rdf:Description rdf:about="https://w3id.org/rains#ModelSpecification"/>
                            <rdf:Description rdf:about="https://w3id.org/rains#SupportingInfrastructureSpecification"/>
                            <rdf:Description rdf:about="https://w3id.org/rains#SystemPurposeSpecification"/>
                        </owl:unionOf>
                    </owl:Class>
                </owl:allValuesFrom>
            </owl:Restriction>
        </rdfs:subClassOf>
        <rdfs:subClassOf>
            <owl:Restriction>
                <owl:onProperty rdf:resource="https://w3id.org/ep-plan#isElementOfPlan"/>
                <owl:allValuesFrom>
                    <owl:Class>
                        <owl:unionOf rdf:parseType="Collection">
                            <rdf:Description rdf:about="https://w3id.org/rains#DeploymentStageAccountabilityPlan"/>
                            <rdf:Description rdf:about="https://w3id.org/rains#DesignStageAccountabilityPlan"/>
                            <rdf:Description rdf:about="https://w3id.org/rains#ImplementationStageAccountabilityPlan"/>
                            <rdf:Description rdf:about="https://w3id.org/rains#InstallationAccountabilityPlan"/>
                            <rdf:Description rdf:about="https://w3id.org/rains#MaintenanceAccountabilityPlan"/>
                            <rdf:Description rdf:about="https://w3id.org/rains#OperationStageAccountabilityPlan"/>
                        </owl:unionOf>
                    </owl:Class>
                </owl:allValuesFrom>
            </owl:Restriction>
        </rdfs:subClassOf>
        <rdfs:subClassOf>
            <owl:Restriction>
                <owl:onProperty rdf:resource="https://w3id.org/ep-plan#isStepOfPlan"/>
                <owl:allValuesFrom>
                    <owl:Class>
                        <owl:unionOf rdf:parseType="Collection">
                            <rdf:Description rdf:about="https://w3id.org/rains#DeploymentStageAccountabilityPlan"/>
                            <rdf:Description rdf:about="https://w3id.org/rains#DesignStageAccountabilityPlan"/>
                            <rdf:Description rdf:about="https://w3id.org/rains#ImplementationStageAccountabilityPlan"/>
                            <rdf:Description rdf:about="https://w3id.org/rains#InstallationAccountabilityPlan"/>
                            <rdf:Description rdf:about="https://w3id.org/rains#MaintenanceAccountabilityPlan"/>
                            <rdf:Description rdf:about="https://w3id.org/rains#OperationStageAccountabilityPlan"/>
                        </owl:unionOf>
                    </owl:Class>
                </owl:allValuesFrom>
            </owl:Restriction>
        </rdfs:subClassOf>
        <owl:disjointWith rdf:resource="https://w3id.org/rains#RealizeComponent"/>
        <owl:disjointWith rdf:resource="https://w3id.org/rains#SystemAction"/>
        <owl:disjointWith rdf:resource="https://w3id.org/rains#TrainUser"/>
        <rdfs:comment>A planned step describing the creation of a specification that has some impact on the AI System, e.g. the production of the design specification describing the training dataset to be used. This step is typically part of the Design stage of an AI System&apos;s life cycle and has members of the subclasses of Design Specification as its expected output(s). It can also be part of the Implementation and Deployment (Installation) Stages as as to allow the creation of specifications related to evaluating the AI system.</rdfs:comment>
        <rdfs:label>Produce Specification</rdfs:label>
    </owl:Class>
    


    <!-- https://w3id.org/rains#ProvideSystemInputData -->


    <owl:Class rdf:about="https://w3id.org/rains#ProvideSystemInputData">
        <rdfs:subClassOf rdf:resource="https://w3id.org/rains#SystemAction"/>
        <rdfs:subClassOf>
            <owl:Restriction>
                <owl:onProperty rdf:resource="https://w3id.org/ep-plan#hasOutputVariable"/>
                <owl:allValuesFrom>
                    <owl:Class>
                        <owl:unionOf rdf:parseType="Collection">
                            <rdf:Description rdf:about="https://w3id.org/rains#ConfigurationData"/>
                            <rdf:Description rdf:about="https://w3id.org/rains#RuntimeInputData"/>
                        </owl:unionOf>
                    </owl:Class>
                </owl:allValuesFrom>
            </owl:Restriction>
        </rdfs:subClassOf>
        <rdfs:subClassOf>
            <owl:Restriction>
                <owl:onProperty rdf:resource="https://w3id.org/ep-plan#isElementOfPlan"/>
                <owl:allValuesFrom>
                    <owl:Class>
                        <owl:unionOf rdf:parseType="Collection">
                            <rdf:Description rdf:about="https://w3id.org/rains#ConfigurationAccountabilityPlan"/>
                            <rdf:Description rdf:about="https://w3id.org/rains#DeploymentStageAccountabilityPlan"/>
                            <rdf:Description rdf:about="https://w3id.org/rains#InstallationAccountabilityPlan"/>
                            <rdf:Description rdf:about="https://w3id.org/rains#OperationStageAccountabilityPlan"/>
                            <rdf:Description rdf:about="https://w3id.org/rains#RuntimeAccountabilityPlan"/>
                        </owl:unionOf>
                    </owl:Class>
                </owl:allValuesFrom>
            </owl:Restriction>
        </rdfs:subClassOf>
        <rdfs:subClassOf>
            <owl:Restriction>
                <owl:onProperty rdf:resource="https://w3id.org/ep-plan#isStepOfPlan"/>
                <owl:allValuesFrom>
                    <owl:Class>
                        <owl:unionOf rdf:parseType="Collection">
                            <rdf:Description rdf:about="https://w3id.org/rains#ConfigurationAccountabilityPlan"/>
                            <rdf:Description rdf:about="https://w3id.org/rains#DeploymentStageAccountabilityPlan"/>
                            <rdf:Description rdf:about="https://w3id.org/rains#InstallationAccountabilityPlan"/>
                            <rdf:Description rdf:about="https://w3id.org/rains#OperationStageAccountabilityPlan"/>
                            <rdf:Description rdf:about="https://w3id.org/rains#RuntimeAccountabilityPlan"/>
                        </owl:unionOf>
                    </owl:Class>
                </owl:allValuesFrom>
            </owl:Restriction>
        </rdfs:subClassOf>
        <owl:disjointWith rdf:resource="https://w3id.org/rains#ReturnOutput"/>
        <owl:disjointWith rdf:resource="https://w3id.org/rains#Validate"/>
        <rdfs:comment>A planned step indicating that input data has been provided to the AI system by a user or a Supporting Infrastructure Component. This step is typically part of the Deployment or Operation stage of the life cycle (specifically, the Installation, Configuration, or Runtime stages). Depending on whether the input data was configuration data or runtime data, the output of this step is either configuration data or runtime data.</rdfs:comment>
        <rdfs:label>Provide System Input Data</rdfs:label>
    </owl:Class>
    


    <!-- https://w3id.org/rains#RealizableObject -->


    <owl:Class rdf:about="https://w3id.org/rains#RealizableObject">
        <rdfs:subClassOf rdf:resource="https://w3id.org/sao#InformationElement"/>
        <rdfs:comment>A sao:InformationElement  which records  information detailing  a piece of data, software or hardware that may be realized during the Implementation stage. A reused object (e.g., public training datasets) is also considered as :RealizableObject during the Design stage as it is not yet implemented (i.e., physical copies have not yet been integrated withing the ML pipeline)</rdfs:comment>
        <rdfs:label>Realizable Object</rdfs:label>
    </owl:Class>
    


    <!-- https://w3id.org/rains#RealizableObjectCharacteristic -->


    <owl:Class rdf:about="https://w3id.org/rains#RealizableObjectCharacteristic">
        <rdfs:subClassOf rdf:resource="https://w3id.org/sao#InformationElement"/>
        <rdfs:comment>A sao:InformationElement  which records  information detailing  a specific quality of :RealizableObject.</rdfs:comment>
        <rdfs:label>Realizable Object Characteristic</rdfs:label>
    </owl:Class>
    


    <!-- https://w3id.org/rains#RealizeComponent -->


    <owl:Class rdf:about="https://w3id.org/rains#RealizeComponent">
        <rdfs:subClassOf rdf:resource="https://w3id.org/sao#AccountableAction"/>
        <rdfs:subClassOf>
            <owl:Restriction>
                <owl:onProperty rdf:resource="https://w3id.org/ep-plan#hasOutputVariable"/>
                <owl:allValuesFrom>
                    <owl:Class>
                        <owl:unionOf rdf:parseType="Collection">
                            <rdf:Description rdf:about="https://w3id.org/rains#ChangeLog"/>
                            <rdf:Description rdf:about="https://w3id.org/rains#DatasetComponent"/>
                            <rdf:Description rdf:about="https://w3id.org/rains#EvaluationDataset"/>
                            <rdf:Description rdf:about="https://w3id.org/rains#ModelComponent"/>
                            <rdf:Description rdf:about="https://w3id.org/rains#SupportingInfrastructureComponent"/>
                            <rdf:Description rdf:about="https://w3id.org/rains#TrainingDataset"/>
                            <rdf:Description rdf:about="https://w3id.org/rains#ValidationDataset"/>
                        </owl:unionOf>
                    </owl:Class>
                </owl:allValuesFrom>
            </owl:Restriction>
        </rdfs:subClassOf>
        <rdfs:subClassOf>
            <owl:Restriction>
                <owl:onProperty rdf:resource="https://w3id.org/ep-plan#isElementOfPlan"/>
                <owl:allValuesFrom rdf:resource="https://w3id.org/rains#ImplementationStageAccountabilityPlan"/>
            </owl:Restriction>
        </rdfs:subClassOf>
        <rdfs:subClassOf>
            <owl:Restriction>
                <owl:onProperty rdf:resource="https://w3id.org/ep-plan#isStepOfPlan"/>
                <owl:allValuesFrom rdf:resource="https://w3id.org/rains#ImplementationStageAccountabilityPlan"/>
            </owl:Restriction>
        </rdfs:subClassOf>
        <owl:disjointWith rdf:resource="https://w3id.org/rains#SystemAction"/>
        <owl:disjointWith rdf:resource="https://w3id.org/rains#TrainUser"/>
        <rdfs:comment>A planned step describing the realization of a component. This includes implementing a component or retrieving it from a different (or third party) source. The realization of the component has some impact on the AI System, e.g. the implementation of the ML model or importing a third party dataset. This step has members of the class Dataset Component, Model Component, and Supporting Infrastructure Component as its expected output(s).  If a deviation from the design specification(s) takes place, then the step will also have as an output a member of the class Change Log.</rdfs:comment>
        <rdfs:label>Realize Component</rdfs:label>
    </owl:Class>
    


    <!-- https://w3id.org/rains#RealizededObject -->


    <owl:Class rdf:about="https://w3id.org/rains#RealizededObject">
        <rdfs:subClassOf rdf:resource="https://w3id.org/sao#InformationElement"/>
        <rdfs:comment>A sao:InformationElement which records information detailing a piece of data, software or hardware that was realized - whether or not it followed a design specification or a guideline.

For example, assume the dataset design specification specifies that dataset foobar is to be realised (to be used to train the model), but the implementation team realises dataset xyzzy. In this case, only dataset xyzzy is created as an instance of Realized Object.</rdfs:comment>
        <rdfs:label>Realized Object</rdfs:label>
    </owl:Class>
    


    <!-- https://w3id.org/rains#ReturnOutput -->


    <owl:Class rdf:about="https://w3id.org/rains#ReturnOutput">
        <rdfs:subClassOf rdf:resource="https://w3id.org/rains#SystemAction"/>
        <rdfs:subClassOf>
            <owl:Restriction>
                <owl:onProperty rdf:resource="https://w3id.org/ep-plan#hasOutputVariable"/>
                <owl:allValuesFrom rdf:resource="https://w3id.org/rains#SystemOutput"/>
            </owl:Restriction>
        </rdfs:subClassOf>
        <rdfs:subClassOf>
            <owl:Restriction>
                <owl:onProperty rdf:resource="https://w3id.org/ep-plan#isElementOfPlan"/>
                <owl:allValuesFrom>
                    <owl:Class>
                        <owl:unionOf rdf:parseType="Collection">
                            <rdf:Description rdf:about="https://w3id.org/rains#OperationStageAccountabilityPlan"/>
                            <rdf:Description rdf:about="https://w3id.org/rains#RuntimeAccountabilityPlan"/>
                        </owl:unionOf>
                    </owl:Class>
                </owl:allValuesFrom>
            </owl:Restriction>
        </rdfs:subClassOf>
        <rdfs:subClassOf>
            <owl:Restriction>
                <owl:onProperty rdf:resource="https://w3id.org/ep-plan#isStepOfPlan"/>
                <owl:allValuesFrom>
                    <owl:Class>
                        <owl:unionOf rdf:parseType="Collection">
                            <rdf:Description rdf:about="https://w3id.org/rains#OperationStageAccountabilityPlan"/>
                            <rdf:Description rdf:about="https://w3id.org/rains#RuntimeAccountabilityPlan"/>
                        </owl:unionOf>
                    </owl:Class>
                </owl:allValuesFrom>
            </owl:Restriction>
        </rdfs:subClassOf>
        <owl:disjointWith rdf:resource="https://w3id.org/rains#Validate"/>
        <rdfs:comment>A planned step that describes returning an output by the AI System. This step is typically part of the Operation stage (specifically Runtime stage) and has a member of the class System Output as its expected output.</rdfs:comment>
        <rdfs:label>Return Output</rdfs:label>
    </owl:Class>
    


    <!-- https://w3id.org/rains#Risk -->


    <owl:Class rdf:about="https://w3id.org/rains#Risk">
        <rdfs:subClassOf rdf:resource="https://w3id.org/sao#InformationElement"/>
        <rdfs:comment>A sao:InformationElement  which records a specific piece of  information detailing possible undesired or dangerous outcomes caused by any aspects of :AI_Sytem. 

If a mitigation strategy is used to abate the risk, then these can be indicated using the property :hasMitigationStrategy. It is advisable that information about the risk before and after mitigation is included.</rdfs:comment>
        <rdfs:label>Risk</rdfs:label>
    </owl:Class>
    


    <!-- https://w3id.org/rains#RuntimeAccountabilityPlan -->


    <owl:Class rdf:about="https://w3id.org/rains#RuntimeAccountabilityPlan">
        <rdfs:subClassOf rdf:resource="https://w3id.org/rains#OperationStageAccountabilityPlan"/>
        <rdfs:comment>A plan that identifies sao:AccountableAction(s) and sao:AccountableResult(s) relevant to running the system as part of the operation stage of an AI system and  which are required to be documented for accountability purposes. This plan is a subplan of the Operation Stage Accountability Plan. The Accountable Actions that can be done at this stage are: Notify User, Consent, Provide System Input Data, Preprocess Input Data, Validate, Generate Model Output, Explain, and Generate Output, Aggregate,  Override, Justify,  Approve Output, Return Output, Actuate Output, and Collect User Feedback.</rdfs:comment>
        <rdfs:label>Runtime Accountability Plan</rdfs:label>
    </owl:Class>
    


    <!-- https://w3id.org/rains#RuntimeInputData -->


    <owl:Class rdf:about="https://w3id.org/rains#RuntimeInputData">
        <rdfs:subClassOf rdf:resource="https://w3id.org/rains#SystemData"/>
        <rdfs:subClassOf>
            <owl:Restriction>
                <owl:onProperty rdf:resource="https://w3id.org/ep-plan#isElementOfPlan"/>
                <owl:allValuesFrom>
                    <owl:Class>
                        <owl:unionOf rdf:parseType="Collection">
                            <rdf:Description rdf:about="https://w3id.org/rains#OperationStageAccountabilityPlan"/>
                            <rdf:Description rdf:about="https://w3id.org/rains#RuntimeAccountabilityPlan"/>
                        </owl:unionOf>
                    </owl:Class>
                </owl:allValuesFrom>
            </owl:Restriction>
        </rdfs:subClassOf>
        <rdfs:subClassOf>
            <owl:Restriction>
                <owl:onProperty rdf:resource="https://w3id.org/ep-plan#isOutputVariableOf"/>
                <owl:allValuesFrom>
                    <owl:Class>
                        <owl:unionOf rdf:parseType="Collection">
                            <rdf:Description rdf:about="https://w3id.org/rains#PreprocessInputData"/>
                            <rdf:Description rdf:about="https://w3id.org/rains#ProvideSystemInputData"/>
                        </owl:unionOf>
                    </owl:Class>
                </owl:allValuesFrom>
            </owl:Restriction>
        </rdfs:subClassOf>
        <rdfs:subClassOf>
            <owl:Restriction>
                <owl:onProperty rdf:resource="https://w3id.org/ep-plan#isVariableOfPlan"/>
                <owl:allValuesFrom>
                    <owl:Class>
                        <owl:unionOf rdf:parseType="Collection">
                            <rdf:Description rdf:about="https://w3id.org/rains#OperationStageAccountabilityPlan"/>
                            <rdf:Description rdf:about="https://w3id.org/rains#RuntimeAccountabilityPlan"/>
                        </owl:unionOf>
                    </owl:Class>
                </owl:allValuesFrom>
            </owl:Restriction>
        </rdfs:subClassOf>
        <owl:disjointWith rdf:resource="https://w3id.org/rains#SystemOutput"/>
        <owl:disjointWith rdf:resource="https://w3id.org/rains#UserConsent"/>
        <owl:disjointWith rdf:resource="https://w3id.org/rains#UserReview"/>
        <owl:disjointWith rdf:resource="https://w3id.org/rains#Validation"/>
        <rdfs:comment>A specific type of planned System Data which represents the data used to operate the AI System during the Operation stage. For example, in a facial recognition AI system, the runtime data may be the picture of the user, the sensor data, and the environment data. 

It is advisable that the information realization corresponding to the Runtime Input Data variable contains the following information elements:
1. Data Item
2. DataCollectionProcedure
3. DataPreprocesingProcedure.
4. Affected Agent if the AI System is involved in making decisions/recommendations/actions affecting human users and the input data can be linked to the affected human (whether they are a user or not).</rdfs:comment>
        <rdfs:label>Runtime Input Data</rdfs:label>
    </owl:Class>
    


    <!-- https://w3id.org/rains#SoftLaw -->


    <owl:Class rdf:about="https://w3id.org/rains#SoftLaw">
        <rdfs:subClassOf rdf:resource="https://w3id.org/rains#ComplianceEntity"/>
        <rdfs:comment>A specific type of compliance entity which records a specific piece of  information about the procedures, standards, protocols, etc that complying with is desired or encouraged as part of an information realization collection.

When used as part of an information realization corresponding to a design specification, it describes the soft laws that are to be complied with. When used as part of an information realization corresponding to an realized component, it describes the soft laws that the component complies with.</rdfs:comment>
        <rdfs:label>Soft Law</rdfs:label>
    </owl:Class>
    


    <!-- https://w3id.org/rains#SupportingInfrastructure -->


    <owl:Class rdf:about="https://w3id.org/rains#SupportingInfrastructure">
        <rdfs:subClassOf rdf:resource="https://w3id.org/rains#RealizableObject"/>
        <rdfs:subClassOf>
            <owl:Class>
                <owl:unionOf rdf:parseType="Collection">
                    <rdf:Description rdf:about="https://w3id.org/rains#ExcludedObject"/>
                    <rdf:Description rdf:about="https://w3id.org/rains#RealizededObject"/>
                </owl:unionOf>
            </owl:Class>
        </rdfs:subClassOf>
        <rdfs:comment>A type of :RealizableObject detailing the hardware and software &apos;plumbing&apos; that is not generally considered part of the AI processes, however, may also be source of erroneous behaviour in :AI_System.</rdfs:comment>
        <rdfs:label>Supporting Infrastructure</rdfs:label>
    </owl:Class>
    


    <!-- https://w3id.org/rains#SupportingInfrastructureComponent -->


    <owl:Class rdf:about="https://w3id.org/rains#SupportingInfrastructureComponent">
        <rdfs:subClassOf rdf:resource="https://w3id.org/sao#AccountableResult"/>
        <rdfs:subClassOf>
            <owl:Restriction>
                <owl:onProperty rdf:resource="https://w3id.org/ep-plan#isElementOfPlan"/>
                <owl:allValuesFrom>
                    <owl:Class>
                        <owl:unionOf rdf:parseType="Collection">
                            <rdf:Description rdf:about="https://w3id.org/rains#ConfigurationAccountabilityPlan"/>
                            <rdf:Description rdf:about="https://w3id.org/rains#DeploymentStageAccountabilityPlan"/>
                            <rdf:Description rdf:about="https://w3id.org/rains#ImplementationStageAccountabilityPlan"/>
                            <rdf:Description rdf:about="https://w3id.org/rains#InstallationAccountabilityPlan"/>
                            <rdf:Description rdf:about="https://w3id.org/rains#MaintenanceAccountabilityPlan"/>
                            <rdf:Description rdf:about="https://w3id.org/rains#OperationStageAccountabilityPlan"/>
                            <rdf:Description rdf:about="https://w3id.org/rains#RuntimeAccountabilityPlan"/>
                        </owl:unionOf>
                    </owl:Class>
                </owl:allValuesFrom>
            </owl:Restriction>
        </rdfs:subClassOf>
        <rdfs:subClassOf>
            <owl:Restriction>
                <owl:onProperty rdf:resource="https://w3id.org/ep-plan#isOutputVariableOf"/>
                <owl:allValuesFrom>
                    <owl:Class>
                        <owl:unionOf rdf:parseType="Collection">
                            <rdf:Description rdf:about="https://w3id.org/rains#Configure"/>
                            <rdf:Description rdf:about="https://w3id.org/rains#Install"/>
                            <rdf:Description rdf:about="https://w3id.org/rains#RealizeComponent"/>
                        </owl:unionOf>
                    </owl:Class>
                </owl:allValuesFrom>
            </owl:Restriction>
        </rdfs:subClassOf>
        <rdfs:subClassOf>
            <owl:Restriction>
                <owl:onProperty rdf:resource="https://w3id.org/ep-plan#isVariableOfPlan"/>
                <owl:allValuesFrom>
                    <owl:Class>
                        <owl:unionOf rdf:parseType="Collection">
                            <rdf:Description rdf:about="https://w3id.org/rains#ConfigurationAccountabilityPlan"/>
                            <rdf:Description rdf:about="https://w3id.org/rains#DeploymentStageAccountabilityPlan"/>
                            <rdf:Description rdf:about="https://w3id.org/rains#ImplementationStageAccountabilityPlan"/>
                            <rdf:Description rdf:about="https://w3id.org/rains#InstallationAccountabilityPlan"/>
                            <rdf:Description rdf:about="https://w3id.org/rains#MaintenanceAccountabilityPlan"/>
                            <rdf:Description rdf:about="https://w3id.org/rains#OperationStageAccountabilityPlan"/>
                            <rdf:Description rdf:about="https://w3id.org/rains#RuntimeAccountabilityPlan"/>
                        </owl:unionOf>
                    </owl:Class>
                </owl:allValuesFrom>
            </owl:Restriction>
        </rdfs:subClassOf>
        <owl:disjointWith rdf:resource="https://w3id.org/rains#SystemData"/>
        <owl:disjointWith rdf:resource="https://w3id.org/rains#UserTrainingReport"/>
        <rdfs:comment>A specific type of planned sao:AccountableResult which represents the characteristics, performance, etc. related to all the implemented hardware and software &apos;plumbing&apos; that is not generally considered part of the AI processes, however, may also be source of erroneous behaviour in AI systems.

It is advisable that the information realization corresponding to the SupportingInfrastructureComponent variable contains the following information elements:
1. SupportingInfrastructure, the realized supporting infrastructure should be an instance of RealizedObject. If the implementation deviates from the design, then an additional upporting infrastructure should be indicated as an instance of ExcludedObject.
2. Limitation
3. Risk its subclass Bias and FairnessOrBiasDetectionSoftware if applicable
4. Tradeoff
5. SystemAuditMechanism
6. SystemExplanationMechanims
7. SystemFeedbackfromUserMechanism
8. SystemHumanOversightMechanism
9. SystemSecurityMechanism
10. The subclasses of Compliance Entity, namely, Hard Law and SoftLaw
11. The subclasses of Use Case, namely IncorrectUseCase and IntendedUseCase</rdfs:comment>
        <rdfs:label>Supporting Infrastructure Component</rdfs:label>
    </owl:Class>
    


    <!-- https://w3id.org/rains#SupportingInfrastructureSpecification -->


    <owl:Class rdf:about="https://w3id.org/rains#SupportingInfrastructureSpecification">
        <rdfs:subClassOf rdf:resource="https://w3id.org/rains#DesignSpecification"/>
        <rdfs:subClassOf>
            <owl:Restriction>
                <owl:onProperty rdf:resource="https://w3id.org/ep-plan#isElementOfPlan"/>
                <owl:allValuesFrom>
                    <owl:Class>
                        <owl:unionOf rdf:parseType="Collection">
                            <rdf:Description rdf:about="https://w3id.org/rains#DesignStageAccountabilityPlan"/>
                            <rdf:Description rdf:about="https://w3id.org/rains#ImplementationStageAccountabilityPlan"/>
                        </owl:unionOf>
                    </owl:Class>
                </owl:allValuesFrom>
            </owl:Restriction>
        </rdfs:subClassOf>
        <rdfs:subClassOf>
            <owl:Restriction>
                <owl:onProperty rdf:resource="https://w3id.org/ep-plan#isOutputVariableOf"/>
                <owl:allValuesFrom rdf:resource="https://w3id.org/rains#ProduceSpecification"/>
            </owl:Restriction>
        </rdfs:subClassOf>
        <rdfs:subClassOf>
            <owl:Restriction>
                <owl:onProperty rdf:resource="https://w3id.org/ep-plan#isVariableOfPlan"/>
                <owl:allValuesFrom>
                    <owl:Class>
                        <owl:unionOf rdf:parseType="Collection">
                            <rdf:Description rdf:about="https://w3id.org/rains#DesignStageAccountabilityPlan"/>
                            <rdf:Description rdf:about="https://w3id.org/rains#ImplementationStageAccountabilityPlan"/>
                        </owl:unionOf>
                    </owl:Class>
                </owl:allValuesFrom>
            </owl:Restriction>
        </rdfs:subClassOf>
        <owl:disjointWith rdf:resource="https://w3id.org/rains#SystemPurposeSpecification"/>
        <rdfs:comment>A specific type of design specification which represents the specification description of planned requirements, characteristics, performance, etc. related to all the hardware and software &apos;plumbing&apos; that is not generally considered part of the AI processes, however, may also be source of erroneous behaviour in AI systems.

It is advisable that the information realization corresponding to SupportingInfrastructureSpecification contains the following information elements:
1. SupportingInfrastructure
2. SystemAuditMechanism
3. SystemExplanationMechanim
4. SystemFeedbackfromUserMechanism
5. SystemHumanOversightMechanism
6. SystemSecurityMechanism
7. Limitation
8. Risk and its subclass Bias
9. Tradeoff
10. The subclasses of Compliance Entity, namely, Hard Law and SoftLaw
11. The subclasses of Use Case, namely IncorrectUseCase and IntendedUseCase</rdfs:comment>
        <rdfs:label>Supporting Infrastructure Specification</rdfs:label>
    </owl:Class>
    


    <!-- https://w3id.org/rains#SystemAction -->


    <owl:Class rdf:about="https://w3id.org/rains#SystemAction">
        <rdfs:subClassOf rdf:resource="https://w3id.org/sao#AccountableAction"/>
        <rdfs:subClassOf>
            <owl:Restriction>
                <owl:onProperty rdf:resource="https://w3id.org/ep-plan#hasOutputVariable"/>
                <owl:allValuesFrom>
                    <owl:Class>
                        <owl:unionOf rdf:parseType="Collection">
                            <rdf:Description rdf:about="https://w3id.org/rains#AggregationResult"/>
                            <rdf:Description rdf:about="https://w3id.org/rains#ChangeLog"/>
                            <rdf:Description rdf:about="https://w3id.org/rains#ConfigurationData"/>
                            <rdf:Description rdf:about="https://w3id.org/rains#DisclaimerNotification"/>
                            <rdf:Description rdf:about="https://w3id.org/rains#ErrorNotification"/>
                            <rdf:Description rdf:about="https://w3id.org/rains#Explanation"/>
                            <rdf:Description rdf:about="https://w3id.org/rains#ExplanationNotification"/>
                            <rdf:Description rdf:about="https://w3id.org/rains#ModelComponent"/>
                            <rdf:Description rdf:about="https://w3id.org/rains#ModelOutput"/>
                            <rdf:Description rdf:about="https://w3id.org/rains#Notification"/>
                            <rdf:Description rdf:about="https://w3id.org/rains#OverrideResult"/>
                            <rdf:Description rdf:about="https://w3id.org/rains#RuntimeInputData"/>
                            <rdf:Description rdf:about="https://w3id.org/rains#SupportingInfrastructureComponent"/>
                            <rdf:Description rdf:about="https://w3id.org/rains#SystemOutput"/>
                            <rdf:Description rdf:about="https://w3id.org/rains#UserConsent"/>
                            <rdf:Description rdf:about="https://w3id.org/rains#UserReview"/>
                            <rdf:Description rdf:about="https://w3id.org/rains#Validation"/>
                        </owl:unionOf>
                    </owl:Class>
                </owl:allValuesFrom>
            </owl:Restriction>
        </rdfs:subClassOf>
        <rdfs:subClassOf>
            <owl:Restriction>
                <owl:onProperty rdf:resource="https://w3id.org/ep-plan#isElementOfPlan"/>
                <owl:allValuesFrom>
                    <owl:Class>
                        <owl:unionOf rdf:parseType="Collection">
                            <rdf:Description rdf:about="https://w3id.org/rains#ConfigurationAccountabilityPlan"/>
                            <rdf:Description rdf:about="https://w3id.org/rains#DeploymentStageAccountabilityPlan"/>
                            <rdf:Description rdf:about="https://w3id.org/rains#InstallationAccountabilityPlan"/>
                            <rdf:Description rdf:about="https://w3id.org/rains#OperationStageAccountabilityPlan"/>
                            <rdf:Description rdf:about="https://w3id.org/rains#RuntimeAccountabilityPlan"/>
                        </owl:unionOf>
                    </owl:Class>
                </owl:allValuesFrom>
            </owl:Restriction>
        </rdfs:subClassOf>
        <rdfs:subClassOf>
            <owl:Restriction>
                <owl:onProperty rdf:resource="https://w3id.org/ep-plan#isStepOfPlan"/>
                <owl:allValuesFrom>
                    <owl:Class>
                        <owl:unionOf rdf:parseType="Collection">
                            <rdf:Description rdf:about="https://w3id.org/rains#ConfigurationAccountabilityPlan"/>
                            <rdf:Description rdf:about="https://w3id.org/rains#DeploymentStageAccountabilityPlan"/>
                            <rdf:Description rdf:about="https://w3id.org/rains#InstallationAccountabilityPlan"/>
                            <rdf:Description rdf:about="https://w3id.org/rains#OperationStageAccountabilityPlan"/>
                            <rdf:Description rdf:about="https://w3id.org/rains#RuntimeAccountabilityPlan"/>
                        </owl:unionOf>
                    </owl:Class>
                </owl:allValuesFrom>
            </owl:Restriction>
        </rdfs:subClassOf>
        <owl:disjointWith rdf:resource="https://w3id.org/rains#TrainUser"/>
        <rdfs:comment>A planned step describing an action performed during the Deployment or Operation stages that has an impact on either a component of the system or an output of the system and which are required to be documented for accountability purposes. The actions may be done by a components of the system or by a user of the system. The specific outputs of the performed action depends on its type, as described more by the subclasses of this step.</rdfs:comment>
        <rdfs:label>System Action</rdfs:label>
    </owl:Class>
    


    <!-- https://w3id.org/rains#SystemAuditMechanism -->


    <owl:Class rdf:about="https://w3id.org/rains#SystemAuditMechanism">
        <rdfs:subClassOf rdf:resource="https://w3id.org/rains#RealizableObjectCharacteristic"/>
        <rdfs:comment>A type of :RealizableObjectCharacteristic detailing how :AI_System may be interrogated about its inner processes and outputs produced.</rdfs:comment>
        <rdfs:label>System Audit Mechanism</rdfs:label>
    </owl:Class>
    


    <!-- https://w3id.org/rains#SystemData -->


    <owl:Class rdf:about="https://w3id.org/rains#SystemData">
        <rdfs:subClassOf rdf:resource="https://w3id.org/sao#AccountableResult"/>
        <rdfs:subClassOf>
            <owl:Restriction>
                <owl:onProperty rdf:resource="https://w3id.org/ep-plan#isElementOfPlan"/>
                <owl:allValuesFrom>
                    <owl:Class>
                        <owl:unionOf rdf:parseType="Collection">
                            <rdf:Description rdf:about="https://w3id.org/rains#ConfigurationAccountabilityPlan"/>
                            <rdf:Description rdf:about="https://w3id.org/rains#DeploymentStageAccountabilityPlan"/>
                            <rdf:Description rdf:about="https://w3id.org/rains#InstallationAccountabilityPlan"/>
                            <rdf:Description rdf:about="https://w3id.org/rains#OperationStageAccountabilityPlan"/>
                            <rdf:Description rdf:about="https://w3id.org/rains#RuntimeAccountabilityPlan"/>
                        </owl:unionOf>
                    </owl:Class>
                </owl:allValuesFrom>
            </owl:Restriction>
        </rdfs:subClassOf>
        <rdfs:subClassOf>
            <owl:Restriction>
                <owl:onProperty rdf:resource="https://w3id.org/ep-plan#isOutputVariableOf"/>
                <owl:allValuesFrom>
                    <owl:Class>
                        <owl:unionOf rdf:parseType="Collection">
                            <rdf:Description rdf:about="https://w3id.org/rains#ActuateOutput"/>
                            <rdf:Description rdf:about="https://w3id.org/rains#Aggregate"/>
                            <rdf:Description rdf:about="https://w3id.org/rains#CollectUserFeedback"/>
                            <rdf:Description rdf:about="https://w3id.org/rains#Consent"/>
                            <rdf:Description rdf:about="https://w3id.org/rains#Explain"/>
                            <rdf:Description rdf:about="https://w3id.org/rains#GenerateModelOutput"/>
                            <rdf:Description rdf:about="https://w3id.org/rains#GenerateOutput"/>
                            <rdf:Description rdf:about="https://w3id.org/rains#NotifyUser"/>
                            <rdf:Description rdf:about="https://w3id.org/rains#Override"/>
                            <rdf:Description rdf:about="https://w3id.org/rains#PreprocessInputData"/>
                            <rdf:Description rdf:about="https://w3id.org/rains#ProvideSystemInputData"/>
                            <rdf:Description rdf:about="https://w3id.org/rains#ReturnOutput"/>
                            <rdf:Description rdf:about="https://w3id.org/rains#SystemAction"/>
                            <rdf:Description rdf:about="https://w3id.org/rains#Validate"/>
                        </owl:unionOf>
                    </owl:Class>
                </owl:allValuesFrom>
            </owl:Restriction>
        </rdfs:subClassOf>
        <rdfs:subClassOf>
            <owl:Restriction>
                <owl:onProperty rdf:resource="https://w3id.org/ep-plan#isVariableOfPlan"/>
                <owl:allValuesFrom>
                    <owl:Class>
                        <owl:unionOf rdf:parseType="Collection">
                            <rdf:Description rdf:about="https://w3id.org/rains#ConfigurationAccountabilityPlan"/>
                            <rdf:Description rdf:about="https://w3id.org/rains#DeploymentStageAccountabilityPlan"/>
                            <rdf:Description rdf:about="https://w3id.org/rains#InstallationAccountabilityPlan"/>
                            <rdf:Description rdf:about="https://w3id.org/rains#OperationStageAccountabilityPlan"/>
                            <rdf:Description rdf:about="https://w3id.org/rains#RuntimeAccountabilityPlan"/>
                        </owl:unionOf>
                    </owl:Class>
                </owl:allValuesFrom>
            </owl:Restriction>
        </rdfs:subClassOf>
        <owl:disjointWith rdf:resource="https://w3id.org/rains#UserTrainingReport"/>
        <rdfs:comment>A specific type of planned sao:AccountableResult which represents a high level reference to data provided to or generated by the AI system after it has been installed, whether during the Deployment or Operation stages.</rdfs:comment>
        <rdfs:label>System Data</rdfs:label>
    </owl:Class>
    


    <!-- https://w3id.org/rains#SystemDeploymentGuidance -->


    <owl:Class rdf:about="https://w3id.org/rains#SystemDeploymentGuidance">
        <rdfs:subClassOf rdf:resource="https://w3id.org/rains#Guidance"/>
        <rdfs:comment>A specific type of Guidance which records a specific piece of information about the guidance to how the :AI_System should be deployed. It has two subclasses to further specify information related to installation and user training.</rdfs:comment>
        <rdfs:label>System Deployment Guidance</rdfs:label>
    </owl:Class>
    


    <!-- https://w3id.org/rains#SystemDeploymentGuideline -->


    <owl:Class rdf:about="https://w3id.org/rains#SystemDeploymentGuideline">
        <rdfs:subClassOf rdf:resource="https://w3id.org/rains#Guideline"/>
        <rdfs:subClassOf>
            <owl:Restriction>
                <owl:onProperty rdf:resource="https://w3id.org/ep-plan#isElementOfPlan"/>
                <owl:allValuesFrom>
                    <owl:Class>
                        <owl:unionOf rdf:parseType="Collection">
                            <rdf:Description rdf:about="https://w3id.org/rains#ConfigurationAccountabilityPlan"/>
                            <rdf:Description rdf:about="https://w3id.org/rains#DeploymentStageAccountabilityPlan"/>
                            <rdf:Description rdf:about="https://w3id.org/rains#ImplementationStageAccountabilityPlan"/>
                            <rdf:Description rdf:about="https://w3id.org/rains#InstallationAccountabilityPlan"/>
                            <rdf:Description rdf:about="https://w3id.org/rains#ManualProductionAccountabilityPlan"/>
                            <rdf:Description rdf:about="https://w3id.org/rains#OperationStageAccountabilityPlan"/>
                            <rdf:Description rdf:about="https://w3id.org/rains#UserTrainingAccountabilityPlan"/>
                        </owl:unionOf>
                    </owl:Class>
                </owl:allValuesFrom>
            </owl:Restriction>
        </rdfs:subClassOf>
        <rdfs:subClassOf>
            <owl:Restriction>
                <owl:onProperty rdf:resource="https://w3id.org/ep-plan#isOutputVariableOf"/>
                <owl:allValuesFrom rdf:resource="https://w3id.org/rains#GenerateGuideline"/>
            </owl:Restriction>
        </rdfs:subClassOf>
        <rdfs:subClassOf>
            <owl:Restriction>
                <owl:onProperty rdf:resource="https://w3id.org/ep-plan#isVariableOfPlan"/>
                <owl:allValuesFrom>
                    <owl:Class>
                        <owl:unionOf rdf:parseType="Collection">
                            <rdf:Description rdf:about="https://w3id.org/rains#ConfigurationAccountabilityPlan"/>
                            <rdf:Description rdf:about="https://w3id.org/rains#DeploymentStageAccountabilityPlan"/>
                            <rdf:Description rdf:about="https://w3id.org/rains#ImplementationStageAccountabilityPlan"/>
                            <rdf:Description rdf:about="https://w3id.org/rains#InstallationAccountabilityPlan"/>
                            <rdf:Description rdf:about="https://w3id.org/rains#ManualProductionAccountabilityPlan"/>
                            <rdf:Description rdf:about="https://w3id.org/rains#OperationStageAccountabilityPlan"/>
                            <rdf:Description rdf:about="https://w3id.org/rains#UserTrainingAccountabilityPlan"/>
                        </owl:unionOf>
                    </owl:Class>
                </owl:allValuesFrom>
            </owl:Restriction>
        </rdfs:subClassOf>
        <rdfs:comment>A specific type of :Guideline which represents the description of guidelines for the Deployment stage of the AI System.

It is advisable that the information realization corresponding to the System Deployment Guideline variable contains the following information elements:
1. SystemInstallationGuidance
2. UserTrainingGuidance</rdfs:comment>
        <rdfs:label>System Deployment Guideline</rdfs:label>
    </owl:Class>
    


    <!-- https://w3id.org/rains#SystemExplanationMechanism -->


    <owl:Class rdf:about="https://w3id.org/rains#SystemExplanationMechanism">
        <rdfs:subClassOf rdf:resource="https://w3id.org/rains#RealizableObjectCharacteristic"/>
        <rdfs:comment>A type of :RealizableObjectCharacteristic detailing how :AI_System produces human readable clarifications and justifications of its inner processes and outputs produced.</rdfs:comment>
        <rdfs:label>System Explanation Mechanism</rdfs:label>
    </owl:Class>
    


    <!-- https://w3id.org/rains#SystemFeedbackFromUserMechanism -->


    <owl:Class rdf:about="https://w3id.org/rains#SystemFeedbackFromUserMechanism">
        <rdfs:subClassOf rdf:resource="https://w3id.org/rains#RealizableObjectCharacteristic"/>
        <rdfs:comment>A type of :RealizableObjectCharacteristic detailing how :AI_System may receive feedback or review from its user(s) about its produced output(s).</rdfs:comment>
        <rdfs:label>System Feedback From User Mechanism</rdfs:label>
    </owl:Class>
    


    <!-- https://w3id.org/rains#SystemHumanOversightMechanism -->


    <owl:Class rdf:about="https://w3id.org/rains#SystemHumanOversightMechanism">
        <rdfs:subClassOf rdf:resource="https://w3id.org/rains#RealizableObjectCharacteristic"/>
        <rdfs:comment>A type of :RealizableObjectCharacteristic detailing how :AI_System integrates human operators in its decision processes to offer them the opportunity to stop, review, or alter the outputs produced by the system.</rdfs:comment>
        <rdfs:label>System Human Oversight Mechanism</rdfs:label>
    </owl:Class>
    


    <!-- https://w3id.org/rains#SystemInstallationGuidance -->


    <owl:Class rdf:about="https://w3id.org/rains#SystemInstallationGuidance">
        <rdfs:subClassOf rdf:resource="https://w3id.org/rains#SystemDeploymentGuidance"/>
        <rdfs:comment>A specific type of :Guidance which records a specific piece of information about the guidance to how the :AI_System should be installed. This includes any installations and integrations. It also includes any configurations that are done during the Deployment stage after the installation and integration, but before any user uses the system in the Operation Stage, for example, configuring an app to connect to WiFi as part of its installation.</rdfs:comment>
        <rdfs:label>System Installation Guidance</rdfs:label>
    </owl:Class>
    


    <!-- https://w3id.org/rains#SystemInstallationGuideline -->


    <owl:Class rdf:about="https://w3id.org/rains#SystemInstallationGuideline">
        <rdfs:subClassOf rdf:resource="https://w3id.org/rains#SystemDeploymentGuideline"/>
        <rdfs:subClassOf>
            <owl:Restriction>
                <owl:onProperty rdf:resource="https://w3id.org/ep-plan#isElementOfPlan"/>
                <owl:allValuesFrom>
                    <owl:Class>
                        <owl:unionOf rdf:parseType="Collection">
                            <rdf:Description rdf:about="https://w3id.org/rains#ConfigurationAccountabilityPlan"/>
                            <rdf:Description rdf:about="https://w3id.org/rains#DeploymentStageAccountabilityPlan"/>
                            <rdf:Description rdf:about="https://w3id.org/rains#ImplementationStageAccountabilityPlan"/>
                            <rdf:Description rdf:about="https://w3id.org/rains#InstallationAccountabilityPlan"/>
                            <rdf:Description rdf:about="https://w3id.org/rains#OperationStageAccountabilityPlan"/>
                        </owl:unionOf>
                    </owl:Class>
                </owl:allValuesFrom>
            </owl:Restriction>
        </rdfs:subClassOf>
        <rdfs:subClassOf>
            <owl:Restriction>
                <owl:onProperty rdf:resource="https://w3id.org/ep-plan#isOutputVariableOf"/>
                <owl:allValuesFrom rdf:resource="https://w3id.org/rains#GenerateGuideline"/>
            </owl:Restriction>
        </rdfs:subClassOf>
        <rdfs:subClassOf>
            <owl:Restriction>
                <owl:onProperty rdf:resource="https://w3id.org/ep-plan#isVariableOfPlan"/>
                <owl:allValuesFrom>
                    <owl:Class>
                        <owl:unionOf rdf:parseType="Collection">
                            <rdf:Description rdf:about="https://w3id.org/rains#ConfigurationAccountabilityPlan"/>
                            <rdf:Description rdf:about="https://w3id.org/rains#DeploymentStageAccountabilityPlan"/>
                            <rdf:Description rdf:about="https://w3id.org/rains#ImplementationStageAccountabilityPlan"/>
                            <rdf:Description rdf:about="https://w3id.org/rains#InstallationAccountabilityPlan"/>
                            <rdf:Description rdf:about="https://w3id.org/rains#OperationStageAccountabilityPlan"/>
                        </owl:unionOf>
                    </owl:Class>
                </owl:allValuesFrom>
            </owl:Restriction>
        </rdfs:subClassOf>
        <rdfs:comment>A specific type of System Deployment Guideline which represents the description of guidelines for the Installing AI System, including any integration and configuration done during the Deployment Stage.

It is advisable that the information realization corresponding to the System Deployment Guideline variable contains the information element: SystemInstallationGuidance.</rdfs:comment>
        <rdfs:label>System Installation Guideline</rdfs:label>
    </owl:Class>
    


    <!-- https://w3id.org/rains#SystemMaintenanceGuidance -->


    <owl:Class rdf:about="https://w3id.org/rains#SystemMaintenanceGuidance">
        <rdfs:subClassOf rdf:resource="https://w3id.org/rains#SystemOperationGuidance"/>
        <rdfs:comment>A specific type of :Guidance which records a specific piece of information about the guidance to how the :AI_System should be maintained.</rdfs:comment>
        <rdfs:label>System Maintenance Guidance</rdfs:label>
    </owl:Class>
    


    <!-- https://w3id.org/rains#SystemMaintenanceGuideline -->


    <owl:Class rdf:about="https://w3id.org/rains#SystemMaintenanceGuideline">
        <rdfs:subClassOf rdf:resource="https://w3id.org/rains#SystemOperationGuideline"/>
        <rdfs:subClassOf>
            <owl:Restriction>
                <owl:onProperty rdf:resource="https://w3id.org/ep-plan#isElementOfPlan"/>
                <owl:allValuesFrom>
                    <owl:Class>
                        <owl:unionOf rdf:parseType="Collection">
                            <rdf:Description rdf:about="https://w3id.org/rains#DeploymentStageAccountabilityPlan"/>
                            <rdf:Description rdf:about="https://w3id.org/rains#ImplementationStageAccountabilityPlan"/>
                            <rdf:Description rdf:about="https://w3id.org/rains#MaintenanceAccountabilityPlan"/>
                            <rdf:Description rdf:about="https://w3id.org/rains#ManualProductionAccountabilityPlan"/>
                            <rdf:Description rdf:about="https://w3id.org/rains#OperationStageAccountabilityPlan"/>
                        </owl:unionOf>
                    </owl:Class>
                </owl:allValuesFrom>
            </owl:Restriction>
        </rdfs:subClassOf>
        <rdfs:subClassOf>
            <owl:Restriction>
                <owl:onProperty rdf:resource="https://w3id.org/ep-plan#isOutputVariableOf"/>
                <owl:allValuesFrom rdf:resource="https://w3id.org/rains#GenerateGuideline"/>
            </owl:Restriction>
        </rdfs:subClassOf>
        <rdfs:subClassOf>
            <owl:Restriction>
                <owl:onProperty rdf:resource="https://w3id.org/ep-plan#isVariableOfPlan"/>
                <owl:allValuesFrom>
                    <owl:Class>
                        <owl:unionOf rdf:parseType="Collection">
                            <rdf:Description rdf:about="https://w3id.org/rains#DeploymentStageAccountabilityPlan"/>
                            <rdf:Description rdf:about="https://w3id.org/rains#ImplementationStageAccountabilityPlan"/>
                            <rdf:Description rdf:about="https://w3id.org/rains#MaintenanceAccountabilityPlan"/>
                            <rdf:Description rdf:about="https://w3id.org/rains#ManualProductionAccountabilityPlan"/>
                            <rdf:Description rdf:about="https://w3id.org/rains#OperationStageAccountabilityPlan"/>
                        </owl:unionOf>
                    </owl:Class>
                </owl:allValuesFrom>
            </owl:Restriction>
        </rdfs:subClassOf>
        <rdfs:comment>A specific type of System Operation Guideline which represents the description of guidelines for how the AI System should be maintained. Typically, such guidance takes the form of a manual. 

It is advisable that the information realization corresponding to the System Maintenance Guideline variable contains the following information element: SystemMaintenanceGuidance.</rdfs:comment>
        <rdfs:label>System Maintenance Guideline</rdfs:label>
    </owl:Class>
    


    <!-- https://w3id.org/rains#SystemOperationGuidance -->


    <owl:Class rdf:about="https://w3id.org/rains#SystemOperationGuidance">
        <rdfs:subClassOf rdf:resource="https://w3id.org/rains#Guidance"/>
        <rdfs:comment>A specific type of :Guidance which records a specific piece of information about the guidance to how the :AI_System should be used and maintained. This class has two subclasses to further specify information related to usage and maintenance.</rdfs:comment>
        <rdfs:label>System Operation Guidance</rdfs:label>
    </owl:Class>
    


    <!-- https://w3id.org/rains#SystemOperationGuideline -->


    <owl:Class rdf:about="https://w3id.org/rains#SystemOperationGuideline">
        <rdfs:subClassOf rdf:resource="https://w3id.org/rains#Guideline"/>
        <rdfs:subClassOf>
            <owl:Restriction>
                <owl:onProperty rdf:resource="https://w3id.org/ep-plan#isElementOfPlan"/>
                <owl:allValuesFrom>
                    <owl:Class>
                        <owl:unionOf rdf:parseType="Collection">
                            <rdf:Description rdf:about="https://w3id.org/rains#DeploymentStageAccountabilityPlan"/>
                            <rdf:Description rdf:about="https://w3id.org/rains#ImplementationStageAccountabilityPlan"/>
                            <rdf:Description rdf:about="https://w3id.org/rains#MaintenanceAccountabilityPlan"/>
                            <rdf:Description rdf:about="https://w3id.org/rains#ManualProductionAccountabilityPlan"/>
                            <rdf:Description rdf:about="https://w3id.org/rains#OperationStageAccountabilityPlan"/>
                            <rdf:Description rdf:about="https://w3id.org/rains#RuntimeAccountabilityPlan"/>
                            <rdf:Description rdf:about="https://w3id.org/rains#UserTrainingAccountabilityPlan"/>
                        </owl:unionOf>
                    </owl:Class>
                </owl:allValuesFrom>
            </owl:Restriction>
        </rdfs:subClassOf>
        <rdfs:subClassOf>
            <owl:Restriction>
                <owl:onProperty rdf:resource="https://w3id.org/ep-plan#isOutputVariableOf"/>
                <owl:allValuesFrom rdf:resource="https://w3id.org/rains#GenerateGuideline"/>
            </owl:Restriction>
        </rdfs:subClassOf>
        <rdfs:subClassOf>
            <owl:Restriction>
                <owl:onProperty rdf:resource="https://w3id.org/ep-plan#isVariableOfPlan"/>
                <owl:allValuesFrom>
                    <owl:Class>
                        <owl:unionOf rdf:parseType="Collection">
                            <rdf:Description rdf:about="https://w3id.org/rains#DeploymentStageAccountabilityPlan"/>
                            <rdf:Description rdf:about="https://w3id.org/rains#ImplementationStageAccountabilityPlan"/>
                            <rdf:Description rdf:about="https://w3id.org/rains#MaintenanceAccountabilityPlan"/>
                            <rdf:Description rdf:about="https://w3id.org/rains#ManualProductionAccountabilityPlan"/>
                            <rdf:Description rdf:about="https://w3id.org/rains#OperationStageAccountabilityPlan"/>
                            <rdf:Description rdf:about="https://w3id.org/rains#RuntimeAccountabilityPlan"/>
                            <rdf:Description rdf:about="https://w3id.org/rains#UserTrainingAccountabilityPlan"/>
                        </owl:unionOf>
                    </owl:Class>
                </owl:allValuesFrom>
            </owl:Restriction>
        </rdfs:subClassOf>
        <rdfs:comment>A specific type of :Guideline which represents the description of guidelines for the Operation stage of the AI System. Typically, such guidance takes the form of a manual. 

It is advisable that the information realization corresponding to the System Operation Guideline variable contains the following information elements:
1. SystemUsageGuidance
2. SystemMaintenanceGuidance</rdfs:comment>
        <rdfs:label>System Operation Guideline</rdfs:label>
    </owl:Class>
    


    <!-- https://w3id.org/rains#SystemOutput -->


    <owl:Class rdf:about="https://w3id.org/rains#SystemOutput">
        <rdfs:subClassOf rdf:resource="https://w3id.org/rains#SystemData"/>
        <rdfs:subClassOf>
            <owl:Restriction>
                <owl:onProperty rdf:resource="https://w3id.org/ep-plan#isElementOfPlan"/>
                <owl:allValuesFrom>
                    <owl:Class>
                        <owl:unionOf rdf:parseType="Collection">
                            <rdf:Description rdf:about="https://w3id.org/rains#ConfigurationAccountabilityPlan"/>
                            <rdf:Description rdf:about="https://w3id.org/rains#DeploymentStageAccountabilityPlan"/>
                            <rdf:Description rdf:about="https://w3id.org/rains#InstallationAccountabilityPlan"/>
                            <rdf:Description rdf:about="https://w3id.org/rains#OperationStageAccountabilityPlan"/>
                            <rdf:Description rdf:about="https://w3id.org/rains#RuntimeAccountabilityPlan"/>
                        </owl:unionOf>
                    </owl:Class>
                </owl:allValuesFrom>
            </owl:Restriction>
        </rdfs:subClassOf>
        <rdfs:subClassOf>
            <owl:Restriction>
                <owl:onProperty rdf:resource="https://w3id.org/ep-plan#isOutputVariableOf"/>
                <owl:allValuesFrom>
                    <owl:Class>
                        <owl:unionOf rdf:parseType="Collection">
                            <rdf:Description rdf:about="https://w3id.org/rains#ActuateOutput"/>
                            <rdf:Description rdf:about="https://w3id.org/rains#Aggregate"/>
                            <rdf:Description rdf:about="https://w3id.org/rains#GenerateModelOutput"/>
                            <rdf:Description rdf:about="https://w3id.org/rains#GenerateOutput"/>
                            <rdf:Description rdf:about="https://w3id.org/rains#Override"/>
                            <rdf:Description rdf:about="https://w3id.org/rains#ReturnOutput"/>
                        </owl:unionOf>
                    </owl:Class>
                </owl:allValuesFrom>
            </owl:Restriction>
        </rdfs:subClassOf>
        <rdfs:subClassOf>
            <owl:Restriction>
                <owl:onProperty rdf:resource="https://w3id.org/ep-plan#isVariableOfPlan"/>
                <owl:allValuesFrom>
                    <owl:Class>
                        <owl:unionOf rdf:parseType="Collection">
                            <rdf:Description rdf:about="https://w3id.org/rains#ConfigurationAccountabilityPlan"/>
                            <rdf:Description rdf:about="https://w3id.org/rains#DeploymentStageAccountabilityPlan"/>
                            <rdf:Description rdf:about="https://w3id.org/rains#InstallationAccountabilityPlan"/>
                            <rdf:Description rdf:about="https://w3id.org/rains#OperationStageAccountabilityPlan"/>
                            <rdf:Description rdf:about="https://w3id.org/rains#RuntimeAccountabilityPlan"/>
                        </owl:unionOf>
                    </owl:Class>
                </owl:allValuesFrom>
            </owl:Restriction>
        </rdfs:subClassOf>
        <owl:disjointWith rdf:resource="https://w3id.org/rains#UserConsent"/>
        <owl:disjointWith rdf:resource="https://w3id.org/rains#UserReview"/>
        <owl:disjointWith rdf:resource="https://w3id.org/rains#Validation"/>
        <rdfs:comment>A specific type of planned System Data which describes an output generated by the system, via its human user, its Model Component (s), or its Supporting Infrastrcuture Component (s).

If the AI System is involved in making decisions/recommendations/actions affecting human users, then it is advisable that the information realization corresponding to the System Output variable contains the following information elements: Affected Agent.</rdfs:comment>
        <rdfs:label>System Output</rdfs:label>
    </owl:Class>
    


    <!-- https://w3id.org/rains#SystemPurposeSpecification -->


    <owl:Class rdf:about="https://w3id.org/rains#SystemPurposeSpecification">
        <rdfs:subClassOf rdf:resource="https://w3id.org/rains#DesignSpecification"/>
        <rdfs:subClassOf>
            <owl:Restriction>
                <owl:onProperty rdf:resource="https://w3id.org/ep-plan#isElementOfPlan"/>
                <owl:allValuesFrom>
                    <owl:Class>
                        <owl:unionOf rdf:parseType="Collection">
                            <rdf:Description rdf:about="https://w3id.org/rains#DesignStageAccountabilityPlan"/>
                            <rdf:Description rdf:about="https://w3id.org/rains#ImplementationStageAccountabilityPlan"/>
                            <rdf:Description rdf:about="https://w3id.org/rains#InstallationAccountabilityPlan"/>
                            <rdf:Description rdf:about="https://w3id.org/rains#MaintenanceAccountabilityPlan"/>
                            <rdf:Description rdf:about="https://w3id.org/rains#ManualProductionAccountabilityPlan"/>
                            <rdf:Description rdf:about="https://w3id.org/rains#OperationStageAccountabilityPlan"/>
                            <rdf:Description rdf:about="https://w3id.org/rains#UserTrainingAccountabilityPlan"/>
                        </owl:unionOf>
                    </owl:Class>
                </owl:allValuesFrom>
            </owl:Restriction>
        </rdfs:subClassOf>
        <rdfs:subClassOf>
            <owl:Restriction>
                <owl:onProperty rdf:resource="https://w3id.org/ep-plan#isOutputVariableOf"/>
                <owl:allValuesFrom rdf:resource="https://w3id.org/rains#ProduceSpecification"/>
            </owl:Restriction>
        </rdfs:subClassOf>
        <rdfs:subClassOf>
            <owl:Restriction>
                <owl:onProperty rdf:resource="https://w3id.org/ep-plan#isVariableOfPlan"/>
                <owl:allValuesFrom>
                    <owl:Class>
                        <owl:unionOf rdf:parseType="Collection">
                            <rdf:Description rdf:about="https://w3id.org/rains#DesignStageAccountabilityPlan"/>
                            <rdf:Description rdf:about="https://w3id.org/rains#ImplementationStageAccountabilityPlan"/>
                            <rdf:Description rdf:about="https://w3id.org/rains#InstallationAccountabilityPlan"/>
                            <rdf:Description rdf:about="https://w3id.org/rains#MaintenanceAccountabilityPlan"/>
                            <rdf:Description rdf:about="https://w3id.org/rains#ManualProductionAccountabilityPlan"/>
                            <rdf:Description rdf:about="https://w3id.org/rains#OperationStageAccountabilityPlan"/>
                            <rdf:Description rdf:about="https://w3id.org/rains#UserTrainingAccountabilityPlan"/>
                        </owl:unionOf>
                    </owl:Class>
                </owl:allValuesFrom>
            </owl:Restriction>
        </rdfs:subClassOf>
        <rdfs:comment>A specific type of design specification which represents  the  description of the purpose(s) for which an AI system is designed and used for.

It is advisable that the information realization corresponding to SystemPurposeSpecification contains the following information elements
1. IntendedUserGroup
2. The subclasses of Use Case, namely IncorrectUseCase and IntendedUseCase</rdfs:comment>
        <rdfs:label>System Purpose Specification</rdfs:label>
    </owl:Class>
    


    <!-- https://w3id.org/rains#SystemSecurityMechanism -->


    <owl:Class rdf:about="https://w3id.org/rains#SystemSecurityMechanism">
        <rdfs:subClassOf rdf:resource="https://w3id.org/rains#RealizableObjectCharacteristic"/>
        <rdfs:comment>A type of :RealizableObjectCharacteristic detailing how :AI_System may be safeguarded against adversarial attacks or potential breaches of security.</rdfs:comment>
        <rdfs:label>System Security Mechanism</rdfs:label>
    </owl:Class>
    


    <!-- https://w3id.org/rains#SystemUsageGuidance -->


    <owl:Class rdf:about="https://w3id.org/rains#SystemUsageGuidance">
        <rdfs:subClassOf rdf:resource="https://w3id.org/rains#SystemOperationGuidance"/>
        <rdfs:comment>A specific type of :Guidance which records a specific piece of information about the guidance to how the :AI_System should be used. This includes configuring the system by the user after it the deployment stage and its configurations have ended. For example, configuring an face detection app to recognise new users.</rdfs:comment>
        <rdfs:label>System Usage Guidance</rdfs:label>
    </owl:Class>
    


    <!-- https://w3id.org/rains#SystemUsageGuideline -->


    <owl:Class rdf:about="https://w3id.org/rains#SystemUsageGuideline">
        <rdfs:subClassOf rdf:resource="https://w3id.org/rains#SystemOperationGuideline"/>
        <rdfs:subClassOf>
            <owl:Restriction>
                <owl:onProperty rdf:resource="https://w3id.org/ep-plan#isElementOfPlan"/>
                <owl:allValuesFrom>
                    <owl:Class>
                        <owl:unionOf rdf:parseType="Collection">
                            <rdf:Description rdf:about="https://w3id.org/rains#ConfigurationAccountabilityPlan"/>
                            <rdf:Description rdf:about="https://w3id.org/rains#DeploymentStageAccountabilityPlan"/>
                            <rdf:Description rdf:about="https://w3id.org/rains#ImplementationStageAccountabilityPlan"/>
                            <rdf:Description rdf:about="https://w3id.org/rains#ManualProductionAccountabilityPlan"/>
                            <rdf:Description rdf:about="https://w3id.org/rains#OperationStageAccountabilityPlan"/>
                            <rdf:Description rdf:about="https://w3id.org/rains#RuntimeAccountabilityPlan"/>
                        </owl:unionOf>
                    </owl:Class>
                </owl:allValuesFrom>
            </owl:Restriction>
        </rdfs:subClassOf>
        <rdfs:subClassOf>
            <owl:Restriction>
                <owl:onProperty rdf:resource="https://w3id.org/ep-plan#isOutputVariableOf"/>
                <owl:allValuesFrom rdf:resource="https://w3id.org/rains#GenerateGuideline"/>
            </owl:Restriction>
        </rdfs:subClassOf>
        <rdfs:subClassOf>
            <owl:Restriction>
                <owl:onProperty rdf:resource="https://w3id.org/ep-plan#isVariableOfPlan"/>
                <owl:allValuesFrom>
                    <owl:Class>
                        <owl:unionOf rdf:parseType="Collection">
                            <rdf:Description rdf:about="https://w3id.org/rains#ConfigurationAccountabilityPlan"/>
                            <rdf:Description rdf:about="https://w3id.org/rains#DeploymentStageAccountabilityPlan"/>
                            <rdf:Description rdf:about="https://w3id.org/rains#ImplementationStageAccountabilityPlan"/>
                            <rdf:Description rdf:about="https://w3id.org/rains#ManualProductionAccountabilityPlan"/>
                            <rdf:Description rdf:about="https://w3id.org/rains#OperationStageAccountabilityPlan"/>
                            <rdf:Description rdf:about="https://w3id.org/rains#RuntimeAccountabilityPlan"/>
                        </owl:unionOf>
                    </owl:Class>
                </owl:allValuesFrom>
            </owl:Restriction>
        </rdfs:subClassOf>
        <rdfs:comment>A specific type of System Operation Guideline which represents the description of guidelines for how the AI System should be used. Typically, such guidance takes the form of a manual. 

It is advisable that the information realization corresponding to the System Maintenance Guideline variable contains the following information element: SystemUsageGuidance.</rdfs:comment>
        <rdfs:label>System Usage Guideline</rdfs:label>
    </owl:Class>
    


    <!-- https://w3id.org/rains#ThirdPartyEvaluation -->


    <owl:Class rdf:about="https://w3id.org/rains#ThirdPartyEvaluation">
        <rdfs:subClassOf rdf:resource="https://w3id.org/rains#Evaluation"/>
        <rdfs:subClassOf>
            <owl:Restriction>
                <owl:onProperty rdf:resource="https://w3id.org/ep-plan#isElementOfPlan"/>
                <owl:allValuesFrom>
                    <owl:Class>
                        <owl:unionOf rdf:parseType="Collection">
                            <rdf:Description rdf:about="https://w3id.org/rains#DeploymentStageAccountabilityPlan"/>
                            <rdf:Description rdf:about="https://w3id.org/rains#ImplementationStageAccountabilityPlan"/>
                            <rdf:Description rdf:about="https://w3id.org/rains#InstallationAccountabilityPlan"/>
                            <rdf:Description rdf:about="https://w3id.org/rains#MaintenanceAccountabilityPlan"/>
                            <rdf:Description rdf:about="https://w3id.org/rains#OperationStageAccountabilityPlan"/>
                        </owl:unionOf>
                    </owl:Class>
                </owl:allValuesFrom>
            </owl:Restriction>
        </rdfs:subClassOf>
        <rdfs:subClassOf>
            <owl:Restriction>
                <owl:onProperty rdf:resource="https://w3id.org/ep-plan#isOutputVariableOf"/>
                <owl:allValuesFrom rdf:resource="https://w3id.org/rains#Evaluate"/>
            </owl:Restriction>
        </rdfs:subClassOf>
        <rdfs:subClassOf>
            <owl:Restriction>
                <owl:onProperty rdf:resource="https://w3id.org/ep-plan#isVariableOfPlan"/>
                <owl:allValuesFrom>
                    <owl:Class>
                        <owl:unionOf rdf:parseType="Collection">
                            <rdf:Description rdf:about="https://w3id.org/rains#DeploymentStageAccountabilityPlan"/>
                            <rdf:Description rdf:about="https://w3id.org/rains#ImplementationStageAccountabilityPlan"/>
                            <rdf:Description rdf:about="https://w3id.org/rains#InstallationAccountabilityPlan"/>
                            <rdf:Description rdf:about="https://w3id.org/rains#MaintenanceAccountabilityPlan"/>
                            <rdf:Description rdf:about="https://w3id.org/rains#OperationStageAccountabilityPlan"/>
                        </owl:unionOf>
                    </owl:Class>
                </owl:allValuesFrom>
            </owl:Restriction>
        </rdfs:subClassOf>
        <rdfs:comment>A specific type of :Evaluation which represents an evaluation performed by a third party independent of the developers of the AI System.</rdfs:comment>
        <rdfs:label>Third Party Evaluation</rdfs:label>
    </owl:Class>
    


    <!-- https://w3id.org/rains#TradeOff -->


    <owl:Class rdf:about="https://w3id.org/rains#TradeOff">
        <rdfs:subClassOf rdf:resource="https://w3id.org/sao#InformationElement"/>
        <rdfs:comment>A sao:InformationElement  which records a specific piece of  information detailing tradeoffs to mitigate possible undesired or dangerous outcomes caused by any aspects of :AI_Sytem.</rdfs:comment>
        <rdfs:label>TradeOff</rdfs:label>
    </owl:Class>
    


    <!-- https://w3id.org/rains#TrainUser -->


    <owl:Class rdf:about="https://w3id.org/rains#TrainUser">
        <rdfs:subClassOf rdf:resource="https://w3id.org/sao#AccountableAction"/>
        <rdfs:subClassOf>
            <owl:Restriction>
                <owl:onProperty rdf:resource="https://w3id.org/ep-plan#hasOutputVariable"/>
                <owl:allValuesFrom>
                    <owl:Class>
                        <owl:unionOf rdf:parseType="Collection">
                            <rdf:Description rdf:about="https://w3id.org/rains#ChangeLog"/>
                            <rdf:Description rdf:about="https://w3id.org/rains#UserTrainingReport"/>
                        </owl:unionOf>
                    </owl:Class>
                </owl:allValuesFrom>
            </owl:Restriction>
        </rdfs:subClassOf>
        <rdfs:subClassOf>
            <owl:Restriction>
                <owl:onProperty rdf:resource="https://w3id.org/ep-plan#isElementOfPlan"/>
                <owl:allValuesFrom>
                    <owl:Class>
                        <owl:unionOf rdf:parseType="Collection">
                            <rdf:Description rdf:about="https://w3id.org/rains#DeploymentStageAccountabilityPlan"/>
                            <rdf:Description rdf:about="https://w3id.org/rains#UserTrainingAccountabilityPlan"/>
                        </owl:unionOf>
                    </owl:Class>
                </owl:allValuesFrom>
            </owl:Restriction>
        </rdfs:subClassOf>
        <rdfs:subClassOf>
            <owl:Restriction>
                <owl:onProperty rdf:resource="https://w3id.org/ep-plan#isStepOfPlan"/>
                <owl:allValuesFrom>
                    <owl:Class>
                        <owl:unionOf rdf:parseType="Collection">
                            <rdf:Description rdf:about="https://w3id.org/rains#DeploymentStageAccountabilityPlan"/>
                            <rdf:Description rdf:about="https://w3id.org/rains#UserTrainingAccountabilityPlan"/>
                        </owl:unionOf>
                    </owl:Class>
                </owl:allValuesFrom>
            </owl:Restriction>
        </rdfs:subClassOf>
        <rdfs:comment>A planned step describing training user(s) to operate and/or maintain the AI System. This step is typically part of the Deployment Stage of an AI system&apos;s life cycle (specifically the User Training stage). This step has a member of the class User Training Report as its expected output. If a change has happened to deviate from how the guideline(s) indicate how training should have been done, then the step will also have as an output a member of the class Change Log.</rdfs:comment>
        <rdfs:label>Train User</rdfs:label>
    </owl:Class>
    


    <!-- https://w3id.org/rains#TrainingDataset -->


    <owl:Class rdf:about="https://w3id.org/rains#TrainingDataset">
        <rdfs:subClassOf rdf:resource="https://w3id.org/rains#DatasetComponent"/>
        <rdfs:subClassOf>
            <owl:Restriction>
                <owl:onProperty rdf:resource="https://w3id.org/ep-plan#isElementOfPlan"/>
                <owl:allValuesFrom rdf:resource="https://w3id.org/rains#ImplementationStageAccountabilityPlan"/>
            </owl:Restriction>
        </rdfs:subClassOf>
        <rdfs:subClassOf>
            <owl:Restriction>
                <owl:onProperty rdf:resource="https://w3id.org/ep-plan#isOutputVariableOf"/>
                <owl:allValuesFrom>
                    <owl:Class>
                        <owl:unionOf rdf:parseType="Collection">
                            <rdf:Description rdf:about="https://w3id.org/rains#MergeAndSplitDataset"/>
                            <rdf:Description rdf:about="https://w3id.org/rains#RealizeComponent"/>
                        </owl:unionOf>
                    </owl:Class>
                </owl:allValuesFrom>
            </owl:Restriction>
        </rdfs:subClassOf>
        <rdfs:subClassOf>
            <owl:Restriction>
                <owl:onProperty rdf:resource="https://w3id.org/ep-plan#isVariableOfPlan"/>
                <owl:allValuesFrom rdf:resource="https://w3id.org/rains#ImplementationStageAccountabilityPlan"/>
            </owl:Restriction>
        </rdfs:subClassOf>
        <rdfs:comment>A specific type of a Dataset Component  which represents a subset of the whole collected and pre-processed datasets after they were merged then split to be fed into the ML Model. This specific type represents the data used to train the ML Model. The other subsets are used to validate and evaluate the model. This accountable result is typically part of the Implementation stage of an AI System&apos;s life cycle.</rdfs:comment>
        <rdfs:label>Training Dataset</rdfs:label>
    </owl:Class>
    


    <!-- https://w3id.org/rains#UseCase -->


    <owl:Class rdf:about="https://w3id.org/rains#UseCase">
        <rdfs:subClassOf rdf:resource="https://w3id.org/sao#InformationElement"/>
        <rdfs:comment>A sao:InformationElement which records a specific piece of information detailing a situation in which any component of :AI_System or the system as whole could potentially be used.</rdfs:comment>
        <rdfs:label>Use Case</rdfs:label>
    </owl:Class>
    


    <!-- https://w3id.org/rains#UserConsent -->


    <owl:Class rdf:about="https://w3id.org/rains#UserConsent">
        <rdfs:subClassOf rdf:resource="https://w3id.org/rains#SystemData"/>
        <rdfs:subClassOf>
            <owl:Restriction>
                <owl:onProperty rdf:resource="https://w3id.org/ep-plan#isElementOfPlan"/>
                <owl:allValuesFrom>
                    <owl:Class>
                        <owl:unionOf rdf:parseType="Collection">
                            <rdf:Description rdf:about="https://w3id.org/rains#ConfigurationAccountabilityPlan"/>
                            <rdf:Description rdf:about="https://w3id.org/rains#OperationStageAccountabilityPlan"/>
                            <rdf:Description rdf:about="https://w3id.org/rains#RuntimeAccountabilityPlan"/>
                        </owl:unionOf>
                    </owl:Class>
                </owl:allValuesFrom>
            </owl:Restriction>
        </rdfs:subClassOf>
        <rdfs:subClassOf>
            <owl:Restriction>
                <owl:onProperty rdf:resource="https://w3id.org/ep-plan#isOutputVariableOf"/>
                <owl:allValuesFrom rdf:resource="https://w3id.org/rains#Consent"/>
            </owl:Restriction>
        </rdfs:subClassOf>
        <rdfs:subClassOf>
            <owl:Restriction>
                <owl:onProperty rdf:resource="https://w3id.org/ep-plan#isVariableOfPlan"/>
                <owl:allValuesFrom>
                    <owl:Class>
                        <owl:unionOf rdf:parseType="Collection">
                            <rdf:Description rdf:about="https://w3id.org/rains#ConfigurationAccountabilityPlan"/>
                            <rdf:Description rdf:about="https://w3id.org/rains#OperationStageAccountabilityPlan"/>
                            <rdf:Description rdf:about="https://w3id.org/rains#RuntimeAccountabilityPlan"/>
                        </owl:unionOf>
                    </owl:Class>
                </owl:allValuesFrom>
            </owl:Restriction>
        </rdfs:subClassOf>
        <owl:disjointWith rdf:resource="https://w3id.org/rains#UserReview"/>
        <owl:disjointWith rdf:resource="https://w3id.org/rains#Validation"/>
        <rdfs:comment>A specific type of planned System Data which represents the consent of the users to use or interact with the AI System.</rdfs:comment>
        <rdfs:label>User Consent</rdfs:label>
    </owl:Class>
    


    <!-- https://w3id.org/rains#UserReview -->


    <owl:Class rdf:about="https://w3id.org/rains#UserReview">
        <rdfs:subClassOf rdf:resource="https://w3id.org/rains#SystemData"/>
        <rdfs:subClassOf>
            <owl:Restriction>
                <owl:onProperty rdf:resource="https://w3id.org/ep-plan#isElementOfPlan"/>
                <owl:allValuesFrom>
                    <owl:Class>
                        <owl:unionOf rdf:parseType="Collection">
                            <rdf:Description rdf:about="https://w3id.org/rains#OperationStageAccountabilityPlan"/>
                            <rdf:Description rdf:about="https://w3id.org/rains#RuntimeAccountabilityPlan"/>
                        </owl:unionOf>
                    </owl:Class>
                </owl:allValuesFrom>
            </owl:Restriction>
        </rdfs:subClassOf>
        <rdfs:subClassOf>
            <owl:Restriction>
                <owl:onProperty rdf:resource="https://w3id.org/ep-plan#isOutputVariableOf"/>
                <owl:allValuesFrom rdf:resource="https://w3id.org/rains#CollectUserFeedback"/>
            </owl:Restriction>
        </rdfs:subClassOf>
        <rdfs:subClassOf>
            <owl:Restriction>
                <owl:onProperty rdf:resource="https://w3id.org/ep-plan#isVariableOfPlan"/>
                <owl:allValuesFrom>
                    <owl:Class>
                        <owl:unionOf rdf:parseType="Collection">
                            <rdf:Description rdf:about="https://w3id.org/rains#OperationStageAccountabilityPlan"/>
                            <rdf:Description rdf:about="https://w3id.org/rains#RuntimeAccountabilityPlan"/>
                        </owl:unionOf>
                    </owl:Class>
                </owl:allValuesFrom>
            </owl:Restriction>
        </rdfs:subClassOf>
        <owl:disjointWith rdf:resource="https://w3id.org/rains#Validation"/>
        <rdfs:comment>A specific type of planned System Data which represents the review of or feedback from the users to use on the final output of the AI System.</rdfs:comment>
        <rdfs:label>User Review</rdfs:label>
    </owl:Class>
    


    <!-- https://w3id.org/rains#UserTrainingAccountabilityPlan -->


    <owl:Class rdf:about="https://w3id.org/rains#UserTrainingAccountabilityPlan">
        <rdfs:subClassOf rdf:resource="https://w3id.org/rains#DeploymentStageAccountabilityPlan"/>
        <rdfs:comment>A plan that identifies sao:AccountableAction(s) and sao:AccountableResult(s) relevant to the training users as part of the deployment stage of an AI system and  which are required to be documented for accountability purposes. This plan is a subplan of the Deployment Stage Accountability Plan. The Accountable Actions that can be done at this stage are: Train User and Decide.</rdfs:comment>
        <rdfs:label>User Training Accountability Plan</rdfs:label>
    </owl:Class>
    


    <!-- https://w3id.org/rains#UserTrainingGuidance -->


    <owl:Class rdf:about="https://w3id.org/rains#UserTrainingGuidance">
        <rdfs:subClassOf rdf:resource="https://w3id.org/rains#SystemDeploymentGuidance"/>
        <rdfs:comment>A specific type of :Guidance which records a specific piece of information about the guidance to how the users of the :AI_System should be trained to use and maintain the system. This is separate from the manuals, as those are expressed using SystemMaintenanceGuidance and SystemUsageGuidance.</rdfs:comment>
        <rdfs:label>User Training Guidance</rdfs:label>
    </owl:Class>
    


    <!-- https://w3id.org/rains#UserTrainingGuideline -->


    <owl:Class rdf:about="https://w3id.org/rains#UserTrainingGuideline">
        <rdfs:subClassOf rdf:resource="https://w3id.org/rains#SystemDeploymentGuideline"/>
        <rdfs:subClassOf>
            <owl:Restriction>
                <owl:onProperty rdf:resource="https://w3id.org/ep-plan#isElementOfPlan"/>
                <owl:allValuesFrom>
                    <owl:Class>
                        <owl:unionOf rdf:parseType="Collection">
                            <rdf:Description rdf:about="https://w3id.org/rains#DeploymentStageAccountabilityPlan"/>
                            <rdf:Description rdf:about="https://w3id.org/rains#ImplementationStageAccountabilityPlan"/>
                            <rdf:Description rdf:about="https://w3id.org/rains#MaintenanceAccountabilityPlan"/>
                            <rdf:Description rdf:about="https://w3id.org/rains#OperationStageAccountabilityPlan"/>
                            <rdf:Description rdf:about="https://w3id.org/rains#RuntimeAccountabilityPlan"/>
                            <rdf:Description rdf:about="https://w3id.org/rains#UserTrainingAccountabilityPlan"/>
                        </owl:unionOf>
                    </owl:Class>
                </owl:allValuesFrom>
            </owl:Restriction>
        </rdfs:subClassOf>
        <rdfs:subClassOf>
            <owl:Restriction>
                <owl:onProperty rdf:resource="https://w3id.org/ep-plan#isOutputVariableOf"/>
                <owl:allValuesFrom rdf:resource="https://w3id.org/rains#GenerateGuideline"/>
            </owl:Restriction>
        </rdfs:subClassOf>
        <rdfs:subClassOf>
            <owl:Restriction>
                <owl:onProperty rdf:resource="https://w3id.org/ep-plan#isVariableOfPlan"/>
                <owl:allValuesFrom>
                    <owl:Class>
                        <owl:unionOf rdf:parseType="Collection">
                            <rdf:Description rdf:about="https://w3id.org/rains#DeploymentStageAccountabilityPlan"/>
                            <rdf:Description rdf:about="https://w3id.org/rains#ImplementationStageAccountabilityPlan"/>
                            <rdf:Description rdf:about="https://w3id.org/rains#MaintenanceAccountabilityPlan"/>
                            <rdf:Description rdf:about="https://w3id.org/rains#OperationStageAccountabilityPlan"/>
                            <rdf:Description rdf:about="https://w3id.org/rains#RuntimeAccountabilityPlan"/>
                            <rdf:Description rdf:about="https://w3id.org/rains#UserTrainingAccountabilityPlan"/>
                        </owl:unionOf>
                    </owl:Class>
                </owl:allValuesFrom>
            </owl:Restriction>
        </rdfs:subClassOf>
        <rdfs:comment>A specific type of System Deployment Guideline which represents the description of guidelines for the how to train the operators of the AI System on how to use and/or maintain the AI system.

It is advisable that the information realization corresponding to the System Deployment Guideline variable contains the information element: UserTrainingGuidance.</rdfs:comment>
        <rdfs:label>User Training Guideline</rdfs:label>
    </owl:Class>
    


    <!-- https://w3id.org/rains#UserTrainingReport -->


    <owl:Class rdf:about="https://w3id.org/rains#UserTrainingReport">
        <rdfs:subClassOf rdf:resource="https://w3id.org/sao#AccountableResult"/>
        <rdfs:subClassOf>
            <owl:Restriction>
                <owl:onProperty rdf:resource="https://w3id.org/ep-plan#isElementOfPlan"/>
                <owl:allValuesFrom>
                    <owl:Class>
                        <owl:unionOf rdf:parseType="Collection">
                            <rdf:Description rdf:about="https://w3id.org/rains#DeploymentStageAccountabilityPlan"/>
                            <rdf:Description rdf:about="https://w3id.org/rains#UserTrainingAccountabilityPlan"/>
                        </owl:unionOf>
                    </owl:Class>
                </owl:allValuesFrom>
            </owl:Restriction>
        </rdfs:subClassOf>
        <rdfs:subClassOf>
            <owl:Restriction>
                <owl:onProperty rdf:resource="https://w3id.org/ep-plan#isOutputVariableOf"/>
                <owl:allValuesFrom rdf:resource="https://w3id.org/rains#TrainUser"/>
            </owl:Restriction>
        </rdfs:subClassOf>
        <rdfs:subClassOf>
            <owl:Restriction>
                <owl:onProperty rdf:resource="https://w3id.org/ep-plan#isStepOfPlan"/>
                <owl:allValuesFrom>
                    <owl:Class>
                        <owl:unionOf rdf:parseType="Collection">
                            <rdf:Description rdf:about="https://w3id.org/rains#DeploymentStageAccountabilityPlan"/>
                            <rdf:Description rdf:about="https://w3id.org/rains#UserTrainingAccountabilityPlan"/>
                        </owl:unionOf>
                    </owl:Class>
                </owl:allValuesFrom>
            </owl:Restriction>
        </rdfs:subClassOf>
        <rdfs:comment>A specific type of planned sao:AccountableResult which represents a high level reference to a report describing how the users of the AI system were trained on the usage and/or maintenance of the AI System. This report is expected to be produced during the deployment stage (preferably using the subplan User Training Accountability Plan).

It is advisable that the information realization corresponding to the User Training Report variable contains the following information elements: Affected Agent (where each instance of Affected Agent corresponds to a trainee).</rdfs:comment>
        <rdfs:label>User Training Report</rdfs:label>
    </owl:Class>
    


    <!-- https://w3id.org/rains#Validate -->


    <owl:Class rdf:about="https://w3id.org/rains#Validate">
        <rdfs:subClassOf rdf:resource="https://w3id.org/rains#SystemAction"/>
        <rdfs:subClassOf>
            <owl:Restriction>
                <owl:onProperty rdf:resource="https://w3id.org/ep-plan#hasOutputVariable"/>
                <owl:allValuesFrom rdf:resource="https://w3id.org/rains#Validation"/>
            </owl:Restriction>
        </rdfs:subClassOf>
        <rdfs:subClassOf>
            <owl:Restriction>
                <owl:onProperty rdf:resource="https://w3id.org/ep-plan#isElementOfPlan"/>
                <owl:allValuesFrom>
                    <owl:Class>
                        <owl:unionOf rdf:parseType="Collection">
                            <rdf:Description rdf:about="https://w3id.org/rains#ConfigurationAccountabilityPlan"/>
                            <rdf:Description rdf:about="https://w3id.org/rains#DeploymentStageAccountabilityPlan"/>
                            <rdf:Description rdf:about="https://w3id.org/rains#InstallationAccountabilityPlan"/>
                            <rdf:Description rdf:about="https://w3id.org/rains#OperationStageAccountabilityPlan"/>
                            <rdf:Description rdf:about="https://w3id.org/rains#RuntimeAccountabilityPlan"/>
                        </owl:unionOf>
                    </owl:Class>
                </owl:allValuesFrom>
            </owl:Restriction>
        </rdfs:subClassOf>
        <rdfs:subClassOf>
            <owl:Restriction>
                <owl:onProperty rdf:resource="https://w3id.org/ep-plan#isStepOfPlan"/>
                <owl:allValuesFrom>
                    <owl:Class>
                        <owl:unionOf rdf:parseType="Collection">
                            <rdf:Description rdf:about="https://w3id.org/rains#ConfigurationAccountabilityPlan"/>
                            <rdf:Description rdf:about="https://w3id.org/rains#DeploymentStageAccountabilityPlan"/>
                            <rdf:Description rdf:about="https://w3id.org/rains#InstallationAccountabilityPlan"/>
                            <rdf:Description rdf:about="https://w3id.org/rains#OperationStageAccountabilityPlan"/>
                            <rdf:Description rdf:about="https://w3id.org/rains#RuntimeAccountabilityPlan"/>
                        </owl:unionOf>
                    </owl:Class>
                </owl:allValuesFrom>
            </owl:Restriction>
        </rdfs:subClassOf>
        <rdfs:comment>A planned step that has some impact on the output of AI System where an output generated by a Supporting Infrastructure component or Model component is validated by a Supporting Infrastructure component. This step is typically part of the Deployment or Operation stages (specifically Installation, Configuration, or Runtime stages). This step has a member of the class Validation as its expected output.</rdfs:comment>
        <rdfs:label>Validate</rdfs:label>
    </owl:Class>
    


    <!-- https://w3id.org/rains#Validation -->


    <owl:Class rdf:about="https://w3id.org/rains#Validation">
        <rdfs:subClassOf rdf:resource="https://w3id.org/rains#SystemData"/>
        <rdfs:subClassOf>
            <owl:Restriction>
                <owl:onProperty rdf:resource="https://w3id.org/ep-plan#isElementOfPlan"/>
                <owl:allValuesFrom>
                    <owl:Class>
                        <owl:unionOf rdf:parseType="Collection">
                            <rdf:Description rdf:about="https://w3id.org/rains#ConfigurationAccountabilityPlan"/>
                            <rdf:Description rdf:about="https://w3id.org/rains#DeploymentStageAccountabilityPlan"/>
                            <rdf:Description rdf:about="https://w3id.org/rains#InstallationAccountabilityPlan"/>
                            <rdf:Description rdf:about="https://w3id.org/rains#OperationStageAccountabilityPlan"/>
                            <rdf:Description rdf:about="https://w3id.org/rains#RuntimeAccountabilityPlan"/>
                        </owl:unionOf>
                    </owl:Class>
                </owl:allValuesFrom>
            </owl:Restriction>
        </rdfs:subClassOf>
        <rdfs:subClassOf>
            <owl:Restriction>
                <owl:onProperty rdf:resource="https://w3id.org/ep-plan#isOutputVariableOf"/>
                <owl:allValuesFrom rdf:resource="https://w3id.org/rains#Validate"/>
            </owl:Restriction>
        </rdfs:subClassOf>
        <rdfs:subClassOf>
            <owl:Restriction>
                <owl:onProperty rdf:resource="https://w3id.org/ep-plan#isVariableOfPlan"/>
                <owl:allValuesFrom>
                    <owl:Class>
                        <owl:unionOf rdf:parseType="Collection">
                            <rdf:Description rdf:about="https://w3id.org/rains#ConfigurationAccountabilityPlan"/>
                            <rdf:Description rdf:about="https://w3id.org/rains#DeploymentStageAccountabilityPlan"/>
                            <rdf:Description rdf:about="https://w3id.org/rains#InstallationAccountabilityPlan"/>
                            <rdf:Description rdf:about="https://w3id.org/rains#OperationStageAccountabilityPlan"/>
                            <rdf:Description rdf:about="https://w3id.org/rains#RuntimeAccountabilityPlan"/>
                        </owl:unionOf>
                    </owl:Class>
                </owl:allValuesFrom>
            </owl:Restriction>
        </rdfs:subClassOf>
        <rdfs:comment>A specific type of planned System Data which represents the information related to validating Configuration Data, Runtime Input Data, Model Output, or System Output..

It is advisable that the information realization corresponding to the Validation variable contains the following information elements:
1. Validation Result
2. Affected Agent if the AI System is involved in making decisions/recommendations/actions affecting human users.</rdfs:comment>
        <rdfs:label>Validation</rdfs:label>
    </owl:Class>
    


    <!-- https://w3id.org/rains#ValidationDataset -->


    <owl:Class rdf:about="https://w3id.org/rains#ValidationDataset">
        <rdfs:subClassOf rdf:resource="https://w3id.org/rains#DatasetComponent"/>
        <rdfs:subClassOf>
            <owl:Restriction>
                <owl:onProperty rdf:resource="https://w3id.org/ep-plan#isElementOfPlan"/>
                <owl:allValuesFrom rdf:resource="https://w3id.org/rains#ImplementationStageAccountabilityPlan"/>
            </owl:Restriction>
        </rdfs:subClassOf>
        <rdfs:subClassOf>
            <owl:Restriction>
                <owl:onProperty rdf:resource="https://w3id.org/ep-plan#isOutputVariableOf"/>
                <owl:allValuesFrom>
                    <owl:Class>
                        <owl:unionOf rdf:parseType="Collection">
                            <rdf:Description rdf:about="https://w3id.org/rains#MergeAndSplitDataset"/>
                            <rdf:Description rdf:about="https://w3id.org/rains#RealizeComponent"/>
                        </owl:unionOf>
                    </owl:Class>
                </owl:allValuesFrom>
            </owl:Restriction>
        </rdfs:subClassOf>
        <rdfs:subClassOf>
            <owl:Restriction>
                <owl:onProperty rdf:resource="https://w3id.org/ep-plan#isVariableOfPlan"/>
                <owl:allValuesFrom rdf:resource="https://w3id.org/rains#ImplementationStageAccountabilityPlan"/>
            </owl:Restriction>
        </rdfs:subClassOf>
        <rdfs:comment>A specific type of a Dataset Component  which represents a subset of the whole collected and pre-processed datasets after they were merged then split to be fed into the ML Model. This specific type represents the data used to validate the ML Model. The dataset is typically used repeatedly during the hyperparameter tuning process. The other subsets are used to train and evaluate the model.  This accountable result is typically part of the Implementation stage of an AI System&apos;s life cycle.</rdfs:comment>
        <rdfs:label>Validation Dataset</rdfs:label>
    </owl:Class>
    


    <!-- https://w3id.org/rains#ValidationResult -->


    <owl:Class rdf:about="https://w3id.org/rains#ValidationResult">
        <rdfs:subClassOf rdf:resource="https://w3id.org/sao#InformationElement"/>
        <rdfs:comment>A type of :RealizableObjectCharacteristic describing the results of validating Configuration  Data, Runtime Input Data, Model Putput, or System Output.</rdfs:comment>
        <rdfs:label>Validation Result</rdfs:label>
    </owl:Class>
    


    <!-- https://w3id.org/sao#AccountabilityPlan -->


    <owl:Class rdf:about="https://w3id.org/sao#AccountabilityPlan"/>
    


    <!-- https://w3id.org/sao#AccountableAction -->


    <owl:Class rdf:about="https://w3id.org/sao#AccountableAction"/>
    


    <!-- https://w3id.org/sao#AccountableAgent -->


    <owl:Class rdf:about="https://w3id.org/sao#AccountableAgent">
        <rdfs:subClassOf rdf:resource="https://w3id.org/ep-plan#Agent"/>
        <rdfs:subClassOf rdf:resource="https://w3id.org/sao#InformationElement"/>
        <rdfs:comment>An agent that can be held accountable for his/her actions. While the agent may typically be a human, components of the AI System, namely, Model Component and Supporting Infrastructure Component, may also be considered accountable to the actions they perform within the system context. This is for documentation purposes, and legal accountability should be traced to the human agent accountable for the component in question. For example, in the context of a facial recognition AI System, the model is accountable for generating a decision about whether it can recongnise a user&apos;s. However, legally, the humans behing the model are those who are to be held finally held accountable in reality.
Note that, within the same AI System a human may take on the role of both or either Affected Agent or Accountable Agent. For example, a user may be accountable for installing and configuring a facial recognition AI system, but may later be affected by the AI System&apos;s output of recognision or not recognision their face. Then may then also be accountable for overriding the system&apos;s output by using a manual passcode.</rdfs:comment>
        <rdfs:label>Accountable Agent</rdfs:label>
    </owl:Class>
    


    <!-- https://w3id.org/sao#AccountableResult -->


    <owl:Class rdf:about="https://w3id.org/sao#AccountableResult"/>
    


    <!-- https://w3id.org/sao#InformationElement -->


    <owl:Class rdf:about="https://w3id.org/sao#InformationElement"/>
    


    <!-- https://w3id.org/sao#InformationRealization -->


    <owl:Class rdf:about="https://w3id.org/sao#InformationRealization"/>
    


    <!-- https://w3id.org/sao#System -->


    <owl:Class rdf:about="https://w3id.org/sao#System"/>
    


    <!-- 
    ///////////////////////////////////////////////////////////////////////////////////////
    //
    // General axioms
    //
    ///////////////////////////////////////////////////////////////////////////////////////
     -->


    <rdf:Description>
        <rdf:type rdf:resource="http://www.w3.org/2002/07/owl#AllDisjointClasses"/>
        <owl:members rdf:parseType="Collection">
            <rdf:Description rdf:about="http://www.w3.org/ns/mls#Algorithm"/>
            <rdf:Description rdf:about="http://www.w3.org/ns/mls#DatasetCharacteristic"/>
            <rdf:Description rdf:about="http://www.w3.org/ns/mls#ModelCharacteristic"/>
            <rdf:Description rdf:about="https://w3id.org/rains#SystemAuditMechanism"/>
            <rdf:Description rdf:about="https://w3id.org/rains#SystemExplanationMechanism"/>
            <rdf:Description rdf:about="https://w3id.org/rains#SystemHumanOversightMechanism"/>
            <rdf:Description rdf:about="https://w3id.org/rains#SystemSecurityMechanism"/>
        </owl:members>
    </rdf:Description>
    <rdf:Description>
        <rdf:type rdf:resource="http://www.w3.org/2002/07/owl#AllDisjointClasses"/>
        <owl:members rdf:parseType="Collection">
            <rdf:Description rdf:about="http://www.w3.org/ns/mls#Dataset"/>
            <rdf:Description rdf:about="http://www.w3.org/ns/mls#Model"/>
            <rdf:Description rdf:about="https://w3id.org/rains#SupportingInfrastructure"/>
        </owl:members>
    </rdf:Description>
    <rdf:Description>
        <rdf:type rdf:resource="http://www.w3.org/2002/07/owl#AllDisjointClasses"/>
        <owl:members rdf:parseType="Collection">
            <rdf:Description rdf:about="https://w3id.org/rains#ApprovalDecision"/>
            <rdf:Description rdf:about="https://w3id.org/rains#ComplianceAssuranceDecision"/>
            <rdf:Description rdf:about="https://w3id.org/rains#FitnessConfirmationDecision"/>
        </owl:members>
    </rdf:Description>
    <rdf:Description>
        <rdf:type rdf:resource="http://www.w3.org/2002/07/owl#AllDisjointClasses"/>
        <owl:members rdf:parseType="Collection">
            <rdf:Description rdf:about="https://w3id.org/rains#DeploymentStageAccountabilityPlan"/>
            <rdf:Description rdf:about="https://w3id.org/rains#DesignStageAccountabilityPlan"/>
            <rdf:Description rdf:about="https://w3id.org/rains#ImplementationStageAccountabilityPlan"/>
            <rdf:Description rdf:about="https://w3id.org/rains#OperationStageAccountabilityPlan"/>
        </owl:members>
    </rdf:Description>
</rdf:RDF>



<!-- Generated by the OWL API (version 5.1.18) https://github.com/owlcs/owlapi/ -->


